<?xml version="1.0"?>
<rdf:RDF xmlns="http://purl.org/net/iot-dm#"
     xml:base="http://purl.org/net/iot-dm"
     xmlns:rdf="http://www.w3.org/1999/02/22-rdf-syntax-ns#"
     xmlns:owl="http://www.w3.org/2002/07/owl#"
     xmlns:xml="http://www.w3.org/XML/1998/namespace"
     xmlns:xsd="http://www.w3.org/2001/XMLSchema#"
     xmlns:rdfs="http://www.w3.org/2000/01/rdf-schema#">
    <owl:Ontology rdf:about="http://purl.org/net/iot-dm">
        <owl:versionIRI rdf:resource="http://purl.org/net/iot-dm/1.0.0"/>
    </owl:Ontology>
    


    <!-- 
    ///////////////////////////////////////////////////////////////////////////////////////
    //
    // Object Properties
    //
    ///////////////////////////////////////////////////////////////////////////////////////
     -->

    


    <!-- http://purl.org/net/iot-dm#OWLObjectProperty_0fa7eb28_bcfe_4d58_a7aa_e774be01ebdf -->

    <owl:ObjectProperty rdf:about="http://purl.org/net/iot-dm#OWLObjectProperty_0fa7eb28_bcfe_4d58_a7aa_e774be01ebdf">
        <rdfs:subPropertyOf rdf:resource="http://www.w3.org/2002/07/owl#topObjectProperty"/>
        <rdfs:domain rdf:resource="http://purl.org/net/iot-dm#OWLClass_44ddb928_3187_4588_90e9_512f4856bf45"/>
        <rdfs:range rdf:resource="http://purl.org/net/iot-dm#OWLClass_15514c90_84d5_4670_93a6_9566cb808feb"/>
        <rdfs:label xml:lang="en">pointsTo</rdfs:label>
    </owl:ObjectProperty>
    


    <!-- http://purl.org/net/iot-dm#OWLObjectProperty_182c885b_d191_4d34_9277_d43a50df590e -->

    <owl:ObjectProperty rdf:about="http://purl.org/net/iot-dm#OWLObjectProperty_182c885b_d191_4d34_9277_d43a50df590e">
        <rdfs:domain rdf:resource="http://purl.org/net/iot-dm#OWLClass_49ac79d7_c437_4c71_8da3_ae6ad1e83073"/>
        <rdfs:range rdf:resource="http://purl.org/net/iot-dm#OWLClass_15514c90_84d5_4670_93a6_9566cb808feb"/>
        <rdfs:range rdf:resource="http://purl.org/net/iot-dm#OWLClass_9706d318_5cd1_4e58_8c3b_72eef36ee70a"/>
        <rdfs:label xml:lang="en">creates</rdfs:label>
    </owl:ObjectProperty>
    


    <!-- http://purl.org/net/iot-dm#OWLObjectProperty_69b46ca5_a154_4bae_848a_e2dc350180da -->

    <owl:ObjectProperty rdf:about="http://purl.org/net/iot-dm#OWLObjectProperty_69b46ca5_a154_4bae_848a_e2dc350180da">
        <rdfs:domain rdf:resource="http://purl.org/net/iot-dm#OWLClass_3a4d744e_1ddc_4fc8_be82_966b2e491882"/>
        <rdfs:range rdf:resource="http://purl.org/net/iot-dm#OWLClass_15514c90_84d5_4670_93a6_9566cb808feb"/>
        <rdfs:range rdf:resource="http://purl.org/net/iot-dm#OWLClass_9706d318_5cd1_4e58_8c3b_72eef36ee70a"/>
        <rdfs:label xml:lang="en">stores</rdfs:label>
    </owl:ObjectProperty>
    


    <!-- http://purl.org/net/iot-dm#OWLObjectProperty_ccd9d9c0_cf1c_4123_b7d8_5d83be47ef1e -->

    <owl:ObjectProperty rdf:about="http://purl.org/net/iot-dm#OWLObjectProperty_ccd9d9c0_cf1c_4123_b7d8_5d83be47ef1e">
        <rdfs:subPropertyOf rdf:resource="http://www.w3.org/2002/07/owl#topObjectProperty"/>
        <rdfs:domain rdf:resource="http://purl.org/net/iot-dm#OWLClass_1d708038_ca44_4723_a910_a811401f688c"/>
        <rdfs:range rdf:resource="http://purl.org/net/iot-dm#OWLClass_9e3d4f19_96c7_4932_a007_26fa592f3423"/>
        <rdfs:comment>draft-moran-suit-architecture-03 (work in progress), p. 6</rdfs:comment>
        <rdfs:label xml:lang="en">shallBeDeliverableToMany</rdfs:label>
    </owl:ObjectProperty>
    


    <!-- http://purl.org/net/iot-dm#OWLObjectProperty_e135cd77_59dc_4f60_97ed_d0ed0948aa4e -->

    <owl:ObjectProperty rdf:about="http://purl.org/net/iot-dm#OWLObjectProperty_e135cd77_59dc_4f60_97ed_d0ed0948aa4e">
        <rdfs:domain rdf:resource="http://purl.org/net/iot-dm#OWLClass_4948fab8_1838_4fe0_82a0_27a8ac8eded5"/>
        <rdfs:range rdf:resource="http://purl.org/net/iot-dm#OWLClass_cfe637aa_ec08_45c2_88c1_6a6c989d5b1e"/>
        <rdfs:range rdf:resource="http://purl.org/net/iot-dm#OWLClass_f1b54d5c_4482_4645_a2f1_6efa8e12b8de"/>
        <rdfs:comment>draft-moran-suit-architecture-03 (work in progress), p. 6</rdfs:comment>
        <rdfs:label xml:lang="en">shallBeAgnosticTo</rdfs:label>
    </owl:ObjectProperty>
    


    <!-- 
    ///////////////////////////////////////////////////////////////////////////////////////
    //
    // Classes
    //
    ///////////////////////////////////////////////////////////////////////////////////////
     -->

    


    <!-- http://purl.org/net/iot-dm#OWLClass_00acf628_285b_4f11_9b67_ef07dc8022cb -->

    <owl:Class rdf:about="http://purl.org/net/iot-dm#OWLClass_00acf628_285b_4f11_9b67_ef07dc8022cb">
        <rdfs:subClassOf rdf:resource="http://purl.org/net/iot-dm#OWLClass_3300e6af_4338_4bf4_ab9e_632af0b5ad65"/>
        <rdfs:comment>OMA-RD-LightweightM2M-V1_0-20170208-A, Label: LightweightM2M-HLF-023</rdfs:comment>
        <rdfs:comment>Recent Advances in Industrial Wireless Sensor Networks Towards Efficient Management in IoT, p. 8</rdfs:comment>
        <rdfs:label xml:lang="en">DeviceConfigurationInitialization</rdfs:label>
        <rdfs:seeAlso>DeviceBootstrapProvisioning</rdfs:seeAlso>
    </owl:Class>
    


    <!-- http://purl.org/net/iot-dm#OWLClass_01f43ad7_3f28_4ffd_a863_c81e5312a767 -->

    <owl:Class rdf:about="http://purl.org/net/iot-dm#OWLClass_01f43ad7_3f28_4ffd_a863_c81e5312a767">
        <rdfs:subClassOf rdf:resource="http://purl.org/net/iot-dm#OWLClass_f6444fa6_1240_4dfa_9bba_affd175076ca"/>
        <rdfs:comment>OMA-RD-LightweightM2M-V1_1-20180710-A, Label: LightweightM2M-IR-001</rdfs:comment>
        <rdfs:label xml:lang="en">ReportingOfResourcesAcrossDifferentObjectsInOneNotification</rdfs:label>
    </owl:Class>
    


    <!-- http://purl.org/net/iot-dm#OWLClass_032afd50_d465_4cb9_9d7d_4042fed8c7cb -->

    <owl:Class rdf:about="http://purl.org/net/iot-dm#OWLClass_032afd50_d465_4cb9_9d7d_4042fed8c7cb">
        <rdfs:subClassOf rdf:resource="http://purl.org/net/iot-dm#OWLClass_0b06f64b_69d9_4b6c_965b_186dc58c39eb"/>
        <rdfs:comment>Recent Advances in Industrial Wireless Sensor Networks Towards Efficient Management in IoT, p. 13</rdfs:comment>
        <rdfs:label xml:lang="en">EventAnalytics</rdfs:label>
    </owl:Class>
    


    <!-- http://purl.org/net/iot-dm#OWLClass_04312c30_fd26_4307_ab50_03991e776620 -->

    <owl:Class rdf:about="http://purl.org/net/iot-dm#OWLClass_04312c30_fd26_4307_ab50_03991e776620">
        <rdfs:subClassOf rdf:resource="http://purl.org/net/iot-dm#OWLClass_5985dbe5_dc91_4677_a070_127370474bb9"/>
        <rdfs:label xml:lang="en">DataReportingConfiguration</rdfs:label>
    </owl:Class>
    


    <!-- http://purl.org/net/iot-dm#OWLClass_04b7e838_4035_4343_a9df_bc2e65615ff2 -->

    <owl:Class rdf:about="http://purl.org/net/iot-dm#OWLClass_04b7e838_4035_4343_a9df_bc2e65615ff2">
        <rdfs:subClassOf rdf:resource="http://purl.org/net/iot-dm#OWLClass_b6721ba6_4ea5_4be0_b34f_ff739be47358"/>
        <rdfs:comment>draft-moran-suit-architecture-03 (work in progress), p. 8-9</rdfs:comment>
        <rdfs:label xml:lang="en">FirmwareUpdatePolicyCheck</rdfs:label>
    </owl:Class>
    


    <!-- http://purl.org/net/iot-dm#OWLClass_04f7335a_fba0_46a8_921f_c743fd57f99f -->

    <owl:Class rdf:about="http://purl.org/net/iot-dm#OWLClass_04f7335a_fba0_46a8_921f_c743fd57f99f">
        <rdfs:subClassOf rdf:resource="http://purl.org/net/iot-dm#OWLClass_a1cefa89_8494_4c67_8d71_44f07b80a613"/>
        <rdfs:comment>OMA-RD-LightweightM2M-V1_1-20180710-A, Label: LightweightM2M-MaU-5</rdfs:comment>
        <rdfs:label xml:lang="en">ConfigurableLagMode</rdfs:label>
    </owl:Class>
    


    <!-- http://purl.org/net/iot-dm#OWLClass_052ba795_e3ac_4e59_831a_65d381fe5a0a -->

    <owl:Class rdf:about="http://purl.org/net/iot-dm#OWLClass_052ba795_e3ac_4e59_831a_65d381fe5a0a">
        <rdfs:subClassOf rdf:resource="http://purl.org/net/iot-dm#OWLClass_d8e49365_06e1_40c2_99fc_891f2256aad1"/>
        <rdfs:comment>IoT home gateway for auto-conﬁguration and management of MQTT devices, section I.</rdfs:comment>
        <rdfs:label xml:lang="en">Upnp</rdfs:label>
    </owl:Class>
    


    <!-- http://purl.org/net/iot-dm#OWLClass_0543cda5_5052_48ab_8952_a680849ce015 -->

    <owl:Class rdf:about="http://purl.org/net/iot-dm#OWLClass_0543cda5_5052_48ab_8952_a680849ce015">
        <rdfs:subClassOf rdf:resource="http://purl.org/net/iot-dm#OWLClass_36c8fbfb_7218_4373_a13b_f46a86f007be"/>
        <rdfs:comment>Management of IoT Devices in a Physical Network, p. 486</rdfs:comment>
        <rdfs:label xml:lang="en">DeviceConfiguration</rdfs:label>
    </owl:Class>
    


    <!-- http://purl.org/net/iot-dm#OWLClass_05c0294e_e33a_42c4_9511_e240252afc2f -->

    <owl:Class rdf:about="http://purl.org/net/iot-dm#OWLClass_05c0294e_e33a_42c4_9511_e240252afc2f">
        <rdfs:subClassOf rdf:resource="http://purl.org/net/iot-dm#OWLClass_71dcf03b_6cc1_4da4_9574_874b4477d105"/>
        <rdfs:comment>https://resin.io/how-it-works/, 2019-09-16</rdfs:comment>
        <rdfs:label xml:lang="en">ContainerRegistry</rdfs:label>
    </owl:Class>
    


    <!-- http://purl.org/net/iot-dm#OWLClass_07f63ab8_1777_4c84_9e30_270e3e84c754 -->

    <owl:Class rdf:about="http://purl.org/net/iot-dm#OWLClass_07f63ab8_1777_4c84_9e30_270e3e84c754">
        <rdfs:subClassOf rdf:resource="http://purl.org/net/iot-dm#OWLClass_09ca2bb4_ca54_4693_816d_f45ba81e59fb"/>
        <rdfs:comment>OMA-RD-LightweightM2M-V1_1-20180710-A, Label: LightweightM2M-LeG-003</rdfs:comment>
        <rdfs:label xml:lang="en">DevicesBehindGateway</rdfs:label>
    </owl:Class>
    


    <!-- http://purl.org/net/iot-dm#OWLClass_0802d184_c79b_4c44_be1c_441d20d3adc4 -->

    <owl:Class rdf:about="http://purl.org/net/iot-dm#OWLClass_0802d184_c79b_4c44_be1c_441d20d3adc4">
        <rdfs:subClassOf rdf:resource="http://purl.org/net/iot-dm#OWLClass_0b06f64b_69d9_4b6c_965b_186dc58c39eb"/>
        <rdfs:comment>Recent Advances in Industrial Wireless Sensor Networks Towards Efficient Management in IoT, p. 8</rdfs:comment>
        <rdfs:label xml:lang="en">MultipleManagementDataSourcesSupport</rdfs:label>
    </owl:Class>
    


    <!-- http://purl.org/net/iot-dm#OWLClass_08385527_c024_48c2_986f_4df96714e457 -->

    <owl:Class rdf:about="http://purl.org/net/iot-dm#OWLClass_08385527_c024_48c2_986f_4df96714e457">
        <rdfs:subClassOf rdf:resource="http://purl.org/net/iot-dm#OWLClass_2281b85a_ace5_4ac3_910f_536f7370505e"/>
        <rdfs:comment>Recent Advances in Industrial Wireless Sensor Networks Towards Efficient Management in IoT, p. 6</rdfs:comment>
        <rdfs:label xml:lang="en">DeviceControlInterface</rdfs:label>
    </owl:Class>
    


    <!-- http://purl.org/net/iot-dm#OWLClass_09418094_9786_4ff2_b5d0_38f24fa88661 -->

    <owl:Class rdf:about="http://purl.org/net/iot-dm#OWLClass_09418094_9786_4ff2_b5d0_38f24fa88661">
        <rdfs:subClassOf rdf:resource="http://purl.org/net/iot-dm#OWLClass_89f81fe4_c0d0_4dd1_b866_babbba4f20de"/>
        <rdfs:comment>https://resin.io/features/, 2018-09-15</rdfs:comment>
        <rdfs:label xml:lang="en">TwoFactorAuthentication</rdfs:label>
    </owl:Class>
    


    <!-- http://purl.org/net/iot-dm#OWLClass_096a024f_bfdd_4fde_8523_ed1d37d8c23e -->

    <owl:Class rdf:about="http://purl.org/net/iot-dm#OWLClass_096a024f_bfdd_4fde_8523_ed1d37d8c23e">
        <rdfs:subClassOf rdf:resource="http://purl.org/net/iot-dm#OWLClass_66c3fc69_337f_4795_a467_f0b64b90cb3b"/>
        <rdfs:comment>Recent Advances in Industrial Wireless Sensor Networks Towards Efficient Management in IoT, p. 6, 12</rdfs:comment>
        <rdfs:label xml:lang="en">QualityOfServiceGuarantee</rdfs:label>
    </owl:Class>
    


    <!-- http://purl.org/net/iot-dm#OWLClass_098db16c_fb93_4aca_8bc2_5b421cfed288 -->

    <owl:Class rdf:about="http://purl.org/net/iot-dm#OWLClass_098db16c_fb93_4aca_8bc2_5b421cfed288">
        <rdfs:subClassOf rdf:resource="http://purl.org/net/iot-dm#OWLClass_845f9a81_9845_4e96_b5cf_5d06ab798969"/>
        <rdfs:comment>Management of IoT Devices in a Physical Network, p. 487</rdfs:comment>
        <rdfs:label xml:lang="en">RealTimeEventAnalytics</rdfs:label>
    </owl:Class>
    


    <!-- http://purl.org/net/iot-dm#OWLClass_09ca2bb4_ca54_4693_816d_f45ba81e59fb -->

    <owl:Class rdf:about="http://purl.org/net/iot-dm#OWLClass_09ca2bb4_ca54_4693_816d_f45ba81e59fb">
        <rdfs:subClassOf rdf:resource="http://purl.org/net/iot-dm#OWLClass_843d87bc_a343_470f_bff0_872b15b14c16"/>
        <rdfs:label xml:lang="en">DeviceSupport</rdfs:label>
    </owl:Class>
    


    <!-- http://purl.org/net/iot-dm#OWLClass_0a007f07_35b8_403d_b457_247dceeb4e16 -->

    <owl:Class rdf:about="http://purl.org/net/iot-dm#OWLClass_0a007f07_35b8_403d_b457_247dceeb4e16">
        <rdfs:subClassOf rdf:resource="http://purl.org/net/iot-dm#OWLClass_04312c30_fd26_4307_ab50_03991e776620"/>
        <rdfs:comment>OMA-RD-LightweightM2M-V1_1-20180710-A, Label: LightweightM2M-DSE-004</rdfs:comment>
        <rdfs:label xml:lang="en">UnsolicitedDataReportingConfiguration</rdfs:label>
    </owl:Class>
    


    <!-- http://purl.org/net/iot-dm#OWLClass_0b06f64b_69d9_4b6c_965b_186dc58c39eb -->

    <owl:Class rdf:about="http://purl.org/net/iot-dm#OWLClass_0b06f64b_69d9_4b6c_965b_186dc58c39eb">
        <rdfs:subClassOf rdf:resource="http://purl.org/net/iot-dm#OWLClass_b21422b7_b049_4b16_b3e0_53d1c9d53e85"/>
        <rdfs:comment>Recent Advances in Industrial Wireless Sensor Networks Towards Efficient Management in IoT, p. 6</rdfs:comment>
        <rdfs:label xml:lang="en">DeviceManagementAnalytics</rdfs:label>
    </owl:Class>
    


    <!-- http://purl.org/net/iot-dm#OWLClass_0b36c390_a253_4c36_97a2_46cd2749e411 -->

    <owl:Class rdf:about="http://purl.org/net/iot-dm#OWLClass_0b36c390_a253_4c36_97a2_46cd2749e411">
        <rdfs:subClassOf rdf:resource="http://purl.org/net/iot-dm#OWLClass_4c69f2df_35c9_4bf1_8b7f_b0e8fcac7aca"/>
        <rdfs:comment>https://resin.io/how-it-works/, 2019-09-16</rdfs:comment>
        <rdfs:label xml:lang="en">ImageNotBootable</rdfs:label>
    </owl:Class>
    


    <!-- http://purl.org/net/iot-dm#OWLClass_0b54422a_6554_4d67_9f00_88c2284689a6 -->

    <owl:Class rdf:about="http://purl.org/net/iot-dm#OWLClass_0b54422a_6554_4d67_9f00_88c2284689a6">
        <rdfs:subClassOf rdf:resource="http://purl.org/net/iot-dm#OWLClass_62fae845_5a8c_4d71_980f_2f8cea75de35"/>
        <rdfs:comment>IoT home gateway for auto-conﬁguration and management of MQTT devices, section III.</rdfs:comment>
        <rdfs:label xml:lang="en">DeviceControlMessageParsing</rdfs:label>
    </owl:Class>
    


    <!-- http://purl.org/net/iot-dm#OWLClass_0b74afc7_ab6a_480c_91c1_fe26c00b8297 -->

    <owl:Class rdf:about="http://purl.org/net/iot-dm#OWLClass_0b74afc7_ab6a_480c_91c1_fe26c00b8297">
        <rdfs:subClassOf rdf:resource="http://purl.org/net/iot-dm#OWLClass_c74a5982_d5bc_40b3_9e18_c03e025b5949"/>
        <rdfs:comment>draft-moran-suit-architecture-03 (work in progress), p. 7</rdfs:comment>
        <rdfs:label xml:lang="en">FlashSupport</rdfs:label>
    </owl:Class>
    


    <!-- http://purl.org/net/iot-dm#OWLClass_0badcf63_2acc_493f_937a_d8aa3625f97c -->

    <owl:Class rdf:about="http://purl.org/net/iot-dm#OWLClass_0badcf63_2acc_493f_937a_d8aa3625f97c">
        <rdfs:subClassOf rdf:resource="http://purl.org/net/iot-dm#OWLClass_201d2207_e63c_4bd0_ac8e_dac6fd8b7d61"/>
        <rdfs:label xml:lang="en">OperatingSystemManagement</rdfs:label>
    </owl:Class>
    


    <!-- http://purl.org/net/iot-dm#OWLClass_0bbb7819_d9df_4553_8196_2a8ee5c4c6e6 -->

    <owl:Class rdf:about="http://purl.org/net/iot-dm#OWLClass_0bbb7819_d9df_4553_8196_2a8ee5c4c6e6">
        <rdfs:label xml:lang="en">InternetOfThingsGateway</rdfs:label>
    </owl:Class>
    


    <!-- http://purl.org/net/iot-dm#OWLClass_0c29c03d_ca35_4020_8fbc_14a78bbc0e6c -->

    <owl:Class rdf:about="http://purl.org/net/iot-dm#OWLClass_0c29c03d_ca35_4020_8fbc_14a78bbc0e6c">
        <rdfs:subClassOf rdf:resource="http://purl.org/net/iot-dm#OWLClass_2fb332cc_9b13_4fbc_af07_4ce1a662e062"/>
        <rdfs:comment>OMA-RD-LightweightM2M-V1_0-20170208-A, Label: LightweightM2M-HLF-030</rdfs:comment>
        <rdfs:label xml:lang="en">DeviceState</rdfs:label>
    </owl:Class>
    


    <!-- http://purl.org/net/iot-dm#OWLClass_0c4e8a84_78ff_41fc_9998_b9845dc97245 -->

    <owl:Class rdf:about="http://purl.org/net/iot-dm#OWLClass_0c4e8a84_78ff_41fc_9998_b9845dc97245">
        <rdfs:subClassOf rdf:resource="http://purl.org/net/iot-dm#OWLClass_1bd19af8_5e90_482f_b798_79ba7cc8d671"/>
        <rdfs:comment>Recent Advances in Industrial Wireless Sensor Networks Towards Efficient Management in IoT, p. 6</rdfs:comment>
        <rdfs:label xml:lang="en">IotComponentReuse</rdfs:label>
    </owl:Class>
    


    <!-- http://purl.org/net/iot-dm#OWLClass_0cdc7aba_2679_474c_b3aa_4b7b9032cb93 -->

    <owl:Class rdf:about="http://purl.org/net/iot-dm#OWLClass_0cdc7aba_2679_474c_b3aa_4b7b9032cb93">
        <rdfs:subClassOf rdf:resource="http://purl.org/net/iot-dm#OWLClass_2c177064_e630_44da_bbb3_d692886a8e4a"/>
        <rdfs:comment>OMA-RD-LightweightM2M-V1_1-20180710-A, Label: LightweightM2M-BsR-007</rdfs:comment>
        <rdfs:label xml:lang="en">BootstrapServiceValidation</rdfs:label>
    </owl:Class>
    


    <!-- http://purl.org/net/iot-dm#OWLClass_0d559ba6_e600_4ffa_a199_bc283051b376 -->

    <owl:Class rdf:about="http://purl.org/net/iot-dm#OWLClass_0d559ba6_e600_4ffa_a199_bc283051b376">
        <rdfs:subClassOf rdf:resource="http://purl.org/net/iot-dm#OWLClass_2c177064_e630_44da_bbb3_d692886a8e4a"/>
        <rdfs:comment>OMA-RD-LightweightM2M-V1_1-20180710-A, Label: LightweightM2M-BsR-008</rdfs:comment>
        <rdfs:label xml:lang="en">ObjectValueSendingMechanism</rdfs:label>
    </owl:Class>
    


    <!-- http://purl.org/net/iot-dm#OWLClass_0d737558_6941_40af_ab34_090d7a6e91b9 -->

    <owl:Class rdf:about="http://purl.org/net/iot-dm#OWLClass_0d737558_6941_40af_ab34_090d7a6e91b9">
        <rdfs:subClassOf rdf:resource="http://purl.org/net/iot-dm#OWLClass_ba85de28_3f87_455f_9993_c51b31e1a44e"/>
        <rdfs:comment>https://resin.io/features/, 2018-09-15</rdfs:comment>
        <rdfs:label xml:lang="en">DeviceImageCreation</rdfs:label>
    </owl:Class>
    


    <!-- http://purl.org/net/iot-dm#OWLClass_0effbd80_fdef_4252_ba03_50bfce2bc7ff -->

    <owl:Class rdf:about="http://purl.org/net/iot-dm#OWLClass_0effbd80_fdef_4252_ba03_50bfce2bc7ff">
        <rdfs:subClassOf rdf:resource="http://purl.org/net/iot-dm#OWLClass_84497e4c_1cfe_4d3f_b1ba_e6304c70216c"/>
        <rdfs:comment>OMA-RD-LightweightM2M-V1_1-20180710-A, Label: LightweightM2M-LPW-10</rdfs:comment>
        <rdfs:label xml:lang="en">DevAddr</rdfs:label>
    </owl:Class>
    


    <!-- http://purl.org/net/iot-dm#OWLClass_0fd00cb3_e44d_420b_bff2_9aafb1b10ace -->

    <owl:Class rdf:about="http://purl.org/net/iot-dm#OWLClass_0fd00cb3_e44d_420b_bff2_9aafb1b10ace">
        <rdfs:subClassOf rdf:resource="http://purl.org/net/iot-dm#OWLClass_ba85de28_3f87_455f_9993_c51b31e1a44e"/>
        <rdfs:comment>OMA-RD-LightweightM2M-V1_0-20170208-A, Label: LightweightM2M-HLF-023</rdfs:comment>
        <rdfs:label xml:lang="en">DeviceDiscovery</rdfs:label>
    </owl:Class>
    


    <!-- http://purl.org/net/iot-dm#OWLClass_10c7eafe_93df_425a_8e9d_870eee7b9e02 -->

    <owl:Class rdf:about="http://purl.org/net/iot-dm#OWLClass_10c7eafe_93df_425a_8e9d_870eee7b9e02">
        <rdfs:subClassOf rdf:resource="http://purl.org/net/iot-dm#OWLClass_f9db282e_22e2_48e5_a643_a42df05c880d"/>
        <rdfs:comment>IoT home gateway for auto-conﬁguration and management of MQTT devices, section I., III.</rdfs:comment>
        <rdfs:label xml:lang="en">DeviceInformationExposure</rdfs:label>
    </owl:Class>
    


    <!-- http://purl.org/net/iot-dm#OWLClass_10ff6f33_7c39_432c_9ac0_c8c9d830b8b9 -->

    <owl:Class rdf:about="http://purl.org/net/iot-dm#OWLClass_10ff6f33_7c39_432c_9ac0_c8c9d830b8b9">
        <rdfs:subClassOf rdf:resource="http://purl.org/net/iot-dm#OWLClass_4bff393a_9b00_4db5_a375_9baf63f63167"/>
        <rdfs:label xml:lang="en">PlatformControlInterface</rdfs:label>
    </owl:Class>
    


    <!-- http://purl.org/net/iot-dm#OWLClass_11ab1b8e_e60f_4b34_bd83_50a77595a516 -->

    <owl:Class rdf:about="http://purl.org/net/iot-dm#OWLClass_11ab1b8e_e60f_4b34_bd83_50a77595a516">
        <rdfs:subClassOf rdf:resource="http://purl.org/net/iot-dm#OWLClass_843d87bc_a343_470f_bff0_872b15b14c16"/>
        <rdfs:label xml:lang="en">FirmwareUpdateInitiation</rdfs:label>
    </owl:Class>
    


    <!-- http://purl.org/net/iot-dm#OWLClass_120574a4_44e7_4d45_836c_63185579c9c5 -->

    <owl:Class rdf:about="http://purl.org/net/iot-dm#OWLClass_120574a4_44e7_4d45_836c_63185579c9c5">
        <rdfs:subClassOf rdf:resource="http://purl.org/net/iot-dm#OWLClass_56ca2f5d_d065_4fe0_bfd8_9c86ea85f200"/>
        <rdfs:comment>IoT home gateway for auto-conﬁguration and management of MQTT devices, section III.</rdfs:comment>
        <rdfs:label xml:lang="en">SensorValues</rdfs:label>
    </owl:Class>
    


    <!-- http://purl.org/net/iot-dm#OWLClass_139ffd25_0d52_4625_8b15_44db26cacc9b -->

    <owl:Class rdf:about="http://purl.org/net/iot-dm#OWLClass_139ffd25_0d52_4625_8b15_44db26cacc9b">
        <rdfs:subClassOf rdf:resource="http://purl.org/net/iot-dm#OWLClass_e73ce412_848f_4de5_aadb_256be525abe9"/>
        <rdfs:comment>draft-moran-suit-architecture-03 (work in progress), p. 12</rdfs:comment>
        <rdfs:label xml:lang="en">DigitalSignatures</rdfs:label>
    </owl:Class>
    


    <!-- http://purl.org/net/iot-dm#OWLClass_13c796b1_46e2_4fc7_b2d1_299b6746d07f -->

    <owl:Class rdf:about="http://purl.org/net/iot-dm#OWLClass_13c796b1_46e2_4fc7_b2d1_299b6746d07f">
        <rdfs:subClassOf rdf:resource="http://purl.org/net/iot-dm#OWLClass_83a75814_662d_468a_bb24_dba5318a80ae"/>
        <rdfs:comment>IoT home gateway for auto-conﬁguration and management of MQTT devices, section III.</rdfs:comment>
        <rdfs:label xml:lang="en">MulticastAdvertisementMessage</rdfs:label>
    </owl:Class>
    


    <!-- http://purl.org/net/iot-dm#OWLClass_14739992_7ff1_4cb3_91a7_25d88fd84a18 -->

    <owl:Class rdf:about="http://purl.org/net/iot-dm#OWLClass_14739992_7ff1_4cb3_91a7_25d88fd84a18">
        <rdfs:subClassOf rdf:resource="http://purl.org/net/iot-dm#OWLClass_4b1504d5_8402_464c_a20c_f1c564d0ff8f"/>
        <rdfs:comment>Management of IoT Devices in a Physical Network, p. 490, 492</rdfs:comment>
        <rdfs:label xml:lang="en">AlertGeneration</rdfs:label>
    </owl:Class>
    


    <!-- http://purl.org/net/iot-dm#OWLClass_14a656e6_bf9d_4fb8_bc47_9dbb20c8c43c -->

    <owl:Class rdf:about="http://purl.org/net/iot-dm#OWLClass_14a656e6_bf9d_4fb8_bc47_9dbb20c8c43c">
        <rdfs:subClassOf rdf:resource="http://purl.org/net/iot-dm#OWLClass_66c3fc69_337f_4795_a467_f0b64b90cb3b"/>
        <rdfs:comment>Recent Advances in Industrial Wireless Sensor Networks Towards Efficient Management in IoT, p. 6, 8</rdfs:comment>
        <rdfs:label xml:lang="en">UnifiedDeviceManagement</rdfs:label>
    </owl:Class>
    


    <!-- http://purl.org/net/iot-dm#OWLClass_14f6ac55_025a_4626_934b_e27de3af1145 -->

    <owl:Class rdf:about="http://purl.org/net/iot-dm#OWLClass_14f6ac55_025a_4626_934b_e27de3af1145">
        <rdfs:subClassOf rdf:resource="http://purl.org/net/iot-dm#OWLClass_b21422b7_b049_4b16_b3e0_53d1c9d53e85"/>
        <rdfs:label xml:lang="en">DeviceTroubleshootingAndDiagnostics</rdfs:label>
    </owl:Class>
    


    <!-- http://purl.org/net/iot-dm#OWLClass_1543e022_678c_4b10_9895_de120d944f03 -->

    <owl:Class rdf:about="http://purl.org/net/iot-dm#OWLClass_1543e022_678c_4b10_9895_de120d944f03">
        <rdfs:subClassOf rdf:resource="http://purl.org/net/iot-dm#OWLClass_08385527_c024_48c2_986f_4df96714e457"/>
        <rdfs:comment>IoT home gateway for auto-conﬁguration and management of MQTT devices, section III.</rdfs:comment>
        <rdfs:label xml:lang="en">PubSubBasedInterface</rdfs:label>
    </owl:Class>
    


    <!-- http://purl.org/net/iot-dm#OWLClass_15514c90_84d5_4670_93a6_9566cb808feb -->

    <owl:Class rdf:about="http://purl.org/net/iot-dm#OWLClass_15514c90_84d5_4670_93a6_9566cb808feb">
        <rdfs:subClassOf rdf:resource="http://purl.org/net/iot-dm#OWLClass_2a645b44_80eb_49d7_8add_d5dc3d46a6f9"/>
        <rdfs:comment xml:lang="en">&quot;The firmware image is a binary that may contain the complete software of a device or a subset of it. The firmware image may consist of multiple images, if the device contains more than one microcontroller. The image may consist of a differential update for performance reasons.  Firmware is the more universal term. Both terms are used in this document and are interchangeable.&quot;, draft-moran-suit-architecture-03 (work in progress), p. 5</rdfs:comment>
        <rdfs:label xml:lang="en">FirmwareImage</rdfs:label>
    </owl:Class>
    


    <!-- http://purl.org/net/iot-dm#OWLClass_15a38f7d_ec90_4773_817a_ebd26cdadc03 -->

    <owl:Class rdf:about="http://purl.org/net/iot-dm#OWLClass_15a38f7d_ec90_4773_817a_ebd26cdadc03">
        <rdfs:subClassOf rdf:resource="http://purl.org/net/iot-dm#OWLClass_56e577ad_039f_4eeb_be83_40fd15e9c7b8"/>
        <rdfs:comment>OMA-RD-LightweightM2M-V1_1-20180710-A, Label: LightweightM2M-SCS-1</rdfs:comment>
        <rdfs:label xml:lang="en">SecureComponentReliance</rdfs:label>
    </owl:Class>
    


    <!-- http://purl.org/net/iot-dm#OWLClass_161fad8e_96a8_4a86_8d17_62ad54363b50 -->

    <owl:Class rdf:about="http://purl.org/net/iot-dm#OWLClass_161fad8e_96a8_4a86_8d17_62ad54363b50">
        <rdfs:subClassOf rdf:resource="http://purl.org/net/iot-dm#OWLClass_6f8197a0_9425_4239_bea9_7e354c8cba24"/>
        <rdfs:label xml:lang="en">FullUpdates</rdfs:label>
    </owl:Class>
    


    <!-- http://purl.org/net/iot-dm#OWLClass_169f3b27_aa22_4707_936a_088618ef2999 -->

    <owl:Class rdf:about="http://purl.org/net/iot-dm#OWLClass_169f3b27_aa22_4707_936a_088618ef2999">
        <rdfs:subClassOf rdf:resource="http://purl.org/net/iot-dm#OWLClass_b6721ba6_4ea5_4be0_b34f_ff739be47358"/>
        <rdfs:label xml:lang="en">RobustPermissionConcept</rdfs:label>
    </owl:Class>
    


    <!-- http://purl.org/net/iot-dm#OWLClass_16cd1e7c_b16e_4612_98eb_8935ff2fe30b -->

    <owl:Class rdf:about="http://purl.org/net/iot-dm#OWLClass_16cd1e7c_b16e_4612_98eb_8935ff2fe30b">
        <rdfs:subClassOf rdf:resource="http://purl.org/net/iot-dm#OWLClass_1d7dd666_95ba_4c41_9a91_d850e9c0f479"/>
        <rdfs:comment>Recent Advances in Industrial Wireless Sensor Networks Towards Efficient Management in IoT, p. 6</rdfs:comment>
        <rdfs:label xml:lang="en">NetworkUsageEfficiency</rdfs:label>
    </owl:Class>
    


    <!-- http://purl.org/net/iot-dm#OWLClass_1725b847_7dbe_46b0_aa1f_3a6c6bdc236f -->

    <owl:Class rdf:about="http://purl.org/net/iot-dm#OWLClass_1725b847_7dbe_46b0_aa1f_3a6c6bdc236f">
        <rdfs:subClassOf rdf:resource="http://purl.org/net/iot-dm#OWLClass_14f6ac55_025a_4626_934b_e27de3af1145"/>
        <rdfs:comment>Recent Advances in Industrial Wireless Sensor Networks Towards Efficient Management in IoT, p. 9</rdfs:comment>
        <rdfs:label xml:lang="en">ConnectionDiagnostics</rdfs:label>
    </owl:Class>
    


    <!-- http://purl.org/net/iot-dm#OWLClass_18471212_0dca_43c7_807a_1e3346b35c76 -->

    <owl:Class rdf:about="http://purl.org/net/iot-dm#OWLClass_18471212_0dca_43c7_807a_1e3346b35c76">
        <rdfs:subClassOf rdf:resource="http://purl.org/net/iot-dm#OWLClass_dd21fadb_8dfb_46e9_a311_b39ddefaad69"/>
        <rdfs:comment>OMA-RD-LightweightM2M-V1_0-20170208-A, Label: LightweightM2M-HLF-026</rdfs:comment>
        <rdfs:label xml:lang="en">DeviceConnectivityStatus</rdfs:label>
    </owl:Class>
    


    <!-- http://purl.org/net/iot-dm#OWLClass_195de59b_34c2_45da_8aa8_591cd3847fc7 -->

    <owl:Class rdf:about="http://purl.org/net/iot-dm#OWLClass_195de59b_34c2_45da_8aa8_591cd3847fc7">
        <rdfs:subClassOf rdf:resource="http://purl.org/net/iot-dm#OWLClass_e7e81967_1b1b_4dfb_b9b6_c40e0ffab441"/>
        <rdfs:comment>OMA-RD-LightweightM2M-V1_1-20180710-A, section 6.1.3.4</rdfs:comment>
        <rdfs:comment>OMA-RD-LightweightM2M-V1_1-20180710-A, section 6.1.3.5</rdfs:comment>
        <rdfs:label xml:lang="en">EndToEndSecuritySolution</rdfs:label>
    </owl:Class>
    


    <!-- http://purl.org/net/iot-dm#OWLClass_1af506a2_819c_4a9b_946d_e113aa62e310 -->

    <owl:Class rdf:about="http://purl.org/net/iot-dm#OWLClass_1af506a2_819c_4a9b_946d_e113aa62e310">
        <rdfs:subClassOf rdf:resource="http://purl.org/net/iot-dm#OWLClass_f4a64f37_cafb_440d_8e03_c1895c63f6ea"/>
        <rdfs:comment>Management of IoT Devices in a Physical Network, p. 487</rdfs:comment>
        <rdfs:label xml:lang="en">VisualizationOfDeviceNetwork</rdfs:label>
    </owl:Class>
    


    <!-- http://purl.org/net/iot-dm#OWLClass_1b1c6eb8_b3e5_458b_9129_f0f558a09b74 -->

    <owl:Class rdf:about="http://purl.org/net/iot-dm#OWLClass_1b1c6eb8_b3e5_458b_9129_f0f558a09b74">
        <rdfs:subClassOf rdf:resource="http://purl.org/net/iot-dm#OWLClass_d5baf8ff_3ca0_40a1_988a_a5e23a144824"/>
        <rdfs:comment>OMA-RD-LightweightM2M-V1_0-20170208-A, Label: LightweightM2M-HLF-036</rdfs:comment>
        <rdfs:label xml:lang="en">MessageDeliveryAcknowledgement</rdfs:label>
    </owl:Class>
    


    <!-- http://purl.org/net/iot-dm#OWLClass_1bd19af8_5e90_482f_b798_79ba7cc8d671 -->

    <owl:Class rdf:about="http://purl.org/net/iot-dm#OWLClass_1bd19af8_5e90_482f_b798_79ba7cc8d671">
        <rdfs:subClassOf rdf:resource="http://purl.org/net/iot-dm#OWLClass_ebbfff77_6bbb_477e_9f30_934e7239601e"/>
        <rdfs:label xml:lang="en">ApplicationPlatform</rdfs:label>
    </owl:Class>
    


    <!-- http://purl.org/net/iot-dm#OWLClass_1c94fa2c_ae83_478d_af9c_a4454dc491c3 -->

    <owl:Class rdf:about="http://purl.org/net/iot-dm#OWLClass_1c94fa2c_ae83_478d_af9c_a4454dc491c3">
        <rdfs:subClassOf rdf:resource="http://purl.org/net/iot-dm#OWLClass_ec9156ee_5023_4804_9c7c_19a9a4ad18b4"/>
        <rdfs:comment>Recent Advances in Industrial Wireless Sensor Networks Towards Efficient Management in IoT, p. 10</rdfs:comment>
        <rdfs:label xml:lang="en">RetransmissionStrategy</rdfs:label>
    </owl:Class>
    


    <!-- http://purl.org/net/iot-dm#OWLClass_1caeb79a_fc8a_4690_b3eb_f48f079dfb85 -->

    <owl:Class rdf:about="http://purl.org/net/iot-dm#OWLClass_1caeb79a_fc8a_4690_b3eb_f48f079dfb85">
        <rdfs:subClassOf rdf:resource="http://purl.org/net/iot-dm#OWLClass_56ebbdf9_64f2_4b0c_acdb_20694cd96f8c"/>
        <rdfs:comment>OMA-RD-LightweightM2M-V1_1-20180710-A, Label: LightweightM2M-LeG-006</rdfs:comment>
        <rdfs:label xml:lang="en">UsedSecurityMechanismsBetweenDeviceAndGateway</rdfs:label>
    </owl:Class>
    


    <!-- http://purl.org/net/iot-dm#OWLClass_1d708038_ca44_4723_a910_a811401f688c -->

    <owl:Class rdf:about="http://purl.org/net/iot-dm#OWLClass_1d708038_ca44_4723_a910_a811401f688c">
        <rdfs:subClassOf rdf:resource="http://purl.org/net/iot-dm#OWLClass_cdca4605_0981_47f3_be76_554636de1e00"/>
        <rdfs:label xml:lang="en">FirmwareDeliveryMessage</rdfs:label>
    </owl:Class>
    


    <!-- http://purl.org/net/iot-dm#OWLClass_1d7dd666_95ba_4c41_9a91_d850e9c0f479 -->

    <owl:Class rdf:about="http://purl.org/net/iot-dm#OWLClass_1d7dd666_95ba_4c41_9a91_d850e9c0f479">
        <rdfs:subClassOf rdf:resource="http://purl.org/net/iot-dm#OWLClass_ffcb0dd3_5746_4e9b_9905_50bfb9faff34"/>
        <rdfs:comment>Recent Advances in Industrial Wireless Sensor Networks Towards Efficient Management in IoT, p. 6</rdfs:comment>
        <rdfs:label xml:lang="en">EfficientCommunication</rdfs:label>
    </owl:Class>
    


    <!-- http://purl.org/net/iot-dm#OWLClass_1d879b7b_ee0d_44b9_90e4_047da18bb445 -->

    <owl:Class rdf:about="http://purl.org/net/iot-dm#OWLClass_1d879b7b_ee0d_44b9_90e4_047da18bb445">
        <rdfs:subClassOf rdf:resource="http://purl.org/net/iot-dm#OWLClass_c8340585_9c41_4f98_8f90_b4e2436e8829"/>
        <rdfs:comment>OMA-RD-LightweightM2M-V1_1-20180710-A, Label: LightweightM2M-LPW-5</rdfs:comment>
        <rdfs:label xml:lang="en">MessageTimeToLive</rdfs:label>
    </owl:Class>
    


    <!-- http://purl.org/net/iot-dm#OWLClass_201d2207_e63c_4bd0_ac8e_dac6fd8b7d61 -->

    <owl:Class rdf:about="http://purl.org/net/iot-dm#OWLClass_201d2207_e63c_4bd0_ac8e_dac6fd8b7d61">
        <rdfs:subClassOf rdf:resource="http://purl.org/net/iot-dm#OWLClass_b21422b7_b049_4b16_b3e0_53d1c9d53e85"/>
        <rdfs:label xml:lang="en">DeviceSoftwareManagement</rdfs:label>
    </owl:Class>
    


    <!-- http://purl.org/net/iot-dm#OWLClass_204fbe41_1ddf_476c_ad8a_1d0161ca1d40 -->

    <owl:Class rdf:about="http://purl.org/net/iot-dm#OWLClass_204fbe41_1ddf_476c_ad8a_1d0161ca1d40">
        <rdfs:subClassOf rdf:resource="http://purl.org/net/iot-dm#OWLClass_3e781bea_1637_4984_bf63_8935b4e49e16"/>
        <rdfs:comment>OMA-RD-LightweightM2M-V1_0-20170208-A, Label: LightweightM2M-HLF-024</rdfs:comment>
        <rdfs:label xml:lang="en">ThresholdBasedReportingMechanism</rdfs:label>
    </owl:Class>
    


    <!-- http://purl.org/net/iot-dm#OWLClass_20ed2639_e6b8_4144_8ec9_34ce2a2a9f15 -->

    <owl:Class rdf:about="http://purl.org/net/iot-dm#OWLClass_20ed2639_e6b8_4144_8ec9_34ce2a2a9f15">
        <rdfs:subClassOf rdf:resource="http://purl.org/net/iot-dm#OWLClass_35675b83_774d_4402_9ce1_6b0bc13b514f"/>
        <rdfs:comment>Ontologies for the Internet of Things, 1.</rdfs:comment>
        <rdfs:comment>Permanently or temporarily</rdfs:comment>
        <rdfs:label xml:lang="en">LeftDevices</rdfs:label>
    </owl:Class>
    


    <!-- http://purl.org/net/iot-dm#OWLClass_213b255b_d2a6_41ac_9e58_75311a7288f3 -->

    <owl:Class rdf:about="http://purl.org/net/iot-dm#OWLClass_213b255b_d2a6_41ac_9e58_75311a7288f3">
        <rdfs:subClassOf rdf:resource="http://purl.org/net/iot-dm#OWLClass_36c8fbfb_7218_4373_a13b_f46a86f007be"/>
        <rdfs:comment>Management of IoT Devices in a Physical Network, p. 486</rdfs:comment>
        <rdfs:label xml:lang="en">InherentDeviceCharacteristics</rdfs:label>
    </owl:Class>
    


    <!-- http://purl.org/net/iot-dm#OWLClass_21fa4e78_3300_43d8_83c7_78d9ee314b79 -->

    <owl:Class rdf:about="http://purl.org/net/iot-dm#OWLClass_21fa4e78_3300_43d8_83c7_78d9ee314b79">
        <rdfs:subClassOf rdf:resource="http://purl.org/net/iot-dm#OWLClass_f6444fa6_1240_4dfa_9bba_affd175076ca"/>
        <rdfs:label xml:lang="en">ReportedObservations</rdfs:label>
    </owl:Class>
    


    <!-- http://purl.org/net/iot-dm#OWLClass_2281b85a_ace5_4ac3_910f_536f7370505e -->

    <owl:Class rdf:about="http://purl.org/net/iot-dm#OWLClass_2281b85a_ace5_4ac3_910f_536f7370505e">
        <rdfs:subClassOf rdf:resource="http://purl.org/net/iot-dm#OWLClass_b21422b7_b049_4b16_b3e0_53d1c9d53e85"/>
        <rdfs:label xml:lang="en">DeviceControl</rdfs:label>
    </owl:Class>
    


    <!-- http://purl.org/net/iot-dm#OWLClass_228f4585_63dc_41a1_8a68_b3cf514d174d -->

    <owl:Class rdf:about="http://purl.org/net/iot-dm#OWLClass_228f4585_63dc_41a1_8a68_b3cf514d174d">
        <rdfs:subClassOf rdf:resource="http://purl.org/net/iot-dm#OWLClass_21fa4e78_3300_43d8_83c7_78d9ee314b79"/>
        <rdfs:comment>OMA-RD-LightweightM2M-V1_0-20170208-A, Label: LightweightM2M-HLF-025</rdfs:comment>
        <rdfs:label xml:lang="en">RadioSignalStrength</rdfs:label>
    </owl:Class>
    


    <!-- http://purl.org/net/iot-dm#OWLClass_22b2bdaa_bda4_4b5e_b89c_45b9385203f7 -->

    <owl:Class rdf:about="http://purl.org/net/iot-dm#OWLClass_22b2bdaa_bda4_4b5e_b89c_45b9385203f7">
        <rdfs:subClassOf rdf:resource="http://purl.org/net/iot-dm#OWLClass_213b255b_d2a6_41ac_9e58_75311a7288f3"/>
        <rdfs:comment>Management of IoT Devices in a Physical Network, p. 488</rdfs:comment>
        <rdfs:label xml:lang="en">DeviceEvents</rdfs:label>
    </owl:Class>
    


    <!-- http://purl.org/net/iot-dm#OWLClass_24b7c457_4c59_45bd_8e3d_430ad08d9863 -->

    <owl:Class rdf:about="http://purl.org/net/iot-dm#OWLClass_24b7c457_4c59_45bd_8e3d_430ad08d9863">
        <rdfs:subClassOf rdf:resource="http://purl.org/net/iot-dm#OWLClass_a9fa280a_8537_4626_a942_bab8a45552c7"/>
        <rdfs:comment>Management of IoT Devices in a Physical Network, p. 490</rdfs:comment>
        <rdfs:label xml:lang="en">TimerEvent</rdfs:label>
    </owl:Class>
    


    <!-- http://purl.org/net/iot-dm#OWLClass_2546b23c_c54a_478f_8b94_7aaebcfce295 -->

    <owl:Class rdf:about="http://purl.org/net/iot-dm#OWLClass_2546b23c_c54a_478f_8b94_7aaebcfce295">
        <rdfs:subClassOf rdf:resource="http://purl.org/net/iot-dm#OWLClass_14739992_7ff1_4cb3_91a7_25d88fd84a18"/>
        <rdfs:comment>OMA-RD-LightweightM2M-V1_0-20170208-A, Label: LightweightM2M-HLF-007</rdfs:comment>
        <rdfs:label xml:lang="en">DeviceErrorReporting</rdfs:label>
    </owl:Class>
    


    <!-- http://purl.org/net/iot-dm#OWLClass_2652aa9f_1a74_458a_9d93_7a48ced1f273 -->

    <owl:Class rdf:about="http://purl.org/net/iot-dm#OWLClass_2652aa9f_1a74_458a_9d93_7a48ced1f273">
        <rdfs:subClassOf rdf:resource="http://purl.org/net/iot-dm#OWLClass_e00944d4_c070_4cf7_91ed_7f4c58ff50c8"/>
        <rdfs:label xml:lang="en">RetryBackOffTimers</rdfs:label>
        <rdfs:seeAlso>OMA-RD-LightweightM2M-V1_1-20180710-A, Label: LightweightM2M-BsR-004</rdfs:seeAlso>
    </owl:Class>
    


    <!-- http://purl.org/net/iot-dm#OWLClass_267278cd_85b2_4704_84d7_a7cb4004d16d -->

    <owl:Class rdf:about="http://purl.org/net/iot-dm#OWLClass_267278cd_85b2_4704_84d7_a7cb4004d16d">
        <rdfs:subClassOf rdf:resource="http://purl.org/net/iot-dm#OWLClass_201d2207_e63c_4bd0_ac8e_dac6fd8b7d61"/>
        <rdfs:label xml:lang="en">ApplicationManagment</rdfs:label>
    </owl:Class>
    


    <!-- http://purl.org/net/iot-dm#OWLClass_26b07b8c_41ba_49a3_9bea_08a9db2affeb -->

    <owl:Class rdf:about="http://purl.org/net/iot-dm#OWLClass_26b07b8c_41ba_49a3_9bea_08a9db2affeb">
        <rdfs:subClassOf rdf:resource="http://purl.org/net/iot-dm#OWLClass_774c7acb_c17d_4e26_8afc_75f16a0910c5"/>
        <rdfs:comment>https://resin.io/how-it-works/, 2019-09-16</rdfs:comment>
        <rdfs:label xml:lang="en">LogsByServiceFilter</rdfs:label>
    </owl:Class>
    


    <!-- http://purl.org/net/iot-dm#OWLClass_26b89687_0b06_4e3f_bb15_6cd4b670a9f4 -->

    <owl:Class rdf:about="http://purl.org/net/iot-dm#OWLClass_26b89687_0b06_4e3f_bb15_6cd4b670a9f4">
        <rdfs:subClassOf rdf:resource="http://purl.org/net/iot-dm#OWLClass_83a75814_662d_468a_bb24_dba5318a80ae"/>
        <rdfs:comment>IoT home gateway for auto-conﬁguration and management of MQTT devices, section III.</rdfs:comment>
        <rdfs:label xml:lang="en">JsonBasedAutoConfigurationMessage</rdfs:label>
    </owl:Class>
    


    <!-- http://purl.org/net/iot-dm#OWLClass_26e4e96a_53e5_4caf_8b2c_6e8ba96479ff -->

    <owl:Class rdf:about="http://purl.org/net/iot-dm#OWLClass_26e4e96a_53e5_4caf_8b2c_6e8ba96479ff">
        <rdfs:subClassOf rdf:resource="http://purl.org/net/iot-dm#OWLClass_829a4147_2a1d_44ea_a9ef_0efaae5eaa5b"/>
        <rdfs:comment>https://resin.io/features/, 2018-09-15</rdfs:comment>
        <rdfs:label xml:lang="en">OdataApi</rdfs:label>
    </owl:Class>
    


    <!-- http://purl.org/net/iot-dm#OWLClass_273d6557_6465_43c6_b4fc_9121cf33d0df -->

    <owl:Class rdf:about="http://purl.org/net/iot-dm#OWLClass_273d6557_6465_43c6_b4fc_9121cf33d0df">
        <rdfs:subClassOf rdf:resource="http://purl.org/net/iot-dm#OWLClass_a18f091d_134e_4059_ada6_9695459aa5f6"/>
        <rdfs:comment>https://resin.io/how-it-works/, 2019-09-16</rdfs:comment>
        <rdfs:label xml:lang="en">Vpn</rdfs:label>
    </owl:Class>
    


    <!-- http://purl.org/net/iot-dm#OWLClass_28082eb5_3e38_41bb_ba51_c4224fe7fdce -->

    <owl:Class rdf:about="http://purl.org/net/iot-dm#OWLClass_28082eb5_3e38_41bb_ba51_c4224fe7fdce">
        <rdfs:subClassOf rdf:resource="http://purl.org/net/iot-dm#OWLClass_348de6b7_7669_4563_ae9b_3b4a7ec8b87f"/>
        <rdfs:label xml:lang="en">PhysicalStatisticalEstimationModels</rdfs:label>
    </owl:Class>
    


    <!-- http://purl.org/net/iot-dm#OWLClass_28fc1a1f_0fa1_4ebe_9d96_c82659208f33 -->

    <owl:Class rdf:about="http://purl.org/net/iot-dm#OWLClass_28fc1a1f_0fa1_4ebe_9d96_c82659208f33">
        <rdfs:subClassOf rdf:resource="http://purl.org/net/iot-dm#OWLClass_84497e4c_1cfe_4d3f_b1ba_e6304c70216c"/>
        <rdfs:comment>OMA-RD-LightweightM2M-V1_1-20180710-A, Label: LightweightM2M-LPW-10</rdfs:comment>
        <rdfs:label xml:lang="en">NwkSKey</rdfs:label>
    </owl:Class>
    


    <!-- http://purl.org/net/iot-dm#OWLClass_29d80687_8df7_4e30_8f2b_05f9b2317021 -->

    <owl:Class rdf:about="http://purl.org/net/iot-dm#OWLClass_29d80687_8df7_4e30_8f2b_05f9b2317021">
        <rdfs:subClassOf rdf:resource="http://purl.org/net/iot-dm#OWLClass_38e18d87_aade_4d8b_ab6e_1da467276a13"/>
        <rdfs:comment>Management of IoT Devices in a Physical Network, p. 488</rdfs:comment>
        <rdfs:label xml:lang="en">Brand</rdfs:label>
    </owl:Class>
    


    <!-- http://purl.org/net/iot-dm#OWLClass_2a645b44_80eb_49d7_8add_d5dc3d46a6f9 -->

    <owl:Class rdf:about="http://purl.org/net/iot-dm#OWLClass_2a645b44_80eb_49d7_8add_d5dc3d46a6f9">
        <rdfs:label xml:lang="en">Firmware</rdfs:label>
    </owl:Class>
    


    <!-- http://purl.org/net/iot-dm#OWLClass_2b77c491_438d_4176_bfc8_1ca1e94c8b12 -->

    <owl:Class rdf:about="http://purl.org/net/iot-dm#OWLClass_2b77c491_438d_4176_bfc8_1ca1e94c8b12">
        <rdfs:subClassOf rdf:resource="http://purl.org/net/iot-dm#OWLClass_6cb818a3_6278_4bad_8a6b_c01ee623c677"/>
        <rdfs:comment>OMA-RD-LightweightM2M-V1_0-20170208-A, Label: LightweightM2M-HLF-008</rdfs:comment>
        <rdfs:label xml:lang="en">DeviceRestart</rdfs:label>
    </owl:Class>
    


    <!-- http://purl.org/net/iot-dm#OWLClass_2c177064_e630_44da_bbb3_d692886a8e4a -->

    <owl:Class rdf:about="http://purl.org/net/iot-dm#OWLClass_2c177064_e630_44da_bbb3_d692886a8e4a">
        <rdfs:subClassOf rdf:resource="http://purl.org/net/iot-dm#OWLClass_f4c68c89_a4ee_4e3f_b527_9a88d50887fe"/>
        <rdfs:label xml:lang="en">Bootstrapping</rdfs:label>
    </owl:Class>
    


    <!-- http://purl.org/net/iot-dm#OWLClass_2d519c83_8e6a_4b5e_829b_640913743110 -->

    <owl:Class rdf:about="http://purl.org/net/iot-dm#OWLClass_2d519c83_8e6a_4b5e_829b_640913743110">
        <rdfs:subClassOf rdf:resource="http://purl.org/net/iot-dm#OWLClass_86628aec_b662_41c9_ae13_eec3bc59261a"/>
        <rdfs:comment>https://resin.io/how-it-works/, 2019-09-16</rdfs:comment>
        <rdfs:label xml:lang="en">NodejsSdk</rdfs:label>
    </owl:Class>
    


    <!-- http://purl.org/net/iot-dm#OWLClass_2d9c2b5f_16f1_4947_b01d_6f7578a2c079 -->

    <owl:Class rdf:about="http://purl.org/net/iot-dm#OWLClass_2d9c2b5f_16f1_4947_b01d_6f7578a2c079">
        <rdfs:subClassOf rdf:resource="http://purl.org/net/iot-dm#OWLClass_8420db7e_6cbf_4959_ac1b_39fdae9da0b3"/>
        <rdfs:label xml:lang="en">AccessMethod</rdfs:label>
    </owl:Class>
    


    <!-- http://purl.org/net/iot-dm#OWLClass_2e990825_4f19_4397_8ccb_fe14344dd987 -->

    <owl:Class rdf:about="http://purl.org/net/iot-dm#OWLClass_2e990825_4f19_4397_8ccb_fe14344dd987">
        <rdfs:subClassOf rdf:resource="http://purl.org/net/iot-dm#OWLClass_35675b83_774d_4402_9ce1_6b0bc13b514f"/>
        <rdfs:comment>Ontologies for the Internet of Things, 1.</rdfs:comment>
        <rdfs:label xml:lang="en">NonExistingDevices</rdfs:label>
    </owl:Class>
    


    <!-- http://purl.org/net/iot-dm#OWLClass_2ee3c907_2ad6_45fc_999f_299667c29188 -->

    <owl:Class rdf:about="http://purl.org/net/iot-dm#OWLClass_2ee3c907_2ad6_45fc_999f_299667c29188">
        <rdfs:subClassOf rdf:resource="http://purl.org/net/iot-dm#OWLClass_3300e6af_4338_4bf4_ab9e_632af0b5ad65"/>
        <rdfs:comment>Management of IoT Devices in a Physical Network, p. 488</rdfs:comment>
        <rdfs:comment>Recent Advances in Industrial Wireless Sensor Networks Towards Efficient Management in IoT, p. 8</rdfs:comment>
        <rdfs:label xml:lang="en">DeviceInformationMaintenance</rdfs:label>
    </owl:Class>
    


    <!-- http://purl.org/net/iot-dm#OWLClass_2fb332cc_9b13_4fbc_af07_4ce1a662e062 -->

    <owl:Class rdf:about="http://purl.org/net/iot-dm#OWLClass_2fb332cc_9b13_4fbc_af07_4ce1a662e062">
        <rdfs:subClassOf rdf:resource="http://purl.org/net/iot-dm#OWLClass_cbca8db6_d106_4651_a12c_b8fe629efbda"/>
        <rdfs:label xml:lang="en">DeviceInformationRetrieval</rdfs:label>
    </owl:Class>
    


    <!-- http://purl.org/net/iot-dm#OWLClass_3021d060_11f7_4192_b341_d89fc03bb8f1 -->

    <owl:Class rdf:about="http://purl.org/net/iot-dm#OWLClass_3021d060_11f7_4192_b341_d89fc03bb8f1">
        <rdfs:subClassOf rdf:resource="http://purl.org/net/iot-dm#OWLClass_defe9266_4e6d_4036_8134_4ad7f7a4797e"/>
        <rdfs:comment>OMA-RD-LightweightM2M-V1_1-20180710-A, Label: LightweightM2M-DSE-001</rdfs:comment>
        <rdfs:label xml:lang="en">TargetListOfDistributedResourcesUsingSingleOperation</rdfs:label>
    </owl:Class>
    


    <!-- http://purl.org/net/iot-dm#OWLClass_308975a3_5765_4401_95ac_7d1b99100408 -->

    <owl:Class rdf:about="http://purl.org/net/iot-dm#OWLClass_308975a3_5765_4401_95ac_7d1b99100408">
        <rdfs:subClassOf rdf:resource="http://purl.org/net/iot-dm#OWLClass_e7e81967_1b1b_4dfb_b9b6_c40e0ffab441"/>
        <rdfs:comment>OMA-RD-LightweightM2M-V1_0-20170208-A, Label: LightweightM2M-SEC-001</rdfs:comment>
        <rdfs:label xml:lang="en">SecureClientServerCommunication</rdfs:label>
    </owl:Class>
    


    <!-- http://purl.org/net/iot-dm#OWLClass_30d8bc8b_4188_4a4f_be58_c4d70f00474e -->

    <owl:Class rdf:about="http://purl.org/net/iot-dm#OWLClass_30d8bc8b_4188_4a4f_be58_c4d70f00474e">
        <rdfs:subClassOf rdf:resource="http://purl.org/net/iot-dm#OWLClass_9e3d4f19_96c7_4932_a007_26fa592f3423"/>
        <rdfs:comment>https://resin.io/how-it-works/, 2018-09-16</rdfs:comment>
        <rdfs:comment>https://www.balena.io/, 2018-09-16</rdfs:comment>
        <rdfs:label xml:lang="en">ContainerEngine</rdfs:label>
    </owl:Class>
    


    <!-- http://purl.org/net/iot-dm#OWLClass_30ea11de_95fd_46c4_a0cb_bcb17dcf6830 -->

    <owl:Class rdf:about="http://purl.org/net/iot-dm#OWLClass_30ea11de_95fd_46c4_a0cb_bcb17dcf6830">
        <rdfs:subClassOf rdf:resource="http://purl.org/net/iot-dm#OWLClass_5985dbe5_dc91_4677_a070_127370474bb9"/>
        <rdfs:comment>Recent Advances in Industrial Wireless Sensor Networks Towards Efficient Management in IoT, p. 1</rdfs:comment>
        <rdfs:label xml:lang="en">NetworkParameters</rdfs:label>
    </owl:Class>
    


    <!-- http://purl.org/net/iot-dm#OWLClass_310d0972_dbed_4baf_8618_2246810e7489 -->

    <owl:Class rdf:about="http://purl.org/net/iot-dm#OWLClass_310d0972_dbed_4baf_8618_2246810e7489">
        <rdfs:subClassOf rdf:resource="http://purl.org/net/iot-dm#OWLClass_195de59b_34c2_45da_8aa8_591cd3847fc7"/>
        <rdfs:comment>OMA-RD-LightweightM2M-V1_1-20180710-A, Label: LightweightM2M-E2E-11</rdfs:comment>
        <rdfs:comment>OMA-RD-LightweightM2M-V1_1-20180710-A, Label: LightweightM2M-E2E-5</rdfs:comment>
        <rdfs:comment>OMA-RD-LightweightM2M-V1_1-20180710-A, Label: LightweightM2M-E2Eo-11</rdfs:comment>
        <rdfs:comment>OMA-RD-LightweightM2M-V1_1-20180710-A, Label: LightweightM2M-E2Eo-5</rdfs:comment>
        <rdfs:label xml:lang="en">SecureRequestResponseBinding</rdfs:label>
    </owl:Class>
    


    <!-- http://purl.org/net/iot-dm#OWLClass_32d5b16a_ce18_4cf3_9f00_3b392ba579df -->

    <owl:Class rdf:about="http://purl.org/net/iot-dm#OWLClass_32d5b16a_ce18_4cf3_9f00_3b392ba579df">
        <rdfs:subClassOf rdf:resource="http://purl.org/net/iot-dm#OWLClass_4c92b333_17aa_4b39_86cb_89b4a5083d67"/>
        <rdfs:comment>OMA-RD-LightweightM2M-V1_0-20170208-A, Label: LightweightM2M-HLF-002</rdfs:comment>
        <rdfs:label xml:lang="en">BinaryDeviceAddress</rdfs:label>
    </owl:Class>
    


    <!-- http://purl.org/net/iot-dm#OWLClass_3300e6af_4338_4bf4_ab9e_632af0b5ad65 -->

    <owl:Class rdf:about="http://purl.org/net/iot-dm#OWLClass_3300e6af_4338_4bf4_ab9e_632af0b5ad65">
        <rdfs:subClassOf rdf:resource="http://purl.org/net/iot-dm#OWLClass_ba85de28_3f87_455f_9993_c51b31e1a44e"/>
        <rdfs:comment>OMA-RD-LightweightM2M-V1_0-20170208-A, Label: LightweightM2M-HLF-023</rdfs:comment>
        <rdfs:comment>Recent Advances in Industrial Wireless Sensor Networks Towards Efficient Management in IoT, p. 8</rdfs:comment>
        <rdfs:label xml:lang="en">VirtualDeviceInstanceRegistration</rdfs:label>
        <rdfs:seeAlso>Bootstrapping</rdfs:seeAlso>
        <rdfs:seeAlso>VirtualDeviceInstanceCreation</rdfs:seeAlso>
    </owl:Class>
    


    <!-- http://purl.org/net/iot-dm#OWLClass_33b97d68_aad6_46b8_976a_88dc9e3d2ae5 -->

    <owl:Class rdf:about="http://purl.org/net/iot-dm#OWLClass_33b97d68_aad6_46b8_976a_88dc9e3d2ae5">
        <rdfs:subClassOf rdf:resource="http://purl.org/net/iot-dm#OWLClass_38e18d87_aade_4d8b_ab6e_1da467276a13"/>
        <rdfs:comment>Management of IoT Devices in a Physical Network, p. 488</rdfs:comment>
        <rdfs:label xml:lang="en">Model</rdfs:label>
    </owl:Class>
    


    <!-- http://purl.org/net/iot-dm#OWLClass_348de6b7_7669_4563_ae9b_3b4a7ec8b87f -->

    <owl:Class rdf:about="http://purl.org/net/iot-dm#OWLClass_348de6b7_7669_4563_ae9b_3b4a7ec8b87f">
        <rdfs:subClassOf rdf:resource="http://purl.org/net/iot-dm#OWLClass_7b141ed0_5648_4402_8f34_8078c00b8ee7"/>
        <rdfs:comment>Ontologies for the Internet of Things, 2.</rdfs:comment>
        <rdfs:label xml:lang="en">EstimationModels</rdfs:label>
    </owl:Class>
    


    <!-- http://purl.org/net/iot-dm#OWLClass_35227df9_2a26_4bf1_ae48_32e3c50a341c -->

    <owl:Class rdf:about="http://purl.org/net/iot-dm#OWLClass_35227df9_2a26_4bf1_ae48_32e3c50a341c">
        <rdfs:subClassOf rdf:resource="http://purl.org/net/iot-dm#OWLClass_a18f091d_134e_4059_ada6_9695459aa5f6"/>
        <rdfs:comment>Recent Advances in Industrial Wireless Sensor Networks Towards Efficient Management in IoT, p. 7</rdfs:comment>
        <rdfs:label xml:lang="en">CommandLineInterface</rdfs:label>
        <rdfs:seeAlso>DeviceTerminal</rdfs:seeAlso>
    </owl:Class>
    


    <!-- http://purl.org/net/iot-dm#OWLClass_354f3545_3c42_493b_a984_cbbfa168c104 -->

    <owl:Class rdf:about="http://purl.org/net/iot-dm#OWLClass_354f3545_3c42_493b_a984_cbbfa168c104">
        <rdfs:subClassOf rdf:resource="http://purl.org/net/iot-dm#OWLClass_574c5366_c20d_467b_8ad6_787581d5f349"/>
        <rdfs:comment>IoT home gateway for auto-conﬁguration and management of MQTT devices, section III.</rdfs:comment>
        <rdfs:label xml:lang="en">IpBased</rdfs:label>
    </owl:Class>
    


    <!-- http://purl.org/net/iot-dm#OWLClass_3555e29b_882f_473a_8681_d6c1ae2c474a -->

    <owl:Class rdf:about="http://purl.org/net/iot-dm#OWLClass_3555e29b_882f_473a_8681_d6c1ae2c474a">
        <rdfs:subClassOf rdf:resource="http://purl.org/net/iot-dm#OWLClass_11ab1b8e_e60f_4b34_bd83_50a77595a516"/>
        <rdfs:comment xml:lang="en">draft-moran-suit-architecture-03 (work in progress), p. 9</rdfs:comment>
        <rdfs:label xml:lang="en">PushToDevice</rdfs:label>
    </owl:Class>
    


    <!-- http://purl.org/net/iot-dm#OWLClass_35675b83_774d_4402_9ce1_6b0bc13b514f -->

    <owl:Class rdf:about="http://purl.org/net/iot-dm#OWLClass_35675b83_774d_4402_9ce1_6b0bc13b514f">
        <rdfs:subClassOf rdf:resource="http://purl.org/net/iot-dm#OWLClass_5236ab9a_e39c_4e90_b265_63064ec80b33"/>
        <rdfs:comment>Ontologies for the Internet of Things, 1.</rdfs:comment>
        <rdfs:label xml:lang="en">MissingDeviceHandling</rdfs:label>
    </owl:Class>
    


    <!-- http://purl.org/net/iot-dm#OWLClass_36aae163_04b8_4f81_a497_d51a026e43cd -->

    <owl:Class rdf:about="http://purl.org/net/iot-dm#OWLClass_36aae163_04b8_4f81_a497_d51a026e43cd">
        <rdfs:subClassOf rdf:resource="http://purl.org/net/iot-dm#OWLClass_ffcb0dd3_5746_4e9b_9905_50bfb9faff34"/>
        <rdfs:comment>OMA-RD-LightweightM2M-V1_0-20170208-A, Label: LightweightM2M-HLF-017</rdfs:comment>
        <rdfs:label xml:lang="en">SessionlessCommunication</rdfs:label>
    </owl:Class>
    


    <!-- http://purl.org/net/iot-dm#OWLClass_36c8fbfb_7218_4373_a13b_f46a86f007be -->

    <owl:Class rdf:about="http://purl.org/net/iot-dm#OWLClass_36c8fbfb_7218_4373_a13b_f46a86f007be">
        <rdfs:subClassOf rdf:resource="http://purl.org/net/iot-dm#OWLClass_f4a64f37_cafb_440d_8e03_c1895c63f6ea"/>
        <rdfs:comment>Management of IoT Devices in a Physical Network, p. 488</rdfs:comment>
        <rdfs:label xml:lang="en">VirtualDeviceInstance</rdfs:label>
    </owl:Class>
    


    <!-- http://purl.org/net/iot-dm#OWLClass_377a1133_d579_4dc6_a9b2_f30dfcb313e2 -->

    <owl:Class rdf:about="http://purl.org/net/iot-dm#OWLClass_377a1133_d579_4dc6_a9b2_f30dfcb313e2">
        <rdfs:subClassOf rdf:resource="http://purl.org/net/iot-dm#OWLClass_506a07f5_4566_41a4_84ac_ea621caa87b7"/>
        <rdfs:comment>https://resin.io/features/, 2018-09-15</rdfs:comment>
        <rdfs:label xml:lang="en">CommandLineInterface</rdfs:label>
    </owl:Class>
    


    <!-- http://purl.org/net/iot-dm#OWLClass_3787149f_55e1_4abd_84be_f329cca80a26 -->

    <owl:Class rdf:about="http://purl.org/net/iot-dm#OWLClass_3787149f_55e1_4abd_84be_f329cca80a26">
        <rdfs:subClassOf rdf:resource="http://purl.org/net/iot-dm#OWLClass_3300e6af_4338_4bf4_ab9e_632af0b5ad65"/>
        <rdfs:comment>https://resin.io/features/, 2018-09-15</rdfs:comment>
        <rdfs:comment>https://resin.io/how-it-works/, 2019-09-16</rdfs:comment>
        <rdfs:label xml:lang="en">UniqueDeviceIdAssignment</rdfs:label>
    </owl:Class>
    


    <!-- http://purl.org/net/iot-dm#OWLClass_38488982_ccd5_4483_bed0_be7fc6bedd59 -->

    <owl:Class rdf:about="http://purl.org/net/iot-dm#OWLClass_38488982_ccd5_4483_bed0_be7fc6bedd59">
        <rdfs:subClassOf rdf:resource="http://purl.org/net/iot-dm#OWLClass_a6cf31e3_5d7b_48b4_bce6_eada63815264"/>
        <rdfs:label xml:lang="en">MicrosoftWindowsOperatingSystem</rdfs:label>
    </owl:Class>
    


    <!-- http://purl.org/net/iot-dm#OWLClass_38648151_2bc3_4eae_ac21_4a37b377b716 -->

    <owl:Class rdf:about="http://purl.org/net/iot-dm#OWLClass_38648151_2bc3_4eae_ac21_4a37b377b716">
        <rdfs:subClassOf rdf:resource="http://purl.org/net/iot-dm#OWLClass_9d0581a1_1bab_4643_9336_b632fa350e2f"/>
        <rdfs:comment>https://resin.io/how-it-works/, 2019-09-16</rdfs:comment>
        <rdfs:label xml:lang="en">ContainerMonitoring</rdfs:label>
    </owl:Class>
    


    <!-- http://purl.org/net/iot-dm#OWLClass_38e18d87_aade_4d8b_ab6e_1da467276a13 -->

    <owl:Class rdf:about="http://purl.org/net/iot-dm#OWLClass_38e18d87_aade_4d8b_ab6e_1da467276a13">
        <rdfs:subClassOf rdf:resource="http://purl.org/net/iot-dm#OWLClass_36c8fbfb_7218_4373_a13b_f46a86f007be"/>
        <rdfs:label xml:lang="en">DeviceAttributes</rdfs:label>
        <rdfs:seeAlso>DeviceMetaData</rdfs:seeAlso>
    </owl:Class>
    


    <!-- http://purl.org/net/iot-dm#OWLClass_391c8c1f_1c6c_400e_94eb_7b7dc8d02ddb -->

    <owl:Class rdf:about="http://purl.org/net/iot-dm#OWLClass_391c8c1f_1c6c_400e_94eb_7b7dc8d02ddb">
        <rdfs:subClassOf rdf:resource="http://purl.org/net/iot-dm#OWLClass_0d737558_6941_40af_ab34_090d7a6e91b9"/>
        <rdfs:label xml:lang="en">DevicePreconfiguration</rdfs:label>
    </owl:Class>
    


    <!-- http://purl.org/net/iot-dm#OWLClass_3a4d744e_1ddc_4fc8_be82_966b2e491882 -->

    <owl:Class rdf:about="http://purl.org/net/iot-dm#OWLClass_3a4d744e_1ddc_4fc8_be82_966b2e491882">
        <rdfs:subClassOf rdf:resource="http://purl.org/net/iot-dm#OWLClass_7ed5a132_c15b_486f_91f4_ad5eb4433cef"/>
        <rdfs:label xml:lang="en">FirmwareStorage</rdfs:label>
    </owl:Class>
    


    <!-- http://purl.org/net/iot-dm#OWLClass_3a67a3e7_f65a_4e72_870f_eadff0700201 -->

    <owl:Class rdf:about="http://purl.org/net/iot-dm#OWLClass_3a67a3e7_f65a_4e72_870f_eadff0700201">
        <rdfs:subClassOf rdf:resource="http://purl.org/net/iot-dm#OWLClass_3e69999a_c294_423f_92bc_6a665a91a72e"/>
        <rdfs:label xml:lang="en">StandardizedDataTypes</rdfs:label>
    </owl:Class>
    


    <!-- http://purl.org/net/iot-dm#OWLClass_3ae3452c_6005_44c9_b207_5ebebcb12c64 -->

    <owl:Class rdf:about="http://purl.org/net/iot-dm#OWLClass_3ae3452c_6005_44c9_b207_5ebebcb12c64">
        <rdfs:subClassOf rdf:resource="http://purl.org/net/iot-dm#OWLClass_4c69720e_8886_407a_b9ce_8fcb374ea363"/>
        <rdfs:comment>OMA-RD-LightweightM2M-V1_1-20180710-A, Label: LightweightM2M-LPW-11</rdfs:comment>
        <rdfs:label xml:lang="en">DevEui</rdfs:label>
    </owl:Class>
    


    <!-- http://purl.org/net/iot-dm#OWLClass_3cddadab_1422_4479_b1cb_4486ecdc0da4 -->

    <owl:Class rdf:about="http://purl.org/net/iot-dm#OWLClass_3cddadab_1422_4479_b1cb_4486ecdc0da4">
        <rdfs:subClassOf rdf:resource="http://purl.org/net/iot-dm#OWLClass_66c3fc69_337f_4795_a467_f0b64b90cb3b"/>
        <rdfs:comment>Recent Advances in Industrial Wireless Sensor Networks Towards Efficient Management in IoT, p. 6</rdfs:comment>
        <rdfs:label xml:lang="en">MassConnections</rdfs:label>
    </owl:Class>
    


    <!-- http://purl.org/net/iot-dm#OWLClass_3ceb9a52_fff5_43aa_9e28_d691e003aff7 -->

    <owl:Class rdf:about="http://purl.org/net/iot-dm#OWLClass_3ceb9a52_fff5_43aa_9e28_d691e003aff7">
        <rdfs:subClassOf rdf:resource="http://purl.org/net/iot-dm#OWLClass_6cb818a3_6278_4bad_8a6b_c01ee623c677"/>
        <rdfs:comment>OMA-RD-LightweightM2M-V1_0-20170208-A, Label: LightweightM2M-HLF-013</rdfs:comment>
        <rdfs:label xml:lang="en">ClientToServerConnectionTriggering</rdfs:label>
    </owl:Class>
    


    <!-- http://purl.org/net/iot-dm#OWLClass_3d63ac6a_4939_44eb_afc5_ebab6cf1cf53 -->

    <owl:Class rdf:about="http://purl.org/net/iot-dm#OWLClass_3d63ac6a_4939_44eb_afc5_ebab6cf1cf53">
        <rdfs:subClassOf rdf:resource="http://purl.org/net/iot-dm#OWLClass_f4a64f37_cafb_440d_8e03_c1895c63f6ea"/>
        <rdfs:label xml:lang="en">ObjectInstanceStorageLocation</rdfs:label>
    </owl:Class>
    


    <!-- http://purl.org/net/iot-dm#OWLClass_3e69999a_c294_423f_92bc_6a665a91a72e -->

    <owl:Class rdf:about="http://purl.org/net/iot-dm#OWLClass_3e69999a_c294_423f_92bc_6a665a91a72e">
        <rdfs:subClassOf rdf:resource="http://purl.org/net/iot-dm#OWLClass_ffcb0dd3_5746_4e9b_9905_50bfb9faff34"/>
        <rdfs:label xml:lang="en">Standardization</rdfs:label>
    </owl:Class>
    


    <!-- http://purl.org/net/iot-dm#OWLClass_3e781bea_1637_4984_bf63_8935b4e49e16 -->

    <owl:Class rdf:about="http://purl.org/net/iot-dm#OWLClass_3e781bea_1637_4984_bf63_8935b4e49e16">
        <rdfs:subClassOf rdf:resource="http://purl.org/net/iot-dm#OWLClass_f6444fa6_1240_4dfa_9bba_affd175076ca"/>
        <rdfs:label xml:lang="en">ReportingModes</rdfs:label>
    </owl:Class>
    


    <!-- http://purl.org/net/iot-dm#OWLClass_3ecade8f_1df9_48ad_a87a_84b305761c34 -->

    <owl:Class rdf:about="http://purl.org/net/iot-dm#OWLClass_3ecade8f_1df9_48ad_a87a_84b305761c34">
        <rdfs:subClassOf rdf:resource="http://purl.org/net/iot-dm#OWLClass_fcd9404e_bd15_4965_8208_dae7b7883655"/>
        <rdfs:comment>Management of IoT Devices in a Physical Network, p. 488</rdfs:comment>
        <rdfs:label xml:lang="en">AutomatedDeviceInformationCompletion</rdfs:label>
    </owl:Class>
    


    <!-- http://purl.org/net/iot-dm#OWLClass_3ff7c7c6_5756_4f3e_ac68_361ae6509fd8 -->

    <owl:Class rdf:about="http://purl.org/net/iot-dm#OWLClass_3ff7c7c6_5756_4f3e_ac68_361ae6509fd8">
        <rdfs:subClassOf rdf:resource="http://purl.org/net/iot-dm#OWLClass_a9fa280a_8537_4626_a942_bab8a45552c7"/>
        <rdfs:comment>Management of IoT Devices in a Physical Network, p. 490</rdfs:comment>
        <rdfs:label xml:lang="en">MessageEvent</rdfs:label>
    </owl:Class>
    


    <!-- http://purl.org/net/iot-dm#OWLClass_402577f2_92ce_4bed_8fd2_eb7be357cddc -->

    <owl:Class rdf:about="http://purl.org/net/iot-dm#OWLClass_402577f2_92ce_4bed_8fd2_eb7be357cddc">
        <rdfs:subClassOf rdf:resource="http://purl.org/net/iot-dm#OWLClass_755c484b_7249_4f24_81fb_2d9ac5948eab"/>
        <rdfs:comment>OMA-RD-LightweightM2M-V1_0-20170208-A, Label: LightweightM2M-HLF-032</rdfs:comment>
        <rdfs:label xml:lang="en">Execute</rdfs:label>
    </owl:Class>
    


    <!-- http://purl.org/net/iot-dm#OWLClass_408c9232_8fd3_469b_8081_2f758ee2f9e8 -->

    <owl:Class rdf:about="http://purl.org/net/iot-dm#OWLClass_408c9232_8fd3_469b_8081_2f758ee2f9e8">
        <rdfs:subClassOf rdf:resource="http://purl.org/net/iot-dm#OWLClass_77093e6d_5bcf_4317_aedc_a07046a659aa"/>
        <rdfs:comment>OMA-RD-LightweightM2M-V1_0-20170208-A, Label: LightweightM2M-AZ-033</rdfs:comment>
        <rdfs:label xml:lang="en">AuthorizationOfCommandsPerResource</rdfs:label>
    </owl:Class>
    


    <!-- http://purl.org/net/iot-dm#OWLClass_41368d9c_8c83_44a2_96df_68f75ba3a48c -->

    <owl:Class rdf:about="http://purl.org/net/iot-dm#OWLClass_41368d9c_8c83_44a2_96df_68f75ba3a48c">
        <rdfs:subClassOf rdf:resource="http://purl.org/net/iot-dm#OWLClass_515bf129_124c_4413_9e49_8de009d76986"/>
        <rdfs:comment>Ontologies for the Internet of Things, 3.2</rdfs:comment>
        <rdfs:label xml:lang="en">DataTransferMethod</rdfs:label>
    </owl:Class>
    


    <!-- http://purl.org/net/iot-dm#OWLClass_41f40ffd_5a9f_42e3_afa1_b9e328d20570 -->

    <owl:Class rdf:about="http://purl.org/net/iot-dm#OWLClass_41f40ffd_5a9f_42e3_afa1_b9e328d20570">
        <rdfs:subClassOf rdf:resource="http://purl.org/net/iot-dm#OWLClass_66c3fc69_337f_4795_a467_f0b64b90cb3b"/>
        <rdfs:comment>IoT home gateway for auto-conﬁguration and management of MQTT devices, section III.</rdfs:comment>
        <rdfs:comment>Management of IoT Devices in a Physical Network, p. 486</rdfs:comment>
        <rdfs:label xml:lang="en">InteroperabilityBetweenHeterogeneousDevices</rdfs:label>
    </owl:Class>
    


    <!-- http://purl.org/net/iot-dm#OWLClass_4238e43b_a030_446d_849f_b48464c7134a -->

    <owl:Class rdf:about="http://purl.org/net/iot-dm#OWLClass_4238e43b_a030_446d_849f_b48464c7134a">
        <rdfs:subClassOf rdf:resource="http://purl.org/net/iot-dm#OWLClass_a2e5a8b7_7e0e_4972_a701_e63b5a3364f6"/>
        <rdfs:label xml:lang="en">ProgrammingLanguage</rdfs:label>
    </owl:Class>
    


    <!-- http://purl.org/net/iot-dm#OWLClass_42d9f56b_27ca_411a_8c4f_91ecb085e413 -->

    <owl:Class rdf:about="http://purl.org/net/iot-dm#OWLClass_42d9f56b_27ca_411a_8c4f_91ecb085e413">
        <rdfs:subClassOf rdf:resource="http://purl.org/net/iot-dm#OWLClass_e7e81967_1b1b_4dfb_b9b6_c40e0ffab441"/>
        <rdfs:label xml:lang="en">TlsDtls</rdfs:label>
    </owl:Class>
    


    <!-- http://purl.org/net/iot-dm#OWLClass_44ddb928_3187_4588_90e9_512f4856bf45 -->

    <owl:Class rdf:about="http://purl.org/net/iot-dm#OWLClass_44ddb928_3187_4588_90e9_512f4856bf45">
        <rdfs:subClassOf rdf:resource="http://purl.org/net/iot-dm#OWLClass_9706d318_5cd1_4e58_8c3b_72eef36ee70a"/>
        <rdfs:comment>draft-moran-suit-architecture-03 (work in progress), p. 12</rdfs:comment>
        <rdfs:label xml:lang="en">FirmwareImagePointers</rdfs:label>
    </owl:Class>
    


    <!-- http://purl.org/net/iot-dm#OWLClass_454a5576_22dd_4d19_ae67_cb6765c19cdf -->

    <owl:Class rdf:about="http://purl.org/net/iot-dm#OWLClass_454a5576_22dd_4d19_ae67_cb6765c19cdf">
        <rdfs:subClassOf rdf:resource="http://purl.org/net/iot-dm#OWLClass_91e1d636_17c7_43c3_ab32_ce7700226d44"/>
        <rdfs:comment>OMA-RD-LightweightM2M-V1_1-20180710-A, Label: LightweightM2M-PKI-003</rdfs:comment>
        <rdfs:label xml:lang="en">CaCertificates</rdfs:label>
    </owl:Class>
    


    <!-- http://purl.org/net/iot-dm#OWLClass_459d0fc6_7d23_4d67_bbf3_641367874b75 -->

    <owl:Class rdf:about="http://purl.org/net/iot-dm#OWLClass_459d0fc6_7d23_4d67_bbf3_641367874b75">
        <rdfs:subClassOf rdf:resource="http://purl.org/net/iot-dm#OWLClass_213b255b_d2a6_41ac_9e58_75311a7288f3"/>
        <rdfs:comment>Management of IoT Devices in a Physical Network, p. 488</rdfs:comment>
        <rdfs:label xml:lang="en">DeviceServices</rdfs:label>
    </owl:Class>
    


    <!-- http://purl.org/net/iot-dm#OWLClass_4684c1c5_feb0_43e2_880b_35fd9f5a6d08 -->

    <owl:Class rdf:about="http://purl.org/net/iot-dm#OWLClass_4684c1c5_feb0_43e2_880b_35fd9f5a6d08">
        <rdfs:subClassOf rdf:resource="http://purl.org/net/iot-dm#OWLClass_ffcb0dd3_5746_4e9b_9905_50bfb9faff34"/>
        <rdfs:comment>OMA-RD-LightweightM2M-V1_1-20180710-A, Label: LightweightM2M-LeG-005</rdfs:comment>
        <rdfs:comment>OMA-RD-LightweightM2M-V1_1-20180710-A, Label: LightweightM2M-MBT-001</rdfs:comment>
        <rdfs:label xml:lang="en">AllNetworkTopologyTraversal</rdfs:label>
    </owl:Class>
    


    <!-- http://purl.org/net/iot-dm#OWLClass_46a7e189_9a8b_455b_8a6e_e53d55e0ef91 -->

    <owl:Class rdf:about="http://purl.org/net/iot-dm#OWLClass_46a7e189_9a8b_455b_8a6e_e53d55e0ef91">
        <rdfs:subClassOf rdf:resource="http://purl.org/net/iot-dm#OWLClass_13c796b1_46e2_4fc7_b2d1_299b6746d07f"/>
        <rdfs:comment>IoT home gateway for auto-conﬁguration and management of MQTT devices, section III.</rdfs:comment>
        <rdfs:label xml:lang="en">Uri</rdfs:label>
    </owl:Class>
    


    <!-- http://purl.org/net/iot-dm#OWLClass_47c759b6_e09c_4798_9056_f499ebeecae4 -->

    <owl:Class rdf:about="http://purl.org/net/iot-dm#OWLClass_47c759b6_e09c_4798_9056_f499ebeecae4">
        <rdfs:subClassOf rdf:resource="http://purl.org/net/iot-dm#OWLClass_10ff6f33_7c39_432c_9ac0_c8c9d830b8b9"/>
        <rdfs:comment>Recent Advances in Industrial Wireless Sensor Networks Towards Efficient Management in IoT, p. 6</rdfs:comment>
        <rdfs:comment>https://resin.io/features/, 2018-09-15</rdfs:comment>
        <rdfs:label xml:lang="en">Api</rdfs:label>
    </owl:Class>
    


    <!-- http://purl.org/net/iot-dm#OWLClass_491b953e_eea2_4cd6_a616_8e5497b95cec -->

    <owl:Class rdf:about="http://purl.org/net/iot-dm#OWLClass_491b953e_eea2_4cd6_a616_8e5497b95cec">
        <rdfs:subClassOf rdf:resource="http://purl.org/net/iot-dm#OWLClass_21fa4e78_3300_43d8_83c7_78d9ee314b79"/>
        <rdfs:comment>OMA-RD-LightweightM2M-V1_1-20180710-A, Label: LightweightM2M-RMo-002</rdfs:comment>
        <rdfs:label xml:lang="en">CausesOfObservation</rdfs:label>
    </owl:Class>
    


    <!-- http://purl.org/net/iot-dm#OWLClass_4948fab8_1838_4fe0_82a0_27a8ac8eded5 -->

    <owl:Class rdf:about="http://purl.org/net/iot-dm#OWLClass_4948fab8_1838_4fe0_82a0_27a8ac8eded5">
        <rdfs:subClassOf rdf:resource="http://purl.org/net/iot-dm#OWLClass_843d87bc_a343_470f_bff0_872b15b14c16"/>
        <rdfs:comment xml:lang="en">draft-moran-suit-architecture-03 (work in progress), p. 6</rdfs:comment>
        <rdfs:label xml:lang="en">FirmwareImageDistribution</rdfs:label>
    </owl:Class>
    


    <!-- http://purl.org/net/iot-dm#OWLClass_49ac79d7_c437_4c71_8da3_ae6ad1e83073 -->

    <owl:Class rdf:about="http://purl.org/net/iot-dm#OWLClass_49ac79d7_c437_4c71_8da3_ae6ad1e83073">
        <rdfs:subClassOf rdf:resource="http://purl.org/net/iot-dm#OWLClass_2a645b44_80eb_49d7_8add_d5dc3d46a6f9"/>
        <rdfs:comment xml:lang="en">&quot;The author is the entity that creates the firmware image, signs and/or encrypts it and attaches a manifest to it. The author is most likely a developer using a set of tools.&quot;, draft-moran-suit-architecture-03 (work in progress), p. 5</rdfs:comment>
        <rdfs:label xml:lang="en">FirmwareAuthor</rdfs:label>
    </owl:Class>
    


    <!-- http://purl.org/net/iot-dm#OWLClass_4aa258d4_0b15_42d1_b4ed_87a2494976e5 -->

    <owl:Class rdf:about="http://purl.org/net/iot-dm#OWLClass_4aa258d4_0b15_42d1_b4ed_87a2494976e5">
        <rdfs:subClassOf rdf:resource="http://purl.org/net/iot-dm#OWLClass_ffcb0dd3_5746_4e9b_9905_50bfb9faff34"/>
        <rdfs:comment>Recent Advances in Industrial Wireless Sensor Networks Towards Efficient Management in IoT, p. 8</rdfs:comment>
        <rdfs:label xml:lang="en">OpenProtocol</rdfs:label>
    </owl:Class>
    


    <!-- http://purl.org/net/iot-dm#OWLClass_4b1504d5_8402_464c_a20c_f1c564d0ff8f -->

    <owl:Class rdf:about="http://purl.org/net/iot-dm#OWLClass_4b1504d5_8402_464c_a20c_f1c564d0ff8f">
        <rdfs:subClassOf rdf:resource="http://purl.org/net/iot-dm#OWLClass_cbca8db6_d106_4651_a12c_b8fe629efbda"/>
        <rdfs:comment>Management of IoT Devices in a Physical Network, p. 490</rdfs:comment>
        <rdfs:label xml:lang="en">AlertingEngine</rdfs:label>
    </owl:Class>
    


    <!-- http://purl.org/net/iot-dm#OWLClass_4bff393a_9b00_4db5_a375_9baf63f63167 -->

    <owl:Class rdf:about="http://purl.org/net/iot-dm#OWLClass_4bff393a_9b00_4db5_a375_9baf63f63167">
        <rdfs:subClassOf rdf:resource="http://purl.org/net/iot-dm#OWLClass_b21422b7_b049_4b16_b3e0_53d1c9d53e85"/>
        <rdfs:label xml:lang="en">PlatformControl</rdfs:label>
    </owl:Class>
    


    <!-- http://purl.org/net/iot-dm#OWLClass_4c2fcbc0_463d_4447_a672_aa371ad22812 -->

    <owl:Class rdf:about="http://purl.org/net/iot-dm#OWLClass_4c2fcbc0_463d_4447_a672_aa371ad22812">
        <rdfs:subClassOf rdf:resource="http://purl.org/net/iot-dm#OWLClass_3ecade8f_1df9_48ad_a87a_84b305761c34"/>
        <rdfs:comment>Management of IoT Devices in a Physical Network, p. 490</rdfs:comment>
        <rdfs:label xml:lang="en">PatternBasedAutomation</rdfs:label>
    </owl:Class>
    


    <!-- http://purl.org/net/iot-dm#OWLClass_4c69720e_8886_407a_b9ce_8fcb374ea363 -->

    <owl:Class rdf:about="http://purl.org/net/iot-dm#OWLClass_4c69720e_8886_407a_b9ce_8fcb374ea363">
        <rdfs:subClassOf rdf:resource="http://purl.org/net/iot-dm#OWLClass_928a3dbe_0ae6_42b7_a752_d48930d19fae"/>
        <rdfs:comment>OMA-RD-LightweightM2M-V1_1-20180710-A, Label: LightweightM2M-LPW-11</rdfs:comment>
        <rdfs:label xml:lang="en">InteroperableLorwanDeviceActivationMethod</rdfs:label>
    </owl:Class>
    


    <!-- http://purl.org/net/iot-dm#OWLClass_4c69f2df_35c9_4bf1_8b7f_b0e8fcac7aca -->

    <owl:Class rdf:about="http://purl.org/net/iot-dm#OWLClass_4c69f2df_35c9_4bf1_8b7f_b0e8fcac7aca">
        <rdfs:subClassOf rdf:resource="http://purl.org/net/iot-dm#OWLClass_7c8282da_3443_4c49_a838_df6cb9a459c9"/>
        <rdfs:label xml:lang="en">FirmwareUpdateFailures</rdfs:label>
    </owl:Class>
    


    <!-- http://purl.org/net/iot-dm#OWLClass_4c92b333_17aa_4b39_86cb_89b4a5083d67 -->

    <owl:Class rdf:about="http://purl.org/net/iot-dm#OWLClass_4c92b333_17aa_4b39_86cb_89b4a5083d67">
        <rdfs:subClassOf rdf:resource="http://purl.org/net/iot-dm#OWLClass_38e18d87_aade_4d8b_ab6e_1da467276a13"/>
        <rdfs:comment>Recent Advances in Industrial Wireless Sensor Networks Towards Efficient Management in IoT, p. 13</rdfs:comment>
        <rdfs:label xml:lang="en">DeviceAddress</rdfs:label>
    </owl:Class>
    


    <!-- http://purl.org/net/iot-dm#OWLClass_4cb539bf_351f_4637_96c6_7a614670f3c1 -->

    <owl:Class rdf:about="http://purl.org/net/iot-dm#OWLClass_4cb539bf_351f_4637_96c6_7a614670f3c1">
        <rdfs:subClassOf rdf:resource="http://purl.org/net/iot-dm#OWLClass_9706d318_5cd1_4e58_8c3b_72eef36ee70a"/>
        <rdfs:comment>draft-moran-suit-architecture-03 (work in progress), p. 12</rdfs:comment>
        <rdfs:label xml:lang="en">FirmwareImageFormat</rdfs:label>
    </owl:Class>
    


    <!-- http://purl.org/net/iot-dm#OWLClass_4cea09eb_fd16_437b_818d_7438ee1c1880 -->

    <owl:Class rdf:about="http://purl.org/net/iot-dm#OWLClass_4cea09eb_fd16_437b_818d_7438ee1c1880">
        <rdfs:subClassOf rdf:resource="http://purl.org/net/iot-dm#OWLClass_3d63ac6a_4939_44eb_afc5_ebab6cf1cf53"/>
        <rdfs:comment>OMA-RD-LightweightM2M-V1_1-20180710-A, Label: LightweightM2M-SCS-6</rdfs:comment>
        <rdfs:label xml:lang="en">ObjectInstanceStorageLocationQuerying</rdfs:label>
    </owl:Class>
    


    <!-- http://purl.org/net/iot-dm#OWLClass_4d2d07e0_681a_4474_8172_e06c372aa119 -->

    <owl:Class rdf:about="http://purl.org/net/iot-dm#OWLClass_4d2d07e0_681a_4474_8172_e06c372aa119">
        <rdfs:subClassOf rdf:resource="http://purl.org/net/iot-dm#OWLClass_8a91ffb6_d1c9_4026_9031_fd318df66665"/>
        <rdfs:comment>Management of IoT Devices in a Physical Network, p. 488</rdfs:comment>
        <rdfs:label xml:lang="en">SerialNumber</rdfs:label>
    </owl:Class>
    


    <!-- http://purl.org/net/iot-dm#OWLClass_4d396412_7f2b_4b3e_bdc6_058a63a3cc91 -->

    <owl:Class rdf:about="http://purl.org/net/iot-dm#OWLClass_4d396412_7f2b_4b3e_bdc6_058a63a3cc91">
        <rdfs:subClassOf rdf:resource="http://purl.org/net/iot-dm#OWLClass_cfbd03e3_461e_49ac_a682_824dcbfcacdd"/>
        <rdfs:comment>Recent Advances in Industrial Wireless Sensor Networks Towards Efficient Management in IoT, p. 13</rdfs:comment>
        <rdfs:label xml:lang="en">ApplicationApi</rdfs:label>
    </owl:Class>
    


    <!-- http://purl.org/net/iot-dm#OWLClass_4d7e76e2_bd97_4f17_8b96_ef326aab5062 -->

    <owl:Class rdf:about="http://purl.org/net/iot-dm#OWLClass_4d7e76e2_bd97_4f17_8b96_ef326aab5062">
        <rdfs:subClassOf rdf:resource="http://purl.org/net/iot-dm#OWLClass_928a3dbe_0ae6_42b7_a752_d48930d19fae"/>
        <rdfs:comment>OMA-RD-LightweightM2M-V1_1-20180710-A, Label: LightweightM2M-LPW-12</rdfs:comment>
        <rdfs:label xml:lang="en">InteroperationWithLorwanSecurityProtocol</rdfs:label>
    </owl:Class>
    


    <!-- http://purl.org/net/iot-dm#OWLClass_4daf23df_ce27_4a36_8ce8_efb91ef3cef6 -->

    <owl:Class rdf:about="http://purl.org/net/iot-dm#OWLClass_4daf23df_ce27_4a36_8ce8_efb91ef3cef6">
        <rdfs:subClassOf rdf:resource="http://purl.org/net/iot-dm#OWLClass_845f9a81_9845_4e96_b5cf_5d06ab798969"/>
        <rdfs:comment>Management of IoT Devices in a Physical Network, p. 488, 490</rdfs:comment>
        <rdfs:label xml:lang="en">RulesEngine</rdfs:label>
    </owl:Class>
    


    <!-- http://purl.org/net/iot-dm#OWLClass_4e1b6f8d_ac53_4b88_a781_eac802f81766 -->

    <owl:Class rdf:about="http://purl.org/net/iot-dm#OWLClass_4e1b6f8d_ac53_4b88_a781_eac802f81766">
        <rdfs:subClassOf rdf:resource="http://purl.org/net/iot-dm#OWLClass_a1b8792e_7d00_48b8_9efe_c6e47629e99c"/>
        <rdfs:comment>Recent Advances in Industrial Wireless Sensor Networks Towards Efficient Management in IoT, p. 13</rdfs:comment>
        <rdfs:label xml:lang="en">EventAnalytics</rdfs:label>
    </owl:Class>
    


    <!-- http://purl.org/net/iot-dm#OWLClass_4e2c8db4_a7e0_48ea_8171_6bb97a042a5e -->

    <owl:Class rdf:about="http://purl.org/net/iot-dm#OWLClass_4e2c8db4_a7e0_48ea_8171_6bb97a042a5e">
        <rdfs:subClassOf rdf:resource="http://purl.org/net/iot-dm#OWLClass_c8340585_9c41_4f98_8f90_b4e2436e8829"/>
        <rdfs:comment>OMA-RD-LightweightM2M-V1_1-20180710-A, Label: LightweightM2M-LPW-1</rdfs:comment>
        <rdfs:label xml:lang="en">ExternalIdentifierFor3gppCellularLpwan</rdfs:label>
    </owl:Class>
    


    <!-- http://purl.org/net/iot-dm#OWLClass_4ed0fde2_9477_4c43_bd55_eca63520c80d -->

    <owl:Class rdf:about="http://purl.org/net/iot-dm#OWLClass_4ed0fde2_9477_4c43_bd55_eca63520c80d">
        <rdfs:subClassOf rdf:resource="http://purl.org/net/iot-dm#OWLClass_56e577ad_039f_4eeb_be83_40fd15e9c7b8"/>
        <rdfs:comment>OMA-RD-LightweightM2M-V1_1-20180710-A, Label: LightweightM2M-SCS-2</rdfs:comment>
        <rdfs:label xml:lang="en">ServerSupportedSecureComponentAuthentication</rdfs:label>
    </owl:Class>
    


    <!-- http://purl.org/net/iot-dm#OWLClass_4eeddc87_d8fa_46cc_b242_0971b707256c -->

    <owl:Class rdf:about="http://purl.org/net/iot-dm#OWLClass_4eeddc87_d8fa_46cc_b242_0971b707256c">
        <rdfs:subClassOf rdf:resource="http://purl.org/net/iot-dm#OWLClass_8e4f6b4d_92dd_4de5_9e89_8d0f3d918c5e"/>
        <rdfs:comment>OMA-RD-LightweightM2M-V1_1-20180710-A, Label: LightweightM2M-RMo-001</rdfs:comment>
        <rdfs:label xml:lang="en">RelationalOperatorBasedReportingMechanism</rdfs:label>
    </owl:Class>
    


    <!-- http://purl.org/net/iot-dm#OWLClass_4fd8d4e2_091f_4675_9391_1f63a7e3e133 -->

    <owl:Class rdf:about="http://purl.org/net/iot-dm#OWLClass_4fd8d4e2_091f_4675_9391_1f63a7e3e133">
        <rdfs:subClassOf rdf:resource="http://purl.org/net/iot-dm#OWLClass_2fb332cc_9b13_4fbc_af07_4ce1a662e062"/>
        <rdfs:comment>OMA-RD-LightweightM2M-V1_1-20180710-A, Label: LightweightM2M-LeG-006</rdfs:comment>
        <rdfs:label xml:lang="en">DeviceCapabilities</rdfs:label>
    </owl:Class>
    


    <!-- http://purl.org/net/iot-dm#OWLClass_506a07f5_4566_41a4_84ac_ea621caa87b7 -->

    <owl:Class rdf:about="http://purl.org/net/iot-dm#OWLClass_506a07f5_4566_41a4_84ac_ea621caa87b7">
        <rdfs:subClassOf rdf:resource="http://purl.org/net/iot-dm#OWLClass_10ff6f33_7c39_432c_9ac0_c8c9d830b8b9"/>
        <rdfs:label xml:lang="en">UserInterface</rdfs:label>
    </owl:Class>
    


    <!-- http://purl.org/net/iot-dm#OWLClass_50fbea29_82d9_4084_8911_5be2605906e2 -->

    <owl:Class rdf:about="http://purl.org/net/iot-dm#OWLClass_50fbea29_82d9_4084_8911_5be2605906e2">
        <rdfs:subClassOf rdf:resource="http://purl.org/net/iot-dm#OWLClass_f86901a5_61d3_4e5a_8ec6_984ffda5de83"/>
        <rdfs:comment>IoT home gateway for auto-conﬁguration and management of MQTT devices, section III.</rdfs:comment>
        <rdfs:label xml:lang="en">RegisterDeviceInformationAfterAdvertisement</rdfs:label>
    </owl:Class>
    


    <!-- http://purl.org/net/iot-dm#OWLClass_51336fa4_fb22_4ebd_a256_d97feab08b64 -->

    <owl:Class rdf:about="http://purl.org/net/iot-dm#OWLClass_51336fa4_fb22_4ebd_a256_d97feab08b64">
        <rdfs:subClassOf rdf:resource="http://purl.org/net/iot-dm#OWLClass_8e4f6b4d_92dd_4de5_9e89_8d0f3d918c5e"/>
        <rdfs:comment>OMA-RD-LightweightM2M-V1_0-20170208-A, Label: LightweightM2M-HLF-021</rdfs:comment>
        <rdfs:label xml:lang="en">EventTriggerReportingMechanismConfiguration</rdfs:label>
    </owl:Class>
    


    <!-- http://purl.org/net/iot-dm#OWLClass_515bf129_124c_4413_9e49_8de009d76986 -->

    <owl:Class rdf:about="http://purl.org/net/iot-dm#OWLClass_515bf129_124c_4413_9e49_8de009d76986">
        <rdfs:subClassOf rdf:resource="http://purl.org/net/iot-dm#OWLClass_213b255b_d2a6_41ac_9e58_75311a7288f3"/>
        <rdfs:comment>Ontologies for the Internet of Things, 2., 3.2</rdfs:comment>
        <rdfs:label xml:lang="en">SensingModality</rdfs:label>
    </owl:Class>
    


    <!-- http://purl.org/net/iot-dm#OWLClass_51f271e6_f53c_4e1c_8f4c_8827c382e69a -->

    <owl:Class rdf:about="http://purl.org/net/iot-dm#OWLClass_51f271e6_f53c_4e1c_8f4c_8827c382e69a">
        <rdfs:subClassOf rdf:resource="http://purl.org/net/iot-dm#OWLClass_0b06f64b_69d9_4b6c_965b_186dc58c39eb"/>
        <rdfs:comment>Recent Advances in Industrial Wireless Sensor Networks Towards Efficient Management in IoT, p. 13</rdfs:comment>
        <rdfs:label xml:lang="en">DataAnalytics</rdfs:label>
    </owl:Class>
    


    <!-- http://purl.org/net/iot-dm#OWLClass_51f80f1b_9d49_4d14_9668_07947f56db35 -->

    <owl:Class rdf:about="http://purl.org/net/iot-dm#OWLClass_51f80f1b_9d49_4d14_9668_07947f56db35">
        <rdfs:subClassOf rdf:resource="http://purl.org/net/iot-dm#OWLClass_f1b54d5c_4482_4645_a2f1_6efa8e12b8de"/>
        <owl:disjointWith rdf:resource="http://purl.org/net/iot-dm#OWLClass_efe7810e_2a97_4b8e_9967_d305e3277152"/>
        <rdfs:label xml:lang="en">WireBased</rdfs:label>
    </owl:Class>
    


    <!-- http://purl.org/net/iot-dm#OWLClass_5210941a_39bd_48b4_9dfe_1d58f87cc61b -->

    <owl:Class rdf:about="http://purl.org/net/iot-dm#OWLClass_5210941a_39bd_48b4_9dfe_1d58f87cc61b">
        <rdfs:subClassOf rdf:resource="http://purl.org/net/iot-dm#OWLClass_267278cd_85b2_4704_84d7_a7cb4004d16d"/>
        <rdfs:comment>https://resin.io/features/, 2018-09-15</rdfs:comment>
        <rdfs:label xml:lang="en">ServiceEnvironmentVariables</rdfs:label>
    </owl:Class>
    


    <!-- http://purl.org/net/iot-dm#OWLClass_5236ab9a_e39c_4e90_b265_63064ec80b33 -->

    <owl:Class rdf:about="http://purl.org/net/iot-dm#OWLClass_5236ab9a_e39c_4e90_b265_63064ec80b33">
        <rdfs:subClassOf rdf:resource="http://purl.org/net/iot-dm#OWLClass_1bd19af8_5e90_482f_b798_79ba7cc8d671"/>
        <rdfs:label xml:lang="en">DeviceDependedServices</rdfs:label>
    </owl:Class>
    


    <!-- http://purl.org/net/iot-dm#OWLClass_5303cc63_d095_4c30_b893_51cfe691cb7e -->

    <owl:Class rdf:about="http://purl.org/net/iot-dm#OWLClass_5303cc63_d095_4c30_b893_51cfe691cb7e">
        <rdfs:subClassOf rdf:resource="http://purl.org/net/iot-dm#OWLClass_5985dbe5_dc91_4677_a070_127370474bb9"/>
        <rdfs:comment>Recent Advances in Industrial Wireless Sensor Networks Towards Efficient Management in IoT, p. 9</rdfs:comment>
        <rdfs:label xml:lang="en">DeviceParameterConfiguration</rdfs:label>
    </owl:Class>
    


    <!-- http://purl.org/net/iot-dm#OWLClass_5445a1b7_eb6b_4343_bd06_a0427b710d6d -->

    <owl:Class rdf:about="http://purl.org/net/iot-dm#OWLClass_5445a1b7_eb6b_4343_bd06_a0427b710d6d">
        <rdfs:subClassOf rdf:resource="http://purl.org/net/iot-dm#OWLClass_9e1800f6_b3ba_41ee_b0ce_dac66a1a8680"/>
        <rdfs:label xml:lang="en">TransportLayerProtocol</rdfs:label>
    </owl:Class>
    


    <!-- http://purl.org/net/iot-dm#OWLClass_55163170_51d6_453d_b20b_de70dbeca410 -->

    <owl:Class rdf:about="http://purl.org/net/iot-dm#OWLClass_55163170_51d6_453d_b20b_de70dbeca410">
        <rdfs:subClassOf rdf:resource="http://purl.org/net/iot-dm#OWLClass_3300e6af_4338_4bf4_ab9e_632af0b5ad65"/>
        <rdfs:comment>OMA-RD-LightweightM2M-V1_1-20180710-A, Label: LightweightM2M-BsR-009</rdfs:comment>
        <rdfs:label xml:lang="en">ApnDesignation</rdfs:label>
    </owl:Class>
    


    <!-- http://purl.org/net/iot-dm#OWLClass_55d1cb26_9c78_4aa1_8a68_6ccd0b705736 -->

    <owl:Class rdf:about="http://purl.org/net/iot-dm#OWLClass_55d1cb26_9c78_4aa1_8a68_6ccd0b705736">
        <rdfs:subClassOf rdf:resource="http://purl.org/net/iot-dm#OWLClass_6f8197a0_9425_4239_bea9_7e354c8cba24"/>
        <rdfs:comment>&quot;This tells the supervisor to only download the binary differences between the old and the new images.&quot;,
https://resin.io/how-it-works/, 2019-09-16</rdfs:comment>
        <rdfs:label xml:lang="en">DeltaUpdates</rdfs:label>
    </owl:Class>
    


    <!-- http://purl.org/net/iot-dm#OWLClass_565b5a10_179b_4c7f_a3fc_ee5842a5210e -->

    <owl:Class rdf:about="http://purl.org/net/iot-dm#OWLClass_565b5a10_179b_4c7f_a3fc_ee5842a5210e">
        <rdfs:subClassOf rdf:resource="http://purl.org/net/iot-dm#OWLClass_fcd9404e_bd15_4965_8208_dae7b7883655"/>
        <rdfs:comment>Management of IoT Devices in a Physical Network, p. 488</rdfs:comment>
        <rdfs:label xml:lang="en">ManualDeviceInformationCompletion</rdfs:label>
    </owl:Class>
    


    <!-- http://purl.org/net/iot-dm#OWLClass_56ca2f5d_d065_4fe0_bfd8_9c86ea85f200 -->

    <owl:Class rdf:about="http://purl.org/net/iot-dm#OWLClass_56ca2f5d_d065_4fe0_bfd8_9c86ea85f200">
        <rdfs:subClassOf rdf:resource="http://purl.org/net/iot-dm#OWLClass_1bd19af8_5e90_482f_b798_79ba7cc8d671"/>
        <rdfs:label xml:lang="en">BigDataManagement</rdfs:label>
    </owl:Class>
    


    <!-- http://purl.org/net/iot-dm#OWLClass_56e577ad_039f_4eeb_be83_40fd15e9c7b8 -->

    <owl:Class rdf:about="http://purl.org/net/iot-dm#OWLClass_56e577ad_039f_4eeb_be83_40fd15e9c7b8">
        <rdfs:subClassOf rdf:resource="http://purl.org/net/iot-dm#OWLClass_9e3d4f19_96c7_4932_a007_26fa592f3423"/>
        <rdfs:label xml:lang="en">SecureComponentSupport</rdfs:label>
    </owl:Class>
    


    <!-- http://purl.org/net/iot-dm#OWLClass_56ebbdf9_64f2_4b0c_acdb_20694cd96f8c -->

    <owl:Class rdf:about="http://purl.org/net/iot-dm#OWLClass_56ebbdf9_64f2_4b0c_acdb_20694cd96f8c">
        <rdfs:subClassOf rdf:resource="http://purl.org/net/iot-dm#OWLClass_2fb332cc_9b13_4fbc_af07_4ce1a662e062"/>
        <rdfs:label xml:lang="en">SecurityMechanisms</rdfs:label>
    </owl:Class>
    


    <!-- http://purl.org/net/iot-dm#OWLClass_574c5366_c20d_467b_8ad6_787581d5f349 -->

    <owl:Class rdf:about="http://purl.org/net/iot-dm#OWLClass_574c5366_c20d_467b_8ad6_787581d5f349">
        <rdfs:subClassOf rdf:resource="http://purl.org/net/iot-dm#OWLClass_d5baf8ff_3ca0_40a1_988a_a5e23a144824"/>
        <rdfs:comment>&quot;translate the captured event from the sensor devices into a standard format and deliver it through broadband or wireless networks to the cloud platform&quot;, Recent Advances in Industrial Wireless Sensor Networks Towards Efficient Management in IoT, p. 6</rdfs:comment>
        <rdfs:label xml:lang="en">DeviceAdapter</rdfs:label>
    </owl:Class>
    


    <!-- http://purl.org/net/iot-dm#OWLClass_57f6a391_24c8_4901_93fb_7b09b9ec1f23 -->

    <owl:Class rdf:about="http://purl.org/net/iot-dm#OWLClass_57f6a391_24c8_4901_93fb_7b09b9ec1f23">
        <rdfs:subClassOf rdf:resource="http://purl.org/net/iot-dm#OWLClass_68e5a285_5ba6_4cb1_85e7_ac792a46c65f"/>
        <rdfs:comment>Ontologies for the Internet of Things, 3.2</rdfs:comment>
        <rdfs:label xml:lang="en">HardwareComponents</rdfs:label>
        <rdfs:seeAlso>InternalComponents</rdfs:seeAlso>
    </owl:Class>
    


    <!-- http://purl.org/net/iot-dm#OWLClass_59540155_cb79_4e35_8db8_7519fb3535d5 -->

    <owl:Class rdf:about="http://purl.org/net/iot-dm#OWLClass_59540155_cb79_4e35_8db8_7519fb3535d5">
        <rdfs:subClassOf rdf:resource="http://purl.org/net/iot-dm#OWLClass_b21422b7_b049_4b16_b3e0_53d1c9d53e85"/>
        <rdfs:label xml:lang="en">DeviceRegistry</rdfs:label>
    </owl:Class>
    


    <!-- http://purl.org/net/iot-dm#OWLClass_5955434e_8208_462c_a26b_6628081fe0bf -->

    <owl:Class rdf:about="http://purl.org/net/iot-dm#OWLClass_5955434e_8208_462c_a26b_6628081fe0bf">
        <rdfs:subClassOf rdf:resource="http://purl.org/net/iot-dm#OWLClass_2fb332cc_9b13_4fbc_af07_4ce1a662e062"/>
        <rdfs:label xml:lang="en">ConfigurationParameters</rdfs:label>
    </owl:Class>
    


    <!-- http://purl.org/net/iot-dm#OWLClass_5985dbe5_dc91_4677_a070_127370474bb9 -->

    <owl:Class rdf:about="http://purl.org/net/iot-dm#OWLClass_5985dbe5_dc91_4677_a070_127370474bb9">
        <rdfs:subClassOf rdf:resource="http://purl.org/net/iot-dm#OWLClass_b21422b7_b049_4b16_b3e0_53d1c9d53e85"/>
        <rdfs:comment>OMA-RD-LightweightM2M-V1_0-20170208-A, Label: LightweightM2M-HLF-012</rdfs:comment>
        <rdfs:label xml:lang="en">DeviceConfiguration</rdfs:label>
    </owl:Class>
    


    <!-- http://purl.org/net/iot-dm#OWLClass_598813b0_a951_4d92_b5a1_a3eefb2d0082 -->

    <owl:Class rdf:about="http://purl.org/net/iot-dm#OWLClass_598813b0_a951_4d92_b5a1_a3eefb2d0082">
        <rdfs:subClassOf rdf:resource="http://purl.org/net/iot-dm#OWLClass_213b255b_d2a6_41ac_9e58_75311a7288f3"/>
        <rdfs:comment>Ontologies for the Internet of Things, 3.2</rdfs:comment>
        <rdfs:label xml:lang="en">HardwareComponents</rdfs:label>
        <rdfs:seeAlso>InternalComponents</rdfs:seeAlso>
    </owl:Class>
    


    <!-- http://purl.org/net/iot-dm#OWLClass_59f9fddd_1432_4e40_a405_357e43b95f6f -->

    <owl:Class rdf:about="http://purl.org/net/iot-dm#OWLClass_59f9fddd_1432_4e40_a405_357e43b95f6f">
        <rdfs:subClassOf rdf:resource="http://purl.org/net/iot-dm#OWLClass_0fd00cb3_e44d_420b_bff2_9aafb1b10ace"/>
        <rdfs:comment>IoT home gateway for auto-conﬁguration and management of MQTT devices, section I., II., III.</rdfs:comment>
        <rdfs:label xml:lang="en">DynamicDeviceDiscovery</rdfs:label>
    </owl:Class>
    


    <!-- http://purl.org/net/iot-dm#OWLClass_5aea1112_cae7_4859_9130_ea812551f4a9 -->

    <owl:Class rdf:about="http://purl.org/net/iot-dm#OWLClass_5aea1112_cae7_4859_9130_ea812551f4a9">
        <rdfs:subClassOf rdf:resource="http://purl.org/net/iot-dm#OWLClass_6cb818a3_6278_4bad_8a6b_c01ee623c677"/>
        <rdfs:comment>OMA-RD-LightweightM2M-V1_0-20170208-A, Label: LightweightM2M-HLF-010</rdfs:comment>
        <rdfs:label xml:lang="en">DeviceEnablingAndDisabling</rdfs:label>
    </owl:Class>
    


    <!-- http://purl.org/net/iot-dm#OWLClass_5b1bfc98_d3eb_4073_934f_984c24ddfef4 -->

    <owl:Class rdf:about="http://purl.org/net/iot-dm#OWLClass_5b1bfc98_d3eb_4073_934f_984c24ddfef4">
        <rdfs:subClassOf rdf:resource="http://purl.org/net/iot-dm#OWLClass_ffcb0dd3_5746_4e9b_9905_50bfb9faff34"/>
        <rdfs:comment>OMA-RD-LightweightM2M-V1_0-20170208-A, Label: LightweightM2M-HLF-015</rdfs:comment>
        <rdfs:label xml:lang="en">SmsBasedCommunication</rdfs:label>
    </owl:Class>
    


    <!-- http://purl.org/net/iot-dm#OWLClass_5c08eefa_8244_4272_b68c_6f24666eb49d -->

    <owl:Class rdf:about="http://purl.org/net/iot-dm#OWLClass_5c08eefa_8244_4272_b68c_6f24666eb49d">
        <rdfs:subClassOf rdf:resource="http://purl.org/net/iot-dm#OWLClass_b21422b7_b049_4b16_b3e0_53d1c9d53e85"/>
        <rdfs:comment>The Internet of Things: An Overview, p. 25</rdfs:comment>
        <rdfs:label xml:lang="en">DeviceSecurityManagement</rdfs:label>
    </owl:Class>
    


    <!-- http://purl.org/net/iot-dm#OWLClass_5df1636e_693f_46b1_b408_696aca13c94a -->

    <owl:Class rdf:about="http://purl.org/net/iot-dm#OWLClass_5df1636e_693f_46b1_b408_696aca13c94a">
        <rdfs:subClassOf rdf:resource="http://purl.org/net/iot-dm#OWLClass_c8340585_9c41_4f98_8f90_b4e2436e8829"/>
        <rdfs:comment>OMA-RD-LightweightM2M-V1_1-20180710-A, Label: LightweightM2M-LPW-4</rdfs:comment>
        <rdfs:label xml:lang="en">3gppCiotNetworkInteroperability</rdfs:label>
    </owl:Class>
    


    <!-- http://purl.org/net/iot-dm#OWLClass_5e93b1d1_1389_4968_a99c_dc58a8d544bb -->

    <owl:Class rdf:about="http://purl.org/net/iot-dm#OWLClass_5e93b1d1_1389_4968_a99c_dc58a8d544bb">
        <rdfs:subClassOf rdf:resource="http://purl.org/net/iot-dm#OWLClass_e8bba4e0_1b39_45bf_b031_aaa20123bd06"/>
        <rdfs:comment>OMA-RD-LightweightM2M-V1_0-20170208-A, Label: LightweightM2M-DI-001</rdfs:comment>
        <rdfs:label xml:lang="en">DataIntegrityEnsuranceMechanism</rdfs:label>
    </owl:Class>
    


    <!-- http://purl.org/net/iot-dm#OWLClass_5fc8a8e2_e2d0_4920_af45_b6393b5ed989 -->

    <owl:Class rdf:about="http://purl.org/net/iot-dm#OWLClass_5fc8a8e2_e2d0_4920_af45_b6393b5ed989">
        <rdfs:subClassOf rdf:resource="http://purl.org/net/iot-dm#OWLClass_b5c0d821_b62f_4098_9a87_9ab068cebe46"/>
        <rdfs:comment>Management of IoT Devices in a Physical Network, p. 488</rdfs:comment>
        <rdfs:label xml:lang="en">DeviceInformationKnowledgeBase</rdfs:label>
    </owl:Class>
    


    <!-- http://purl.org/net/iot-dm#OWLClass_60093b73_8d79_4465_911f_edf5a8029c89 -->

    <owl:Class rdf:about="http://purl.org/net/iot-dm#OWLClass_60093b73_8d79_4465_911f_edf5a8029c89">
        <rdfs:subClassOf rdf:resource="http://purl.org/net/iot-dm#OWLClass_18471212_0dca_43c7_807a_1e3346b35c76"/>
        <rdfs:comment>OMA-RD-LightweightM2M-V1_0-20170208-A, Label: LightweightM2M-HLF-028</rdfs:comment>
        <rdfs:label xml:lang="en">RadioCellId</rdfs:label>
    </owl:Class>
    


    <!-- http://purl.org/net/iot-dm#OWLClass_6097d2e6_765c_4afb_adf0_729cc96dab8b -->

    <owl:Class rdf:about="http://purl.org/net/iot-dm#OWLClass_6097d2e6_765c_4afb_adf0_729cc96dab8b">
        <rdfs:subClassOf rdf:resource="http://purl.org/net/iot-dm#OWLClass_9d0581a1_1bab_4643_9336_b632fa350e2f"/>
        <rdfs:comment>Recent Advances in Industrial Wireless Sensor Networks Towards Efficient Management in IoT, p. 13</rdfs:comment>
        <rdfs:label xml:lang="en">ProcessMonitoring</rdfs:label>
    </owl:Class>
    


    <!-- http://purl.org/net/iot-dm#OWLClass_6144415a_e463_4ac3_80e3_02fcc4029989 -->

    <owl:Class rdf:about="http://purl.org/net/iot-dm#OWLClass_6144415a_e463_4ac3_80e3_02fcc4029989">
        <rdfs:subClassOf rdf:resource="http://purl.org/net/iot-dm#OWLClass_9706d318_5cd1_4e58_8c3b_72eef36ee70a"/>
        <rdfs:comment>draft-moran-suit-architecture-03 (work in progress), p. 12</rdfs:comment>
        <rdfs:label xml:lang="en">BestBeforeDate</rdfs:label>
    </owl:Class>
    


    <!-- http://purl.org/net/iot-dm#OWLClass_6180ecee_83e6_4cbb_8a64_70437f1dd883 -->

    <owl:Class rdf:about="http://purl.org/net/iot-dm#OWLClass_6180ecee_83e6_4cbb_8a64_70437f1dd883">
        <rdfs:subClassOf rdf:resource="http://purl.org/net/iot-dm#OWLClass_3300e6af_4338_4bf4_ab9e_632af0b5ad65"/>
        <rdfs:comment>OMA-RD-LightweightM2M-V1_1-20180710-A, Label: LightweightM2M-BsR-002</rdfs:comment>
        <rdfs:label xml:lang="en">ClientInitiatedBootstrapModeTriggering</rdfs:label>
    </owl:Class>
    


    <!-- http://purl.org/net/iot-dm#OWLClass_61f9a451_6c61_43bf_a7b9_b953e6a05724 -->

    <owl:Class rdf:about="http://purl.org/net/iot-dm#OWLClass_61f9a451_6c61_43bf_a7b9_b953e6a05724">
        <rdfs:subClassOf rdf:resource="http://purl.org/net/iot-dm#OWLClass_cbca8db6_d106_4651_a12c_b8fe629efbda"/>
        <rdfs:comment>Management of IoT Devices in a Physical Network, p. 487</rdfs:comment>
        <rdfs:label xml:lang="en">UnauthorizedAccessDetectionAndMonitoring</rdfs:label>
    </owl:Class>
    


    <!-- http://purl.org/net/iot-dm#OWLClass_629f62fe_a656_498c_aedb_17b631a536c1 -->

    <owl:Class rdf:about="http://purl.org/net/iot-dm#OWLClass_629f62fe_a656_498c_aedb_17b631a536c1">
        <rdfs:subClassOf rdf:resource="http://purl.org/net/iot-dm#OWLClass_989411ba_e811_4185_bc1f_277d10d81160"/>
        <rdfs:comment>https://resin.io/how-it-works/, 2019-09-16</rdfs:comment>
        <rdfs:label xml:lang="en">Ssh</rdfs:label>
    </owl:Class>
    


    <!-- http://purl.org/net/iot-dm#OWLClass_62fae845_5a8c_4d71_980f_2f8cea75de35 -->

    <owl:Class rdf:about="http://purl.org/net/iot-dm#OWLClass_62fae845_5a8c_4d71_980f_2f8cea75de35">
        <rdfs:subClassOf rdf:resource="http://purl.org/net/iot-dm#OWLClass_f86901a5_61d3_4e5a_8ec6_984ffda5de83"/>
        <rdfs:comment>IoT home gateway for auto-conﬁguration and management of MQTT devices, section III.</rdfs:comment>
        <rdfs:label xml:lang="en">DeviceControlMessageTranslation</rdfs:label>
    </owl:Class>
    


    <!-- http://purl.org/net/iot-dm#OWLClass_63057798_6c27_4642_9ffc_9e5b09529dd2 -->

    <owl:Class rdf:about="http://purl.org/net/iot-dm#OWLClass_63057798_6c27_4642_9ffc_9e5b09529dd2">
        <rdfs:subClassOf rdf:resource="http://purl.org/net/iot-dm#OWLClass_391c8c1f_1c6c_400e_94eb_7b7dc8d02ddb"/>
        <rdfs:label xml:lang="en">NetworkingPreconfiguration</rdfs:label>
    </owl:Class>
    


    <!-- http://purl.org/net/iot-dm#OWLClass_63ca1431_e88a_4323_a5fd_4c5b7c041c9e -->

    <owl:Class rdf:about="http://purl.org/net/iot-dm#OWLClass_63ca1431_e88a_4323_a5fd_4c5b7c041c9e">
        <rdfs:subClassOf rdf:resource="http://purl.org/net/iot-dm#OWLClass_66c3fc69_337f_4795_a467_f0b64b90cb3b"/>
        <rdfs:comment>Recent Advances in Industrial Wireless Sensor Networks Towards Efficient Management in IoT, p. 13</rdfs:comment>
        <rdfs:label xml:lang="en">Trust</rdfs:label>
    </owl:Class>
    


    <!-- http://purl.org/net/iot-dm#OWLClass_6401126c_9648_4650_8d8e_79c426dd575e -->

    <owl:Class rdf:about="http://purl.org/net/iot-dm#OWLClass_6401126c_9648_4650_8d8e_79c426dd575e">
        <rdfs:subClassOf rdf:resource="http://purl.org/net/iot-dm#OWLClass_2c177064_e630_44da_bbb3_d692886a8e4a"/>
        <rdfs:comment>OMA-RD-LightweightM2M-V1_1-20180710-A, Label: LightweightM2M-BsR-006</rdfs:comment>
        <rdfs:label xml:lang="en">BootstrappingPreconditionDetermination</rdfs:label>
    </owl:Class>
    


    <!-- http://purl.org/net/iot-dm#OWLClass_645a8b53_bb59_48a7_a3e4_e66874f1e93a -->

    <owl:Class rdf:about="http://purl.org/net/iot-dm#OWLClass_645a8b53_bb59_48a7_a3e4_e66874f1e93a">
        <rdfs:subClassOf rdf:resource="http://purl.org/net/iot-dm#OWLClass_3e781bea_1637_4984_bf63_8935b4e49e16"/>
        <rdfs:comment>OMA-RD-LightweightM2M-V1_0-20170208-A, Label: LightweightM2M-HLF-019</rdfs:comment>
        <rdfs:label xml:lang="en">PeriodicResourceReportingMechanism</rdfs:label>
    </owl:Class>
    


    <!-- http://purl.org/net/iot-dm#OWLClass_64c0c545_2d62_4a61_ac06_9c832a2e4708 -->

    <owl:Class rdf:about="http://purl.org/net/iot-dm#OWLClass_64c0c545_2d62_4a61_ac06_9c832a2e4708">
        <rdfs:subClassOf rdf:resource="http://purl.org/net/iot-dm#OWLClass_b6721ba6_4ea5_4be0_b34f_ff739be47358"/>
        <rdfs:comment xml:lang="en">draft-moran-suit-architecture-03 (work in progress), p. 6</rdfs:comment>
        <rdfs:label xml:lang="en">RollbackAttackPrevention</rdfs:label>
    </owl:Class>
    


    <!-- http://purl.org/net/iot-dm#OWLClass_64df463c_d105_497a_8a42_0a003352ad6d -->

    <owl:Class rdf:about="http://purl.org/net/iot-dm#OWLClass_64df463c_d105_497a_8a42_0a003352ad6d">
        <rdfs:subClassOf rdf:resource="http://purl.org/net/iot-dm#OWLClass_d8e49365_06e1_40c2_99fc_891f2256aad1"/>
        <rdfs:comment>IoT home gateway for auto-conﬁguration and management of MQTT devices, section I.</rdfs:comment>
        <rdfs:label xml:lang="en">Dpws</rdfs:label>
    </owl:Class>
    


    <!-- http://purl.org/net/iot-dm#OWLClass_66c3fc69_337f_4795_a467_f0b64b90cb3b -->

    <owl:Class rdf:about="http://purl.org/net/iot-dm#OWLClass_66c3fc69_337f_4795_a467_f0b64b90cb3b">
        <rdfs:subClassOf rdf:resource="http://purl.org/net/iot-dm#OWLClass_b21422b7_b049_4b16_b3e0_53d1c9d53e85"/>
        <rdfs:label xml:lang="en">NonFunctional</rdfs:label>
    </owl:Class>
    


    <!-- http://purl.org/net/iot-dm#OWLClass_6783e7e3_bc50_49de_8d69_4e137eec977b -->

    <owl:Class rdf:about="http://purl.org/net/iot-dm#OWLClass_6783e7e3_bc50_49de_8d69_4e137eec977b">
        <rdfs:subClassOf rdf:resource="http://purl.org/net/iot-dm#OWLClass_a18f091d_134e_4059_ada6_9695459aa5f6"/>
        <rdfs:label xml:lang="en">SecureDeviceCommunication</rdfs:label>
    </owl:Class>
    


    <!-- http://purl.org/net/iot-dm#OWLClass_679e1f1b_68ba_4f57_924f_2e3ac97255da -->

    <owl:Class rdf:about="http://purl.org/net/iot-dm#OWLClass_679e1f1b_68ba_4f57_924f_2e3ac97255da">
        <rdfs:subClassOf rdf:resource="http://purl.org/net/iot-dm#OWLClass_c74a5982_d5bc_40b3_9e18_c03e025b5949"/>
        <rdfs:comment>draft-moran-suit-architecture-03 (work in progress), p. 7</rdfs:comment>
        <rdfs:label xml:lang="en">RecoveryMechanism</rdfs:label>
    </owl:Class>
    


    <!-- http://purl.org/net/iot-dm#OWLClass_67b38741_3bca_4859_8ea9_d5d9d7aecbff -->

    <owl:Class rdf:about="http://purl.org/net/iot-dm#OWLClass_67b38741_3bca_4859_8ea9_d5d9d7aecbff">
        <rdfs:subClassOf rdf:resource="http://purl.org/net/iot-dm#OWLClass_91e1d636_17c7_43c3_ab32_ce7700226d44"/>
        <rdfs:comment>OMA-RD-LightweightM2M-V1_1-20180710-A, Label: LightweightM2M-PKI-002</rdfs:comment>
        <rdfs:label xml:lang="en">TimeInformationInitialization</rdfs:label>
    </owl:Class>
    


    <!-- http://purl.org/net/iot-dm#OWLClass_683fab4d_9f26_4338_a3f0_86e30b859e13 -->

    <owl:Class rdf:about="http://purl.org/net/iot-dm#OWLClass_683fab4d_9f26_4338_a3f0_86e30b859e13">
        <rdfs:subClassOf rdf:resource="http://purl.org/net/iot-dm#OWLClass_843d87bc_a343_470f_bff0_872b15b14c16"/>
        <rdfs:comment>OMA-RD-LightweightM2M-V1_0-20170208-A, Label: LightweightM2M-HLF-005</rdfs:comment>
        <rdfs:label xml:lang="en">FirmwareUpdateResultIndication</rdfs:label>
    </owl:Class>
    


    <!-- http://purl.org/net/iot-dm#OWLClass_68e5a285_5ba6_4cb1_85e7_ac792a46c65f -->

    <owl:Class rdf:about="http://purl.org/net/iot-dm#OWLClass_68e5a285_5ba6_4cb1_85e7_ac792a46c65f">
        <rdfs:subClassOf rdf:resource="http://purl.org/net/iot-dm#OWLClass_5fc8a8e2_e2d0_4920_af45_b6393b5ed989"/>
        <rdfs:comment>Management of IoT Devices in a Physical Network, p. 488</rdfs:comment>
        <rdfs:label xml:lang="en">DeviceOntology</rdfs:label>
    </owl:Class>
    


    <!-- http://purl.org/net/iot-dm#OWLClass_69034fb8_1114_422f_b34b_2c884813d6eb -->

    <owl:Class rdf:about="http://purl.org/net/iot-dm#OWLClass_69034fb8_1114_422f_b34b_2c884813d6eb">
        <rdfs:subClassOf rdf:resource="http://purl.org/net/iot-dm#OWLClass_ffcb0dd3_5746_4e9b_9905_50bfb9faff34"/>
        <rdfs:comment>OMA-RD-LightweightM2M-V1_0-20170208-A, Label: LightweightM2M-HLF-016</rdfs:comment>
        <rdfs:label xml:lang="en">SessionBasedCommunication</rdfs:label>
    </owl:Class>
    


    <!-- http://purl.org/net/iot-dm#OWLClass_698bc07c_d088_45cb_a213_e564e199ab3e -->

    <owl:Class rdf:about="http://purl.org/net/iot-dm#OWLClass_698bc07c_d088_45cb_a213_e564e199ab3e">
        <rdfs:subClassOf rdf:resource="http://purl.org/net/iot-dm#OWLClass_755c484b_7249_4f24_81fb_2d9ac5948eab"/>
        <rdfs:comment>OMA-RD-LightweightM2M-V1_0-20170208-A, Label: LightweightM2M-HLF-032</rdfs:comment>
        <rdfs:label xml:lang="en">ReadWrite</rdfs:label>
    </owl:Class>
    


    <!-- http://purl.org/net/iot-dm#OWLClass_69b61702_f9bd_42e9_a966_7599a9404867 -->

    <owl:Class rdf:about="http://purl.org/net/iot-dm#OWLClass_69b61702_f9bd_42e9_a966_7599a9404867">
        <rdfs:subClassOf rdf:resource="http://purl.org/net/iot-dm#OWLClass_3e69999a_c294_423f_92bc_6a665a91a72e"/>
        <rdfs:comment>OMA-RD-LightweightM2M-V1_1-20180710-A, Label: LightweightM2M-ENC-3</rdfs:comment>
        <rdfs:label xml:lang="en">StandardizedDataFormat</rdfs:label>
    </owl:Class>
    


    <!-- http://purl.org/net/iot-dm#OWLClass_6a861511_ae7e_429b_aa27_b5378544b99e -->

    <owl:Class rdf:about="http://purl.org/net/iot-dm#OWLClass_6a861511_ae7e_429b_aa27_b5378544b99e">
        <rdfs:subClassOf rdf:resource="http://purl.org/net/iot-dm#OWLClass_e68b7577_38f1_497e_8b5c_229be057d711"/>
        <rdfs:comment>https://resin.io/features/, 2018-09-15</rdfs:comment>
        <rdfs:label xml:lang="en">ProvidedDeviceName</rdfs:label>
    </owl:Class>
    


    <!-- http://purl.org/net/iot-dm#OWLClass_6c28e358_b8d8_4bd2_81e9_21b2d308b2a8 -->

    <owl:Class rdf:about="http://purl.org/net/iot-dm#OWLClass_6c28e358_b8d8_4bd2_81e9_21b2d308b2a8">
        <rdfs:subClassOf rdf:resource="http://purl.org/net/iot-dm#OWLClass_843d87bc_a343_470f_bff0_872b15b14c16"/>
        <rdfs:label xml:lang="en">MassUpdates</rdfs:label>
    </owl:Class>
    


    <!-- http://purl.org/net/iot-dm#OWLClass_6c880a72_9e64_487c_96fd_37a321cb1838 -->

    <owl:Class rdf:about="http://purl.org/net/iot-dm#OWLClass_6c880a72_9e64_487c_96fd_37a321cb1838">
        <rdfs:subClassOf rdf:resource="http://purl.org/net/iot-dm#OWLClass_1543e022_678c_4b10_9895_de120d944f03"/>
        <rdfs:comment>IoT home gateway for auto-conﬁguration and management of MQTT devices, section III.</rdfs:comment>
        <rdfs:label xml:lang="en">DeviceStatusChangeMessage</rdfs:label>
    </owl:Class>
    


    <!-- http://purl.org/net/iot-dm#OWLClass_6cb818a3_6278_4bad_8a6b_c01ee623c677 -->

    <owl:Class rdf:about="http://purl.org/net/iot-dm#OWLClass_6cb818a3_6278_4bad_8a6b_c01ee623c677">
        <rdfs:subClassOf rdf:resource="http://purl.org/net/iot-dm#OWLClass_2281b85a_ace5_4ac3_910f_536f7370505e"/>
        <rdfs:label xml:lang="en">RemoteDeviceControl</rdfs:label>
    </owl:Class>
    


    <!-- http://purl.org/net/iot-dm#OWLClass_6dbd00cf_8e98_4cc0_812b_960bd34dc6e4 -->

    <owl:Class rdf:about="http://purl.org/net/iot-dm#OWLClass_6dbd00cf_8e98_4cc0_812b_960bd34dc6e4">
        <rdfs:subClassOf rdf:resource="http://purl.org/net/iot-dm#OWLClass_515bf129_124c_4413_9e49_8de009d76986"/>
        <rdfs:comment>Management of IoT Devices in a Physical Network, p. 488</rdfs:comment>
        <rdfs:label xml:lang="en">UnitOfMeasure</rdfs:label>
    </owl:Class>
    


    <!-- http://purl.org/net/iot-dm#OWLClass_6ee17bd2_bce5_4451_acf5_892cf55ad27b -->

    <owl:Class rdf:about="http://purl.org/net/iot-dm#OWLClass_6ee17bd2_bce5_4451_acf5_892cf55ad27b">
        <rdfs:subClassOf rdf:resource="http://purl.org/net/iot-dm#OWLClass_c8340585_9c41_4f98_8f90_b4e2436e8829"/>
        <rdfs:comment>OMA-RD-LightweightM2M-V1_1-20180710-A, Label: LightweightM2M-LPW-6</rdfs:comment>
        <rdfs:label xml:lang="en">PerDeviceRateAndByteQuota</rdfs:label>
    </owl:Class>
    


    <!-- http://purl.org/net/iot-dm#OWLClass_6f8197a0_9425_4239_bea9_7e354c8cba24 -->

    <owl:Class rdf:about="http://purl.org/net/iot-dm#OWLClass_6f8197a0_9425_4239_bea9_7e354c8cba24">
        <rdfs:subClassOf rdf:resource="http://purl.org/net/iot-dm#OWLClass_ae34f5cf_8888_4de3_9170_7e8f6eab5f86"/>
        <rdfs:comment>https://resin.io/how-it-works/, 2018-09-16</rdfs:comment>
        <rdfs:label xml:lang="en">ContainerUpdate</rdfs:label>
    </owl:Class>
    


    <!-- http://purl.org/net/iot-dm#OWLClass_6ff26810_f417_457e_90e7_f7187268ec90 -->

    <owl:Class rdf:about="http://purl.org/net/iot-dm#OWLClass_6ff26810_f417_457e_90e7_f7187268ec90">
        <rdfs:subClassOf rdf:resource="http://purl.org/net/iot-dm#OWLClass_2fb332cc_9b13_4fbc_af07_4ce1a662e062"/>
        <rdfs:comment>https://resin.io/features/, 2018-09-15</rdfs:comment>
        <rdfs:label xml:lang="en">DeviceLogs</rdfs:label>
    </owl:Class>
    


    <!-- http://purl.org/net/iot-dm#OWLClass_70551cc2_7de8_4f8d_afea_e8657644845f -->

    <owl:Class rdf:about="http://purl.org/net/iot-dm#OWLClass_70551cc2_7de8_4f8d_afea_e8657644845f">
        <rdfs:subClassOf rdf:resource="http://purl.org/net/iot-dm#OWLClass_195de59b_34c2_45da_8aa8_591cd3847fc7"/>
        <rdfs:comment>OMA-RD-LightweightM2M-V1_1-20180710-A, Label: LightweightM2M-E2E-1</rdfs:comment>
        <rdfs:comment>OMA-RD-LightweightM2M-V1_1-20180710-A, Label: LightweightM2M-E2E-7</rdfs:comment>
        <rdfs:comment>OMA-RD-LightweightM2M-V1_1-20180710-A, Label: LightweightM2M-E2Eo-1</rdfs:comment>
        <rdfs:comment>OMA-RD-LightweightM2M-V1_1-20180710-A, Label: LightweightM2M-E2Eo-7</rdfs:comment>
        <rdfs:label xml:lang="en">Integrity</rdfs:label>
    </owl:Class>
    


    <!-- http://purl.org/net/iot-dm#OWLClass_71dcf03b_6cc1_4da4_9574_874b4477d105 -->

    <owl:Class rdf:about="http://purl.org/net/iot-dm#OWLClass_71dcf03b_6cc1_4da4_9574_874b4477d105">
        <rdfs:subClassOf rdf:resource="http://purl.org/net/iot-dm#OWLClass_267278cd_85b2_4704_84d7_a7cb4004d16d"/>
        <rdfs:label xml:lang="en">ContainerBasedApplicationManagment</rdfs:label>
    </owl:Class>
    


    <!-- http://purl.org/net/iot-dm#OWLClass_72335bc0_8df9_4e9f_96a7_ba4aaeaff99b -->

    <owl:Class rdf:about="http://purl.org/net/iot-dm#OWLClass_72335bc0_8df9_4e9f_96a7_ba4aaeaff99b">
        <rdfs:subClassOf rdf:resource="http://purl.org/net/iot-dm#OWLClass_42d9f56b_27ca_411a_8c4f_91ecb085e413"/>
        <rdfs:comment>OMA-RD-LightweightM2M-V1_1-20180710-A, Label: LightweightM2M-TLS-001</rdfs:comment>
        <rdfs:label xml:lang="en">TlsDtlsSupportOverVariousTransportBindings</rdfs:label>
    </owl:Class>
    


    <!-- http://purl.org/net/iot-dm#OWLClass_72dc5ecb_db1f_475d_bd80_0e7d6d1e1c56 -->

    <owl:Class rdf:about="http://purl.org/net/iot-dm#OWLClass_72dc5ecb_db1f_475d_bd80_0e7d6d1e1c56">
        <rdfs:subClassOf rdf:resource="http://purl.org/net/iot-dm#OWLClass_213b255b_d2a6_41ac_9e58_75311a7288f3"/>
        <rdfs:comment>Ontologies for the Internet of Things, 2.</rdfs:comment>
        <rdfs:label xml:lang="en">ErrorCharacteristics</rdfs:label>
    </owl:Class>
    


    <!-- http://purl.org/net/iot-dm#OWLClass_72f7af0a_2f54_4917_8f5b_506328e7b603 -->

    <owl:Class rdf:about="http://purl.org/net/iot-dm#OWLClass_72f7af0a_2f54_4917_8f5b_506328e7b603">
        <rdfs:subClassOf rdf:resource="http://purl.org/net/iot-dm#OWLClass_869abf01_eaf3_41bc_95ed_6a11d4959818"/>
        <rdfs:comment>draft-moran-suit-architecture-03 (work in progress), p. 7</rdfs:comment>
        <rdfs:label xml:lang="en">TwoStageBootloader</rdfs:label>
    </owl:Class>
    


    <!-- http://purl.org/net/iot-dm#OWLClass_7342b5ca_517a_4a8f_bb63_cd633d02bb65 -->

    <owl:Class rdf:about="http://purl.org/net/iot-dm#OWLClass_7342b5ca_517a_4a8f_bb63_cd633d02bb65">
        <rdfs:subClassOf rdf:resource="http://purl.org/net/iot-dm#OWLClass_c74a5982_d5bc_40b3_9e18_c03e025b5949"/>
        <rdfs:comment>draft-moran-suit-architecture-03 (work in progress), p. 7</rdfs:comment>
        <rdfs:label xml:lang="en">CryptographicPrimitives</rdfs:label>
    </owl:Class>
    


    <!-- http://purl.org/net/iot-dm#OWLClass_749421de_be9b_4633_b63b_302dc8e546ff -->

    <owl:Class rdf:about="http://purl.org/net/iot-dm#OWLClass_749421de_be9b_4633_b63b_302dc8e546ff">
        <rdfs:subClassOf rdf:resource="http://purl.org/net/iot-dm#OWLClass_4c69f2df_35c9_4bf1_8b7f_b0e8fcac7aca"/>
        <rdfs:comment>draft-moran-suit-architecture-03 (work in progress), p. 6</rdfs:comment>
        <rdfs:label xml:lang="en">PowerFailure</rdfs:label>
    </owl:Class>
    


    <!-- http://purl.org/net/iot-dm#OWLClass_74bba417_5316_4b3f_b7d2_9fb2a118db2f -->

    <owl:Class rdf:about="http://purl.org/net/iot-dm#OWLClass_74bba417_5316_4b3f_b7d2_9fb2a118db2f">
        <rdfs:subClassOf rdf:resource="http://purl.org/net/iot-dm#OWLClass_66c3fc69_337f_4795_a467_f0b64b90cb3b"/>
        <rdfs:label xml:lang="en">Confidentiality</rdfs:label>
    </owl:Class>
    


    <!-- http://purl.org/net/iot-dm#OWLClass_755c484b_7249_4f24_81fb_2d9ac5948eab -->

    <owl:Class rdf:about="http://purl.org/net/iot-dm#OWLClass_755c484b_7249_4f24_81fb_2d9ac5948eab">
        <rdfs:subClassOf rdf:resource="http://purl.org/net/iot-dm#OWLClass_5c08eefa_8244_4272_b68c_6f24666eb49d"/>
        <rdfs:comment>OMA-RD-LightweightM2M-V1_0-20170208-A, Label: LightweightM2M-HLF-032</rdfs:comment>
        <rdfs:label xml:lang="en">ResourceAccessControl</rdfs:label>
    </owl:Class>
    


    <!-- http://purl.org/net/iot-dm#OWLClass_75c6328f_52a3_4d5f_becc_ca0e07757ed6 -->

    <owl:Class rdf:about="http://purl.org/net/iot-dm#OWLClass_75c6328f_52a3_4d5f_becc_ca0e07757ed6">
        <rdfs:subClassOf rdf:resource="http://purl.org/net/iot-dm#OWLClass_9706d318_5cd1_4e58_8c3b_72eef36ee70a"/>
        <rdfs:comment>draft-moran-suit-architecture-03 (work in progress), p. 12</rdfs:comment>
        <rdfs:label xml:lang="en">IntendedDevicesForApplication</rdfs:label>
    </owl:Class>
    


    <!-- http://purl.org/net/iot-dm#OWLClass_77093e6d_5bcf_4317_aedc_a07046a659aa -->

    <owl:Class rdf:about="http://purl.org/net/iot-dm#OWLClass_77093e6d_5bcf_4317_aedc_a07046a659aa">
        <rdfs:subClassOf rdf:resource="http://purl.org/net/iot-dm#OWLClass_66c3fc69_337f_4795_a467_f0b64b90cb3b"/>
        <rdfs:label xml:lang="en">Authorization</rdfs:label>
    </owl:Class>
    


    <!-- http://purl.org/net/iot-dm#OWLClass_774b5f3e_c378_4bfa_8bb7_2a9c4fd4190b -->

    <owl:Class rdf:about="http://purl.org/net/iot-dm#OWLClass_774b5f3e_c378_4bfa_8bb7_2a9c4fd4190b">
        <rdfs:subClassOf rdf:resource="http://purl.org/net/iot-dm#OWLClass_755c484b_7249_4f24_81fb_2d9ac5948eab"/>
        <rdfs:comment>OMA-RD-LightweightM2M-V1_0-20170208-A, Label: LightweightM2M-HLF-032</rdfs:comment>
        <rdfs:label xml:lang="en">ReadOnly</rdfs:label>
    </owl:Class>
    


    <!-- http://purl.org/net/iot-dm#OWLClass_774c7acb_c17d_4e26_8afc_75f16a0910c5 -->

    <owl:Class rdf:about="http://purl.org/net/iot-dm#OWLClass_774c7acb_c17d_4e26_8afc_75f16a0910c5">
        <rdfs:subClassOf rdf:resource="http://purl.org/net/iot-dm#OWLClass_6ff26810_f417_457e_90e7_f7187268ec90"/>
        <rdfs:label xml:lang="en">LogMonitoringTools</rdfs:label>
    </owl:Class>
    


    <!-- http://purl.org/net/iot-dm#OWLClass_77a107a3_4ca0_4ca4_bc4d_65a90d131824 -->

    <owl:Class rdf:about="http://purl.org/net/iot-dm#OWLClass_77a107a3_4ca0_4ca4_bc4d_65a90d131824">
        <rdfs:subClassOf rdf:resource="http://purl.org/net/iot-dm#OWLClass_80cdf1ca_1960_443d_abdb_8842cae1f466"/>
        <rdfs:comment>OMA-RD-LightweightM2M-V1_1-20180710-A, Label: LightweightM2M-MaU-3</rdfs:comment>
        <rdfs:label xml:lang="en">BringBackSavedDeviceSettingsAfterFirmwareUpgrade</rdfs:label>
    </owl:Class>
    


    <!-- http://purl.org/net/iot-dm#OWLClass_781f6c56_e24b_4fc7_9ae7_455aa2a4ec60 -->

    <owl:Class rdf:about="http://purl.org/net/iot-dm#OWLClass_781f6c56_e24b_4fc7_9ae7_455aa2a4ec60">
        <rdfs:subClassOf rdf:resource="http://purl.org/net/iot-dm#OWLClass_ffcb0dd3_5746_4e9b_9905_50bfb9faff34"/>
        <rdfs:comment>OMA-RD-LightweightM2M-V1_0-20170208-A, Label: LightweightM2M-HLF-014</rdfs:comment>
        <rdfs:label xml:lang="en">IpBasedCommunication</rdfs:label>
    </owl:Class>
    


    <!-- http://purl.org/net/iot-dm#OWLClass_7860c554_e01a_4475_aca9_f00705849c9d -->

    <owl:Class rdf:about="http://purl.org/net/iot-dm#OWLClass_7860c554_e01a_4475_aca9_f00705849c9d">
        <rdfs:subClassOf rdf:resource="http://purl.org/net/iot-dm#OWLClass_cfc68839_b898_454c_9314_0822698917f2"/>
        <rdfs:comment>https://resin.io/how-it-works/, 2019-09-16</rdfs:comment>
        <rdfs:label xml:lang="en">OperatingSystemVersion</rdfs:label>
    </owl:Class>
    


    <!-- http://purl.org/net/iot-dm#OWLClass_794b6e93_f7ec_4b06_8f74_fe96709e33a2 -->

    <owl:Class rdf:about="http://purl.org/net/iot-dm#OWLClass_794b6e93_f7ec_4b06_8f74_fe96709e33a2">
        <rdfs:subClassOf rdf:resource="http://purl.org/net/iot-dm#OWLClass_9d0581a1_1bab_4643_9336_b632fa350e2f"/>
        <rdfs:comment>https://resin.io/how-it-works/, 2018-09-16</rdfs:comment>
        <rdfs:label xml:lang="en">ServiceMonitoring</rdfs:label>
    </owl:Class>
    


    <!-- http://purl.org/net/iot-dm#OWLClass_7a42bb23_408d_438d_9e91_c2ab809aff6d -->

    <owl:Class rdf:about="http://purl.org/net/iot-dm#OWLClass_7a42bb23_408d_438d_9e91_c2ab809aff6d">
        <rdfs:subClassOf rdf:resource="http://purl.org/net/iot-dm#OWLClass_9fcb5dc3_b98f_464b_ad5b_3b1b47050d11"/>
        <rdfs:comment>Recent Advances in Industrial Wireless Sensor Networks Towards Efficient Management in IoT, p. 9</rdfs:comment>
        <rdfs:label xml:lang="en">RemoteControl</rdfs:label>
    </owl:Class>
    


    <!-- http://purl.org/net/iot-dm#OWLClass_7ab62ac7_c17f_4f51_a14b_cac41106ad38 -->

    <owl:Class rdf:about="http://purl.org/net/iot-dm#OWLClass_7ab62ac7_c17f_4f51_a14b_cac41106ad38">
        <rdfs:subClassOf rdf:resource="http://purl.org/net/iot-dm#OWLClass_3e781bea_1637_4984_bf63_8935b4e49e16"/>
        <rdfs:comment>OMA-RD-LightweightM2M-V1_0-20170208-A, Label: LightweightM2M-HLF-020</rdfs:comment>
        <rdfs:label xml:lang="en">EventTriggerReportingMechanism</rdfs:label>
    </owl:Class>
    


    <!-- http://purl.org/net/iot-dm#OWLClass_7abbfbf0_1913_4412_b2ef_39bc779ff6b0 -->

    <owl:Class rdf:about="http://purl.org/net/iot-dm#OWLClass_7abbfbf0_1913_4412_b2ef_39bc779ff6b0">
        <rdfs:subClassOf rdf:resource="http://purl.org/net/iot-dm#OWLClass_5303cc63_d095_4c30_b893_51cfe691cb7e"/>
        <rdfs:comment>OMA-RD-LightweightM2M-V1_0-20170208-A, Label: LightweightM2M-HLF-018</rdfs:comment>
        <rdfs:label xml:lang="en">PowerSavingModeConfiguration</rdfs:label>
    </owl:Class>
    


    <!-- http://purl.org/net/iot-dm#OWLClass_7ad0de06_bf2c_48e8_8f51_f7b782f0aa04 -->

    <owl:Class rdf:about="http://purl.org/net/iot-dm#OWLClass_7ad0de06_bf2c_48e8_8f51_f7b782f0aa04">
        <rdfs:subClassOf rdf:resource="http://purl.org/net/iot-dm#OWLClass_21fa4e78_3300_43d8_83c7_78d9ee314b79"/>
        <rdfs:label xml:lang="en">SingleResourcePerRequest</rdfs:label>
    </owl:Class>
    


    <!-- http://purl.org/net/iot-dm#OWLClass_7ad7ced8_90c7_430c_be99_6cc4328aef1a -->

    <owl:Class rdf:about="http://purl.org/net/iot-dm#OWLClass_7ad7ced8_90c7_430c_be99_6cc4328aef1a">
        <rdfs:subClassOf rdf:resource="http://purl.org/net/iot-dm#OWLClass_f519e17a_515d_402f_a5da_1cffe41727ea"/>
        <rdfs:comment>IoT home gateway for auto-conﬁguration and management of MQTT devices, section III.</rdfs:comment>
        <rdfs:label xml:lang="en">NonIpBased</rdfs:label>
    </owl:Class>
    


    <!-- http://purl.org/net/iot-dm#OWLClass_7b141ed0_5648_4402_8f34_8078c00b8ee7 -->

    <owl:Class rdf:about="http://purl.org/net/iot-dm#OWLClass_7b141ed0_5648_4402_8f34_8078c00b8ee7">
        <rdfs:subClassOf rdf:resource="http://purl.org/net/iot-dm#OWLClass_56ca2f5d_d065_4fe0_bfd8_9c86ea85f200"/>
        <rdfs:comment>Ontologies for the Internet of Things, 2.</rdfs:comment>
        <rdfs:label xml:lang="en">MissingDataPointEstimation</rdfs:label>
    </owl:Class>
    


    <!-- http://purl.org/net/iot-dm#OWLClass_7c2176c4_6101_411a_8a88_a0bf08b9399c -->

    <owl:Class rdf:about="http://purl.org/net/iot-dm#OWLClass_7c2176c4_6101_411a_8a88_a0bf08b9399c">
        <rdfs:subClassOf rdf:resource="http://purl.org/net/iot-dm#OWLClass_1d7dd666_95ba_4c41_9a91_d850e9c0f479"/>
        <rdfs:comment>OMA-RD-LightweightM2M-V1_1-20180710-A, Label: LightweightM2M-ENC-1</rdfs:comment>
        <rdfs:label xml:lang="en">CompactDataFormat</rdfs:label>
    </owl:Class>
    


    <!-- http://purl.org/net/iot-dm#OWLClass_7c8282da_3443_4c49_a838_df6cb9a459c9 -->

    <owl:Class rdf:about="http://purl.org/net/iot-dm#OWLClass_7c8282da_3443_4c49_a838_df6cb9a459c9">
        <rdfs:subClassOf rdf:resource="http://purl.org/net/iot-dm#OWLClass_b6721ba6_4ea5_4be0_b34f_ff739be47358"/>
        <rdfs:label xml:lang="en">ReliableUpdateMechanism</rdfs:label>
    </owl:Class>
    


    <!-- http://purl.org/net/iot-dm#OWLClass_7ed5a132_c15b_486f_91f4_ad5eb4433cef -->

    <owl:Class rdf:about="http://purl.org/net/iot-dm#OWLClass_7ed5a132_c15b_486f_91f4_ad5eb4433cef">
        <rdfs:subClassOf rdf:resource="http://purl.org/net/iot-dm#OWLClass_201d2207_e63c_4bd0_ac8e_dac6fd8b7d61"/>
        <rdfs:comment>Recent Advances in Industrial Wireless Sensor Networks Towards Efficient Management in IoT, p. 1</rdfs:comment>
        <rdfs:label xml:lang="en">FirmwareUpdateManagement</rdfs:label>
        <rdfs:seeAlso>FirmwareUpgradeManagement</rdfs:seeAlso>
    </owl:Class>
    


    <!-- http://purl.org/net/iot-dm#OWLClass_808d7fbb_8678_46ad_a137_a3811cd7dfc8 -->

    <owl:Class rdf:about="http://purl.org/net/iot-dm#OWLClass_808d7fbb_8678_46ad_a137_a3811cd7dfc8">
        <rdfs:subClassOf rdf:resource="http://purl.org/net/iot-dm#OWLClass_e7e81967_1b1b_4dfb_b9b6_c40e0ffab441"/>
        <rdfs:comment>OMA-RD-LightweightM2M-V1_0-20170208-A, Label: LightweightM2M-SEC-002</rdfs:comment>
        <rdfs:label xml:lang="en">ReplayAttackPrevention</rdfs:label>
    </owl:Class>
    


    <!-- http://purl.org/net/iot-dm#OWLClass_80cdf1ca_1960_443d_abdb_8842cae1f466 -->

    <owl:Class rdf:about="http://purl.org/net/iot-dm#OWLClass_80cdf1ca_1960_443d_abdb_8842cae1f466">
        <rdfs:subClassOf rdf:resource="http://purl.org/net/iot-dm#OWLClass_843d87bc_a343_470f_bff0_872b15b14c16"/>
        <rdfs:label xml:lang="en">DeviceSettings</rdfs:label>
    </owl:Class>
    


    <!-- http://purl.org/net/iot-dm#OWLClass_81e411c6_43af_4e07_9341_d53659bfbb91 -->

    <owl:Class rdf:about="http://purl.org/net/iot-dm#OWLClass_81e411c6_43af_4e07_9341_d53659bfbb91">
        <rdfs:subClassOf rdf:resource="http://purl.org/net/iot-dm#OWLClass_68e5a285_5ba6_4cb1_85e7_ac792a46c65f"/>
        <rdfs:comment>Management of IoT Devices in a Physical Network, p. 490</rdfs:comment>
        <rdfs:label xml:lang="en">InitialDeviceSetupRequirements</rdfs:label>
    </owl:Class>
    


    <!-- http://purl.org/net/iot-dm#OWLClass_829a4147_2a1d_44ea_a9ef_0efaae5eaa5b -->

    <owl:Class rdf:about="http://purl.org/net/iot-dm#OWLClass_829a4147_2a1d_44ea_a9ef_0efaae5eaa5b">
        <rdfs:subClassOf rdf:resource="http://purl.org/net/iot-dm#OWLClass_47c759b6_e09c_4798_9056_f499ebeecae4"/>
        <rdfs:label xml:lang="en">Restful</rdfs:label>
    </owl:Class>
    


    <!-- http://purl.org/net/iot-dm#OWLClass_8389ec5b_7331_4069_8de0_92e9994d81ee -->

    <owl:Class rdf:about="http://purl.org/net/iot-dm#OWLClass_8389ec5b_7331_4069_8de0_92e9994d81ee">
        <rdfs:subClassOf rdf:resource="http://purl.org/net/iot-dm#OWLClass_11ab1b8e_e60f_4b34_bd83_50a77595a516"/>
        <rdfs:comment xml:lang="en">draft-moran-suit-architecture-03 (work in progress), p. 9</rdfs:comment>
        <rdfs:label xml:lang="en">FetchByDevice</rdfs:label>
    </owl:Class>
    


    <!-- http://purl.org/net/iot-dm#OWLClass_83a75814_662d_468a_bb24_dba5318a80ae -->

    <owl:Class rdf:about="http://purl.org/net/iot-dm#OWLClass_83a75814_662d_468a_bb24_dba5318a80ae">
        <rdfs:subClassOf rdf:resource="http://purl.org/net/iot-dm#OWLClass_9e3d4f19_96c7_4932_a007_26fa592f3423"/>
        <rdfs:comment>IoT home gateway for auto-conﬁguration and management of MQTT devices, section III.</rdfs:comment>
        <rdfs:label xml:lang="en">AutoConfiguration</rdfs:label>
    </owl:Class>
    


    <!-- http://purl.org/net/iot-dm#OWLClass_8420db7e_6cbf_4959_ac1b_39fdae9da0b3 -->

    <owl:Class rdf:about="http://purl.org/net/iot-dm#OWLClass_8420db7e_6cbf_4959_ac1b_39fdae9da0b3">
        <rdfs:subClassOf rdf:resource="http://purl.org/net/iot-dm#OWLClass_a18f091d_134e_4059_ada6_9695459aa5f6"/>
        <rdfs:label xml:lang="en">AccessToLocalDeviceData</rdfs:label>
    </owl:Class>
    


    <!-- http://purl.org/net/iot-dm#OWLClass_843d87bc_a343_470f_bff0_872b15b14c16 -->

    <owl:Class rdf:about="http://purl.org/net/iot-dm#OWLClass_843d87bc_a343_470f_bff0_872b15b14c16">
        <rdfs:subClassOf rdf:resource="http://purl.org/net/iot-dm#OWLClass_7ed5a132_c15b_486f_91f4_ad5eb4433cef"/>
        <rdfs:comment>OMA-RD-LightweightM2M-V1_0-20170208-A, Label: LightweightM2M-HLF-004</rdfs:comment>
        <rdfs:label xml:lang="en">FirmwareUpdateMechanism</rdfs:label>
        <rdfs:seeAlso>FirmwareUpgradeMechanism</rdfs:seeAlso>
    </owl:Class>
    


    <!-- http://purl.org/net/iot-dm#OWLClass_84497e4c_1cfe_4d3f_b1ba_e6304c70216c -->

    <owl:Class rdf:about="http://purl.org/net/iot-dm#OWLClass_84497e4c_1cfe_4d3f_b1ba_e6304c70216c">
        <rdfs:subClassOf rdf:resource="http://purl.org/net/iot-dm#OWLClass_928a3dbe_0ae6_42b7_a752_d48930d19fae"/>
        <rdfs:comment>OMA-RD-LightweightM2M-V1_1-20180710-A, Label: LightweightM2M-LPW-10</rdfs:comment>
        <rdfs:label xml:lang="en">LorawanIdentifierBindings</rdfs:label>
    </owl:Class>
    


    <!-- http://purl.org/net/iot-dm#OWLClass_845f9a81_9845_4e96_b5cf_5d06ab798969 -->

    <owl:Class rdf:about="http://purl.org/net/iot-dm#OWLClass_845f9a81_9845_4e96_b5cf_5d06ab798969">
        <rdfs:subClassOf rdf:resource="http://purl.org/net/iot-dm#OWLClass_cbca8db6_d106_4651_a12c_b8fe629efbda"/>
        <rdfs:comment>Management of IoT Devices in a Physical Network, p. 487</rdfs:comment>
        <rdfs:label xml:lang="en">EventProcessingEngine</rdfs:label>
    </owl:Class>
    


    <!-- http://purl.org/net/iot-dm#OWLClass_84e47b54_0e55_484f_a6c3_7c9b2ac210c3 -->

    <owl:Class rdf:about="http://purl.org/net/iot-dm#OWLClass_84e47b54_0e55_484f_a6c3_7c9b2ac210c3">
        <rdfs:subClassOf rdf:resource="http://purl.org/net/iot-dm#OWLClass_81e411c6_43af_4e07_9341_d53659bfbb91"/>
        <rdfs:comment>Management of IoT Devices in a Physical Network, p. 488</rdfs:comment>
        <rdfs:label xml:lang="en">PreDefinedDeviceEvents</rdfs:label>
    </owl:Class>
    


    <!-- http://purl.org/net/iot-dm#OWLClass_8596de3a_a167_4503_9a19_64a1d5fbcd9b -->

    <owl:Class rdf:about="http://purl.org/net/iot-dm#OWLClass_8596de3a_a167_4503_9a19_64a1d5fbcd9b">
        <rdfs:subClassOf rdf:resource="http://purl.org/net/iot-dm#OWLClass_3300e6af_4338_4bf4_ab9e_632af0b5ad65"/>
        <rdfs:comment>OMA-RD-LightweightM2M-V1_1-20180710-A, Label: LightweightM2M-BsR-001</rdfs:comment>
        <rdfs:label xml:lang="en">AccessControlRightsRetrieval</rdfs:label>
    </owl:Class>
    


    <!-- http://purl.org/net/iot-dm#OWLClass_86628aec_b662_41c9_ae13_eec3bc59261a -->

    <owl:Class rdf:about="http://purl.org/net/iot-dm#OWLClass_86628aec_b662_41c9_ae13_eec3bc59261a">
        <rdfs:subClassOf rdf:resource="http://purl.org/net/iot-dm#OWLClass_10ff6f33_7c39_432c_9ac0_c8c9d830b8b9"/>
        <rdfs:comment>https://resin.io/features/, 2018-09-15</rdfs:comment>
        <rdfs:label xml:lang="en">Sdk</rdfs:label>
    </owl:Class>
    


    <!-- http://purl.org/net/iot-dm#OWLClass_869676ae_38cc_42d1_99e8_d76b7a144f45 -->

    <owl:Class rdf:about="http://purl.org/net/iot-dm#OWLClass_869676ae_38cc_42d1_99e8_d76b7a144f45">
        <rdfs:subClassOf rdf:resource="http://purl.org/net/iot-dm#OWLClass_f9db282e_22e2_48e5_a643_a42df05c880d"/>
        <rdfs:comment>IoT home gateway for auto-conﬁguration and management of MQTT devices, section I.</rdfs:comment>
        <rdfs:label xml:lang="en">CommunicationProtocolTranslation</rdfs:label>
    </owl:Class>
    


    <!-- http://purl.org/net/iot-dm#OWLClass_869abf01_eaf3_41bc_95ed_6a11d4959818 -->

    <owl:Class rdf:about="http://purl.org/net/iot-dm#OWLClass_869abf01_eaf3_41bc_95ed_6a11d4959818">
        <rdfs:subClassOf rdf:resource="http://purl.org/net/iot-dm#OWLClass_9e3d4f19_96c7_4932_a007_26fa592f3423"/>
        <rdfs:label xml:lang="en">Bootloader</rdfs:label>
    </owl:Class>
    


    <!-- http://purl.org/net/iot-dm#OWLClass_86bc12fa_4b44_4cb3_bc89_b209cf044cf0 -->

    <owl:Class rdf:about="http://purl.org/net/iot-dm#OWLClass_86bc12fa_4b44_4cb3_bc89_b209cf044cf0">
        <rdfs:subClassOf rdf:resource="http://purl.org/net/iot-dm#OWLClass_38e18d87_aade_4d8b_ab6e_1da467276a13"/>
        <rdfs:comment>Ontologies for the Internet of Things, 2., 3.2</rdfs:comment>
        <rdfs:label xml:lang="en">GeographicLocation</rdfs:label>
    </owl:Class>
    


    <!-- http://purl.org/net/iot-dm#OWLClass_8880aec0_29cf_4557_a1c3_3505555b54eb -->

    <owl:Class rdf:about="http://purl.org/net/iot-dm#OWLClass_8880aec0_29cf_4557_a1c3_3505555b54eb">
        <rdfs:subClassOf rdf:resource="http://purl.org/net/iot-dm#OWLClass_506a07f5_4566_41a4_84ac_ea621caa87b7"/>
        <rdfs:comment>https://resin.io/how-it-works/, 2019-09-16</rdfs:comment>
        <rdfs:label xml:lang="en">WebBasedDashboard</rdfs:label>
    </owl:Class>
    


    <!-- http://purl.org/net/iot-dm#OWLClass_88ad35cc_61a1_4cc0_bbd6_f74a256051bb -->

    <owl:Class rdf:about="http://purl.org/net/iot-dm#OWLClass_88ad35cc_61a1_4cc0_bbd6_f74a256051bb">
        <rdfs:subClassOf rdf:resource="http://purl.org/net/iot-dm#OWLClass_66c3fc69_337f_4795_a467_f0b64b90cb3b"/>
        <rdfs:comment>Recent Advances in Industrial Wireless Sensor Networks Towards Efficient Management in IoT, p. 13</rdfs:comment>
        <rdfs:label xml:lang="en">Privacy</rdfs:label>
    </owl:Class>
    


    <!-- http://purl.org/net/iot-dm#OWLClass_88bd0206_ec77_40fc_bde2_6c1e2637b12a -->

    <owl:Class rdf:about="http://purl.org/net/iot-dm#OWLClass_88bd0206_ec77_40fc_bde2_6c1e2637b12a">
        <rdfs:subClassOf rdf:resource="http://purl.org/net/iot-dm#OWLClass_6ff26810_f417_457e_90e7_f7187268ec90"/>
        <rdfs:label xml:lang="en">Categories</rdfs:label>
    </owl:Class>
    


    <!-- http://purl.org/net/iot-dm#OWLClass_88f21017_7856_4dc4_b90f_1a031f25dbb1 -->

    <owl:Class rdf:about="http://purl.org/net/iot-dm#OWLClass_88f21017_7856_4dc4_b90f_1a031f25dbb1">
        <rdfs:subClassOf rdf:resource="http://purl.org/net/iot-dm#OWLClass_3e781bea_1637_4984_bf63_8935b4e49e16"/>
        <rdfs:comment>OMA-RD-LightweightM2M-V1_1-20180710-A, Label: LightweightM2M-RMo-001</rdfs:comment>
        <rdfs:label xml:lang="en">RelationalOperatorBasedReportingMechanism</rdfs:label>
    </owl:Class>
    


    <!-- http://purl.org/net/iot-dm#OWLClass_89f81fe4_c0d0_4dd1_b866_babbba4f20de -->

    <owl:Class rdf:about="http://purl.org/net/iot-dm#OWLClass_89f81fe4_c0d0_4dd1_b866_babbba4f20de">
        <rdfs:subClassOf rdf:resource="http://purl.org/net/iot-dm#OWLClass_10ff6f33_7c39_432c_9ac0_c8c9d830b8b9"/>
        <rdfs:label xml:lang="en">ControlInterfaceSecurity</rdfs:label>
    </owl:Class>
    


    <!-- http://purl.org/net/iot-dm#OWLClass_8a91ffb6_d1c9_4026_9031_fd318df66665 -->

    <owl:Class rdf:about="http://purl.org/net/iot-dm#OWLClass_8a91ffb6_d1c9_4026_9031_fd318df66665">
        <rdfs:subClassOf rdf:resource="http://purl.org/net/iot-dm#OWLClass_38e18d87_aade_4d8b_ab6e_1da467276a13"/>
        <rdfs:comment>OMA-RD-LightweightM2M-V1_0-20170208-A, Label: LightweightM2M-HLF-001</rdfs:comment>
        <rdfs:comment>https://resin.io/how-it-works/, 2019-09-16</rdfs:comment>
        <rdfs:label xml:lang="en">UniqueDeviceId</rdfs:label>
    </owl:Class>
    


    <!-- http://purl.org/net/iot-dm#OWLClass_8b38f2cc_e06e_4d7c_b178_d4eb90c79a9f -->

    <owl:Class rdf:about="http://purl.org/net/iot-dm#OWLClass_8b38f2cc_e06e_4d7c_b178_d4eb90c79a9f">
        <rdfs:subClassOf rdf:resource="http://purl.org/net/iot-dm#OWLClass_30d8bc8b_4188_4a4f_be58_c4d70f00474e"/>
        <rdfs:comment>https://resin.io/how-it-works/, 2018-09-16</rdfs:comment>
        <rdfs:label xml:lang="en">ContainerSupervisor</rdfs:label>
    </owl:Class>
    


    <!-- http://purl.org/net/iot-dm#OWLClass_8bf32c78_6c9c_4513_bbe2_dd201c1aad26 -->

    <owl:Class rdf:about="http://purl.org/net/iot-dm#OWLClass_8bf32c78_6c9c_4513_bbe2_dd201c1aad26">
        <rdfs:subClassOf rdf:resource="http://purl.org/net/iot-dm#OWLClass_dd21fadb_8dfb_46e9_a311_b39ddefaad69"/>
        <rdfs:comment>OMA-RD-LightweightM2M-V1_0-20170208-A, Label: LightweightM2M-HLF-006</rdfs:comment>
        <rdfs:label xml:lang="en">PowerSourceStatus</rdfs:label>
    </owl:Class>
    


    <!-- http://purl.org/net/iot-dm#OWLClass_8c2c705b_ddcf_4dc0_b9d5_6e507868806e -->

    <owl:Class rdf:about="http://purl.org/net/iot-dm#OWLClass_8c2c705b_ddcf_4dc0_b9d5_6e507868806e">
        <rdfs:subClassOf rdf:resource="http://purl.org/net/iot-dm#OWLClass_2fb332cc_9b13_4fbc_af07_4ce1a662e062"/>
        <rdfs:label xml:lang="en">NetworkParameters</rdfs:label>
    </owl:Class>
    


    <!-- http://purl.org/net/iot-dm#OWLClass_8d022cdf_70be_45f9_9d88_cbb0eed5ddcb -->

    <owl:Class rdf:about="http://purl.org/net/iot-dm#OWLClass_8d022cdf_70be_45f9_9d88_cbb0eed5ddcb">
        <rdfs:subClassOf rdf:resource="http://purl.org/net/iot-dm#OWLClass_195de59b_34c2_45da_8aa8_591cd3847fc7"/>
        <rdfs:comment>OMA-RD-LightweightM2M-V1_1-20180710-A, Label: LightweightM2M-E2E-3</rdfs:comment>
        <rdfs:comment>OMA-RD-LightweightM2M-V1_1-20180710-A, Label: LightweightM2M-E2E-9</rdfs:comment>
        <rdfs:comment>OMA-RD-LightweightM2M-V1_1-20180710-A, Label: LightweightM2M-E2Eo-3</rdfs:comment>
        <rdfs:comment>OMA-RD-LightweightM2M-V1_1-20180710-A, Label: LightweightM2M-E2Eo-9</rdfs:comment>
        <rdfs:label xml:lang="en">ReplayProtection</rdfs:label>
    </owl:Class>
    


    <!-- http://purl.org/net/iot-dm#OWLClass_8d0e042d_1b1f_49ba_adfe_c0f3225daaf6 -->

    <owl:Class rdf:about="http://purl.org/net/iot-dm#OWLClass_8d0e042d_1b1f_49ba_adfe_c0f3225daaf6">
        <rdfs:subClassOf rdf:resource="http://purl.org/net/iot-dm#OWLClass_cfc68839_b898_454c_9314_0822698917f2"/>
        <rdfs:comment>https://resin.io/how-it-works/, 2019-09-16</rdfs:comment>
        <rdfs:label xml:lang="en">ContainerSupervisorVersion</rdfs:label>
    </owl:Class>
    


    <!-- http://purl.org/net/iot-dm#OWLClass_8d8b18d1_f087_4e04_b2f5_633089490ba1 -->

    <owl:Class rdf:about="http://purl.org/net/iot-dm#OWLClass_8d8b18d1_f087_4e04_b2f5_633089490ba1">
        <rdfs:subClassOf rdf:resource="http://purl.org/net/iot-dm#OWLClass_0fd00cb3_e44d_420b_bff2_9aafb1b10ace"/>
        <rdfs:comment>Management of IoT Devices in a Physical Network, p. 487</rdfs:comment>
        <rdfs:label xml:lang="en">NewDeviceDiscoveryInNetwork</rdfs:label>
    </owl:Class>
    


    <!-- http://purl.org/net/iot-dm#OWLClass_8df9f631_124d_4ae8_bd80_f06501eb3875 -->

    <owl:Class rdf:about="http://purl.org/net/iot-dm#OWLClass_8df9f631_124d_4ae8_bd80_f06501eb3875">
        <rdfs:subClassOf rdf:resource="http://purl.org/net/iot-dm#OWLClass_21fa4e78_3300_43d8_83c7_78d9ee314b79"/>
        <rdfs:comment>OMA-RD-LightweightM2M-V1_0-20170208-A, Label: LightweightM2M-HLF-027</rdfs:comment>
        <rdfs:label xml:lang="en">ConnectivityStatus</rdfs:label>
    </owl:Class>
    


    <!-- http://purl.org/net/iot-dm#OWLClass_8e4f6b4d_92dd_4de5_9e89_8d0f3d918c5e -->

    <owl:Class rdf:about="http://purl.org/net/iot-dm#OWLClass_8e4f6b4d_92dd_4de5_9e89_8d0f3d918c5e">
        <rdfs:subClassOf rdf:resource="http://purl.org/net/iot-dm#OWLClass_04312c30_fd26_4307_ab50_03991e776620"/>
        <rdfs:label xml:lang="en">ReportingModeConfiguration</rdfs:label>
    </owl:Class>
    


    <!-- http://purl.org/net/iot-dm#OWLClass_8ef34b5e_e120_4420_acd3_d1d04918da6b -->

    <owl:Class rdf:about="http://purl.org/net/iot-dm#OWLClass_8ef34b5e_e120_4420_acd3_d1d04918da6b">
        <rdfs:subClassOf rdf:resource="http://purl.org/net/iot-dm#OWLClass_6cb818a3_6278_4bad_8a6b_c01ee623c677"/>
        <rdfs:comment>OMA-RD-LightweightM2M-V1_0-20170208-A, Label: LightweightM2M-HLF-039</rdfs:comment>
        <rdfs:label xml:lang="en">TemporaryNetworkConnectionProhibition</rdfs:label>
    </owl:Class>
    


    <!-- http://purl.org/net/iot-dm#OWLClass_9062c375_f510_47a7_85fc_84f547a06681 -->

    <owl:Class rdf:about="http://purl.org/net/iot-dm#OWLClass_9062c375_f510_47a7_85fc_84f547a06681">
        <rdfs:subClassOf rdf:resource="http://purl.org/net/iot-dm#OWLClass_7c8282da_3443_4c49_a838_df6cb9a459c9"/>
        <rdfs:comment>draft-moran-suit-architecture-03 (work in progress), p. 6-7</rdfs:comment>
        <rdfs:comment>https://resin.io/how-it-works/, 2019-09-16</rdfs:comment>
        <rdfs:label xml:lang="en">MultipleFirmwareLocations</rdfs:label>
    </owl:Class>
    


    <!-- http://purl.org/net/iot-dm#OWLClass_91e1d636_17c7_43c3_ab32_ce7700226d44 -->

    <owl:Class rdf:about="http://purl.org/net/iot-dm#OWLClass_91e1d636_17c7_43c3_ab32_ce7700226d44">
        <rdfs:subClassOf rdf:resource="http://purl.org/net/iot-dm#OWLClass_e7e81967_1b1b_4dfb_b9b6_c40e0ffab441"/>
        <rdfs:label xml:lang="en">ExtendedPkiSupport</rdfs:label>
    </owl:Class>
    


    <!-- http://purl.org/net/iot-dm#OWLClass_9262cf89_f165_4ed8_9dd2_cf6a02eb9924 -->

    <owl:Class rdf:about="http://purl.org/net/iot-dm#OWLClass_9262cf89_f165_4ed8_9dd2_cf6a02eb9924">
        <rdfs:subClassOf rdf:resource="http://purl.org/net/iot-dm#OWLClass_63057798_6c27_4642_9ffc_9e5b09529dd2"/>
        <rdfs:comment>https://resin.io/features/, 2018-09-15</rdfs:comment>
        <rdfs:label xml:lang="en">WifiCredentials</rdfs:label>
    </owl:Class>
    


    <!-- http://purl.org/net/iot-dm#OWLClass_928a3dbe_0ae6_42b7_a752_d48930d19fae -->

    <owl:Class rdf:about="http://purl.org/net/iot-dm#OWLClass_928a3dbe_0ae6_42b7_a752_d48930d19fae">
        <rdfs:subClassOf rdf:resource="http://purl.org/net/iot-dm#OWLClass_c8340585_9c41_4f98_8f90_b4e2436e8829"/>
        <rdfs:label xml:lang="en">Lorawan</rdfs:label>
    </owl:Class>
    


    <!-- http://purl.org/net/iot-dm#OWLClass_9336e33f_2982_4ed9_b26a_5d3d28cbde20 -->

    <owl:Class rdf:about="http://purl.org/net/iot-dm#OWLClass_9336e33f_2982_4ed9_b26a_5d3d28cbde20">
        <rdfs:subClassOf rdf:resource="http://purl.org/net/iot-dm#OWLClass_2ee3c907_2ad6_45fc_999f_299667c29188"/>
        <rdfs:comment>Management of IoT Devices in a Physical Network, p. 488</rdfs:comment>
        <rdfs:label xml:lang="en">DeviceServices</rdfs:label>
    </owl:Class>
    


    <!-- http://purl.org/net/iot-dm#OWLClass_93985764_b5c7_4178_8d26_1d64d20d9922 -->

    <owl:Class rdf:about="http://purl.org/net/iot-dm#OWLClass_93985764_b5c7_4178_8d26_1d64d20d9922">
        <rdfs:subClassOf rdf:resource="http://purl.org/net/iot-dm#OWLClass_df537b47_a081_4de8_8904_3c63392ae836"/>
        <rdfs:comment>Management of IoT Devices in a Physical Network, p. 487</rdfs:comment>
        <rdfs:label xml:lang="en">KpiMonitoring</rdfs:label>
    </owl:Class>
    


    <!-- http://purl.org/net/iot-dm#OWLClass_93ed9d35_04e1_444d_a5ec_83b88ec7913b -->

    <owl:Class rdf:about="http://purl.org/net/iot-dm#OWLClass_93ed9d35_04e1_444d_a5ec_83b88ec7913b">
        <rdfs:subClassOf rdf:resource="http://purl.org/net/iot-dm#OWLClass_81e411c6_43af_4e07_9341_d53659bfbb91"/>
        <rdfs:comment>Management of IoT Devices in a Physical Network, p. 488</rdfs:comment>
        <rdfs:label xml:lang="en">PreDefinedDeviceServices</rdfs:label>
    </owl:Class>
    


    <!-- http://purl.org/net/iot-dm#OWLClass_94c76311_3b18_4d07_8b75_42b44d7fb1eb -->

    <owl:Class rdf:about="http://purl.org/net/iot-dm#OWLClass_94c76311_3b18_4d07_8b75_42b44d7fb1eb">
        <rdfs:subClassOf rdf:resource="http://purl.org/net/iot-dm#OWLClass_c8340585_9c41_4f98_8f90_b4e2436e8829"/>
        <rdfs:comment>OMA-RD-LightweightM2M-V1_1-20180710-A, Label: LightweightM2M-LPW-2</rdfs:comment>
        <rdfs:label xml:lang="en">DelayedOrNoAcknowledgementMethodSupport</rdfs:label>
    </owl:Class>
    


    <!-- http://purl.org/net/iot-dm#OWLClass_96668876_e17b_46e9_b086_5835d62ceaaa -->

    <owl:Class rdf:about="http://purl.org/net/iot-dm#OWLClass_96668876_e17b_46e9_b086_5835d62ceaaa">
        <rdfs:subClassOf rdf:resource="http://purl.org/net/iot-dm#OWLClass_cbca8db6_d106_4651_a12c_b8fe629efbda"/>
        <rdfs:comment>Recent Advances in Industrial Wireless Sensor Networks Towards Efficient Management in IoT, p. 1</rdfs:comment>
        <rdfs:label xml:lang="en">DevicePerformanceMonitoring</rdfs:label>
    </owl:Class>
    


    <!-- http://purl.org/net/iot-dm#OWLClass_9706d318_5cd1_4e58_8c3b_72eef36ee70a -->

    <owl:Class rdf:about="http://purl.org/net/iot-dm#OWLClass_9706d318_5cd1_4e58_8c3b_72eef36ee70a">
        <rdfs:subClassOf rdf:resource="http://purl.org/net/iot-dm#OWLClass_2a645b44_80eb_49d7_8add_d5dc3d46a6f9"/>
        <rdfs:comment xml:lang="en">&quot;The manifest contains meta-data about the firmware image. The manifest is protected against modification and provides information about the author.&quot;, draft-moran-suit-architecture-03 (work in progress), p. 5</rdfs:comment>
        <rdfs:label xml:lang="en">FirmwareManifest</rdfs:label>
    </owl:Class>
    


    <!-- http://purl.org/net/iot-dm#OWLClass_977dbd48_c449_473e_98e9_9e683f0e87e6 -->

    <owl:Class rdf:about="http://purl.org/net/iot-dm#OWLClass_977dbd48_c449_473e_98e9_9e683f0e87e6">
        <rdfs:subClassOf rdf:resource="http://purl.org/net/iot-dm#OWLClass_91e1d636_17c7_43c3_ab32_ce7700226d44"/>
        <rdfs:comment>OMA-RD-LightweightM2M-V1_1-20180710-A, Label: LightweightM2M-PKI-001</rdfs:comment>
        <rdfs:label xml:lang="en">CertificatesStatusCheck</rdfs:label>
    </owl:Class>
    


    <!-- http://purl.org/net/iot-dm#OWLClass_9848edfa_0cb1_4d11_96e3_a0d197164164 -->

    <owl:Class rdf:about="http://purl.org/net/iot-dm#OWLClass_9848edfa_0cb1_4d11_96e3_a0d197164164">
        <rdfs:subClassOf rdf:resource="http://purl.org/net/iot-dm#OWLClass_843d87bc_a343_470f_bff0_872b15b14c16"/>
        <rdfs:label xml:lang="en">FirmwareDelivery</rdfs:label>
    </owl:Class>
    


    <!-- http://purl.org/net/iot-dm#OWLClass_989411ba_e811_4185_bc1f_277d10d81160 -->

    <owl:Class rdf:about="http://purl.org/net/iot-dm#OWLClass_989411ba_e811_4185_bc1f_277d10d81160">
        <rdfs:subClassOf rdf:resource="http://purl.org/net/iot-dm#OWLClass_35227df9_2a26_4bf1_ae48_32e3c50a341c"/>
        <rdfs:comment>https://resin.io/how-it-works/, 2019-09-16</rdfs:comment>
        <rdfs:label xml:lang="en">WebTerminal</rdfs:label>
    </owl:Class>
    


    <!-- http://purl.org/net/iot-dm#OWLClass_98c7c2d8_185b_4994_82a7_b5e82b2bcdde -->

    <owl:Class rdf:about="http://purl.org/net/iot-dm#OWLClass_98c7c2d8_185b_4994_82a7_b5e82b2bcdde">
        <rdfs:subClassOf rdf:resource="http://purl.org/net/iot-dm#OWLClass_cf7d1708_1ca4_40a2_8852_72361ee2b730"/>
        <rdfs:comment>draft-moran-suit-architecture-03 (work in progress), p. 6</rdfs:comment>
        <rdfs:label xml:lang="en">FirmwareImageEncryption</rdfs:label>
    </owl:Class>
    


    <!-- http://purl.org/net/iot-dm#OWLClass_99b11aed_52eb_4a10_bb75_199cc40de00f -->

    <owl:Class rdf:about="http://purl.org/net/iot-dm#OWLClass_99b11aed_52eb_4a10_bb75_199cc40de00f">
        <rdfs:subClassOf rdf:resource="http://purl.org/net/iot-dm#OWLClass_66c3fc69_337f_4795_a467_f0b64b90cb3b"/>
        <rdfs:label xml:lang="en">Authentication</rdfs:label>
    </owl:Class>
    


    <!-- http://purl.org/net/iot-dm#OWLClass_99c4f5ac_bd0a_4686_9de1_4f1b80bc296a -->

    <owl:Class rdf:about="http://purl.org/net/iot-dm#OWLClass_99c4f5ac_bd0a_4686_9de1_4f1b80bc296a">
        <rdfs:subClassOf rdf:resource="http://purl.org/net/iot-dm#OWLClass_86628aec_b662_41c9_ae13_eec3bc59261a"/>
        <rdfs:comment>https://resin.io/features/, 2018-09-15</rdfs:comment>
        <rdfs:label xml:lang="en">JavaScriptSdk</rdfs:label>
    </owl:Class>
    


    <!-- http://purl.org/net/iot-dm#OWLClass_9ac2a5e2_d1a8_4c6c_a900_ed624c7fcef0 -->

    <owl:Class rdf:about="http://purl.org/net/iot-dm#OWLClass_9ac2a5e2_d1a8_4c6c_a900_ed624c7fcef0">
        <rdfs:subClassOf rdf:resource="http://purl.org/net/iot-dm#OWLClass_56ca2f5d_d065_4fe0_bfd8_9c86ea85f200"/>
        <rdfs:comment>IoT home gateway for auto-conﬁguration and management of MQTT devices, section III.</rdfs:comment>
        <rdfs:label xml:lang="en">StatusInformation</rdfs:label>
    </owl:Class>
    


    <!-- http://purl.org/net/iot-dm#OWLClass_9ad954d6_93a6_46e3_94d4_e486143e0812 -->

    <owl:Class rdf:about="http://purl.org/net/iot-dm#OWLClass_9ad954d6_93a6_46e3_94d4_e486143e0812">
        <rdfs:subClassOf rdf:resource="http://purl.org/net/iot-dm#OWLClass_68e5a285_5ba6_4cb1_85e7_ac792a46c65f"/>
        <rdfs:comment>Ontologies for the Internet of Things, 2.</rdfs:comment>
        <rdfs:label xml:lang="en">ErrorModels</rdfs:label>
    </owl:Class>
    


    <!-- http://purl.org/net/iot-dm#OWLClass_9c9ae891_01b4_4e9e_a355_30769cecfc13 -->

    <owl:Class rdf:about="http://purl.org/net/iot-dm#OWLClass_9c9ae891_01b4_4e9e_a355_30769cecfc13">
        <rdfs:subClassOf rdf:resource="http://purl.org/net/iot-dm#OWLClass_ffcb0dd3_5746_4e9b_9905_50bfb9faff34"/>
        <rdfs:comment>OMA-RD-LightweightM2M-V1_1-20180710-A, Label: LightweightM2M-LeG-001</rdfs:comment>
        <rdfs:label xml:lang="en">LegacyDeviceProtocolSupport</rdfs:label>
    </owl:Class>
    


    <!-- http://purl.org/net/iot-dm#OWLClass_9ceb488f_3183_4fed_a52c_afbad9d64014 -->

    <owl:Class rdf:about="http://purl.org/net/iot-dm#OWLClass_9ceb488f_3183_4fed_a52c_afbad9d64014">
        <rdfs:subClassOf rdf:resource="http://purl.org/net/iot-dm#OWLClass_cfbd03e3_461e_49ac_a682_824dcbfcacdd"/>
        <rdfs:comment>Recent Advances in Industrial Wireless Sensor Networks Towards Efficient Management in IoT, p. 6</rdfs:comment>
        <rdfs:label xml:lang="en">RouteForwardingToApplicationLayer</rdfs:label>
    </owl:Class>
    


    <!-- http://purl.org/net/iot-dm#OWLClass_9d0581a1_1bab_4643_9336_b632fa350e2f -->

    <owl:Class rdf:about="http://purl.org/net/iot-dm#OWLClass_9d0581a1_1bab_4643_9336_b632fa350e2f">
        <rdfs:subClassOf rdf:resource="http://purl.org/net/iot-dm#OWLClass_cbca8db6_d106_4651_a12c_b8fe629efbda"/>
        <rdfs:label xml:lang="en">SoftwareMonitoring</rdfs:label>
    </owl:Class>
    


    <!-- http://purl.org/net/iot-dm#OWLClass_9e1800f6_b3ba_41ee_b0ce_dac66a1a8680 -->

    <owl:Class rdf:about="http://purl.org/net/iot-dm#OWLClass_9e1800f6_b3ba_41ee_b0ce_dac66a1a8680">
        <rdfs:subClassOf rdf:resource="http://purl.org/net/iot-dm#OWLClass_cfe637aa_ec08_45c2_88c1_6a6c989d5b1e"/>
        <rdfs:label xml:lang="en">InternetProtocolSuite</rdfs:label>
    </owl:Class>
    


    <!-- http://purl.org/net/iot-dm#OWLClass_9e3d4f19_96c7_4932_a007_26fa592f3423 -->

    <owl:Class rdf:about="http://purl.org/net/iot-dm#OWLClass_9e3d4f19_96c7_4932_a007_26fa592f3423">
        <rdfs:comment xml:lang="en">&quot;The device is the recipient of the firmware image and the manifest. The goal is to update the firmware of the device.&quot;, draft-moran-suit-architecture-03 (work in progress), p. 5</rdfs:comment>
        <rdfs:label xml:lang="en">InternetOfThingsDevice</rdfs:label>
    </owl:Class>
    


    <!-- http://purl.org/net/iot-dm#OWLClass_9e7db1e6_48ce_4068_8b89_935b193258d4 -->

    <owl:Class rdf:about="http://purl.org/net/iot-dm#OWLClass_9e7db1e6_48ce_4068_8b89_935b193258d4">
        <rdfs:subClassOf rdf:resource="http://purl.org/net/iot-dm#OWLClass_a6cf31e3_5d7b_48b4_bce6_eada63815264"/>
        <rdfs:label xml:lang="en">OtherOperatingSystem</rdfs:label>
    </owl:Class>
    


    <!-- http://purl.org/net/iot-dm#OWLClass_9e9be86d_d950_4eb4_a6f6_717f9456afd4 -->

    <owl:Class rdf:about="http://purl.org/net/iot-dm#OWLClass_9e9be86d_d950_4eb4_a6f6_717f9456afd4">
        <rdfs:subClassOf rdf:resource="http://purl.org/net/iot-dm#OWLClass_86628aec_b662_41c9_ae13_eec3bc59261a"/>
        <rdfs:comment>https://resin.io/how-it-works/, 2019-09-16</rdfs:comment>
        <rdfs:label xml:lang="en">PythonSdk</rdfs:label>
    </owl:Class>
    


    <!-- http://purl.org/net/iot-dm#OWLClass_9f7e7307_2ac9_4f08_a47b_fc4d7ff74843 -->

    <owl:Class rdf:about="http://purl.org/net/iot-dm#OWLClass_9f7e7307_2ac9_4f08_a47b_fc4d7ff74843">
        <rdfs:subClassOf rdf:resource="http://purl.org/net/iot-dm#OWLClass_74bba417_5316_4b3f_b7d2_9fb2a118db2f"/>
        <rdfs:comment>OMA-RD-LightweightM2M-V1_0-20170208-A, Label: LightweightM2M-CF-001</rdfs:comment>
        <rdfs:label xml:lang="en">ConfidentialityEnsuranceMechanism</rdfs:label>
    </owl:Class>
    


    <!-- http://purl.org/net/iot-dm#OWLClass_9fcb5dc3_b98f_464b_ad5b_3b1b47050d11 -->

    <owl:Class rdf:about="http://purl.org/net/iot-dm#OWLClass_9fcb5dc3_b98f_464b_ad5b_3b1b47050d11">
        <rdfs:subClassOf rdf:resource="http://purl.org/net/iot-dm#OWLClass_66c3fc69_337f_4795_a467_f0b64b90cb3b"/>
        <rdfs:comment>&quot;little or no direct human interactions&quot;, Recent Advances in Industrial Wireless Sensor Networks Towards Efficient Management in IoT, p. 1

&quot;No direct human interaction: It is necessary to ensure a reliable communication via remote device and communication managements.&quot;, Recent Advances in Industrial Wireless Sensor Networks Towards Efficient Management in IoT, p. 6</rdfs:comment>
        <rdfs:label xml:lang="en">AutonomousDeviceOperationSupport</rdfs:label>
    </owl:Class>
    


    <!-- http://purl.org/net/iot-dm#OWLClass_a0392fad_b9d8_449e_a5ee_9a4633fe2912 -->

    <owl:Class rdf:about="http://purl.org/net/iot-dm#OWLClass_a0392fad_b9d8_449e_a5ee_9a4633fe2912">
        <rdfs:subClassOf rdf:resource="http://purl.org/net/iot-dm#OWLClass_515bf129_124c_4413_9e49_8de009d76986"/>
        <rdfs:comment>Ontologies for the Internet of Things, 3.2</rdfs:comment>
        <rdfs:label xml:lang="en">SamplingMethod</rdfs:label>
    </owl:Class>
    


    <!-- http://purl.org/net/iot-dm#OWLClass_a0c15140_3337_410f_a4f2_1d50988d93fd -->

    <owl:Class rdf:about="http://purl.org/net/iot-dm#OWLClass_a0c15140_3337_410f_a4f2_1d50988d93fd">
        <rdfs:subClassOf rdf:resource="http://purl.org/net/iot-dm#OWLClass_84e47b54_0e55_484f_a6c3_7c9b2ac210c3"/>
        <rdfs:comment>Management of IoT Devices in a Physical Network, p. 492</rdfs:comment>
        <rdfs:label xml:lang="en">PreDefinedDeviceRules</rdfs:label>
    </owl:Class>
    


    <!-- http://purl.org/net/iot-dm#OWLClass_a0f94d3c_fb8e_479e_81cd_4412cc42771f -->

    <owl:Class rdf:about="http://purl.org/net/iot-dm#OWLClass_a0f94d3c_fb8e_479e_81cd_4412cc42771f">
        <rdfs:subClassOf rdf:resource="http://purl.org/net/iot-dm#OWLClass_ba85de28_3f87_455f_9993_c51b31e1a44e"/>
        <rdfs:comment>Recent Advances in Industrial Wireless Sensor Networks Towards Efficient Management in IoT, p. 8</rdfs:comment>
        <rdfs:label xml:lang="en">VirtualDeviceInstanceDeregistration</rdfs:label>
    </owl:Class>
    


    <!-- http://purl.org/net/iot-dm#OWLClass_a1218b84_bf57_4b13_a97f_f6174a106e05 -->

    <owl:Class rdf:about="http://purl.org/net/iot-dm#OWLClass_a1218b84_bf57_4b13_a97f_f6174a106e05">
        <rdfs:subClassOf rdf:resource="http://purl.org/net/iot-dm#OWLClass_f519e17a_515d_402f_a5da_1cffe41727ea"/>
        <rdfs:comment>IoT home gateway for auto-conﬁguration and management of MQTT devices, section III.</rdfs:comment>
        <rdfs:label xml:lang="en">IpBased</rdfs:label>
    </owl:Class>
    


    <!-- http://purl.org/net/iot-dm#OWLClass_a142f55f_44aa_4869_8331_fa02fba549fb -->

    <owl:Class rdf:about="http://purl.org/net/iot-dm#OWLClass_a142f55f_44aa_4869_8331_fa02fba549fb">
        <rdfs:subClassOf rdf:resource="http://purl.org/net/iot-dm#OWLClass_04312c30_fd26_4307_ab50_03991e776620"/>
        <rdfs:comment>OMA-RD-LightweightM2M-V1_1-20180710-A, Label: LightweightM2M-LeG-005</rdfs:comment>
        <rdfs:label xml:lang="en">DataMapping</rdfs:label>
    </owl:Class>
    


    <!-- http://purl.org/net/iot-dm#OWLClass_a18f091d_134e_4059_ada6_9695459aa5f6 -->

    <owl:Class rdf:about="http://purl.org/net/iot-dm#OWLClass_a18f091d_134e_4059_ada6_9695459aa5f6">
        <rdfs:subClassOf rdf:resource="http://purl.org/net/iot-dm#OWLClass_b21422b7_b049_4b16_b3e0_53d1c9d53e85"/>
        <rdfs:label xml:lang="en">DeviceManagementCommunicationChannel</rdfs:label>
    </owl:Class>
    


    <!-- http://purl.org/net/iot-dm#OWLClass_a1b8792e_7d00_48b8_9efe_c6e47629e99c -->

    <owl:Class rdf:about="http://purl.org/net/iot-dm#OWLClass_a1b8792e_7d00_48b8_9efe_c6e47629e99c">
        <rdfs:subClassOf rdf:resource="http://purl.org/net/iot-dm#OWLClass_1bd19af8_5e90_482f_b798_79ba7cc8d671"/>
        <rdfs:comment>Recent Advances in Industrial Wireless Sensor Networks Towards Efficient Management in IoT, p. 6</rdfs:comment>
        <rdfs:label xml:lang="en">BigDataAnalytics</rdfs:label>
    </owl:Class>
    


    <!-- http://purl.org/net/iot-dm#OWLClass_a1cefa89_8494_4c67_8d71_44f07b80a613 -->

    <owl:Class rdf:about="http://purl.org/net/iot-dm#OWLClass_a1cefa89_8494_4c67_8d71_44f07b80a613">
        <rdfs:subClassOf rdf:resource="http://purl.org/net/iot-dm#OWLClass_2c177064_e630_44da_bbb3_d692886a8e4a"/>
        <rdfs:comment>OMA-RD-LightweightM2M-V1_1-20180710-A, Label: LightweightM2M-MaU-4</rdfs:comment>
        <rdfs:label xml:lang="en">LagModeInitialRegistration</rdfs:label>
    </owl:Class>
    


    <!-- http://purl.org/net/iot-dm#OWLClass_a2e5a8b7_7e0e_4972_a701_e63b5a3364f6 -->

    <owl:Class rdf:about="http://purl.org/net/iot-dm#OWLClass_a2e5a8b7_7e0e_4972_a701_e63b5a3364f6">
        <rdfs:label xml:lang="en">Language</rdfs:label>
    </owl:Class>
    


    <!-- http://purl.org/net/iot-dm#OWLClass_a36da934_36bc_4c07_bf06_2116cc5819b7 -->

    <owl:Class rdf:about="http://purl.org/net/iot-dm#OWLClass_a36da934_36bc_4c07_bf06_2116cc5819b7">
        <rdfs:subClassOf rdf:resource="http://purl.org/net/iot-dm#OWLClass_ae34f5cf_8888_4de3_9170_7e8f6eab5f86"/>
        <rdfs:comment>https://resin.io/how-it-works/, 2018-09-16</rdfs:comment>
        <rdfs:label xml:lang="en">ContainerDelivery</rdfs:label>
    </owl:Class>
    


    <!-- http://purl.org/net/iot-dm#OWLClass_a3f89bfa_5845_4577_b7f6_39d59036f955 -->

    <owl:Class rdf:about="http://purl.org/net/iot-dm#OWLClass_a3f89bfa_5845_4577_b7f6_39d59036f955">
        <rdfs:subClassOf rdf:resource="http://purl.org/net/iot-dm#OWLClass_e7e81967_1b1b_4dfb_b9b6_c40e0ffab441"/>
        <rdfs:comment xml:lang="en">draft-moran-suit-architecture-03 (work in progress), p. 5</rdfs:comment>
        <rdfs:label xml:lang="en">FirmwareUpdateStateOfTheArtSecurityMechanisms</rdfs:label>
    </owl:Class>
    


    <!-- http://purl.org/net/iot-dm#OWLClass_a5471a39_87b3_405c_bcfe_fd5eb03c9db9 -->

    <owl:Class rdf:about="http://purl.org/net/iot-dm#OWLClass_a5471a39_87b3_405c_bcfe_fd5eb03c9db9">
        <rdfs:subClassOf rdf:resource="http://purl.org/net/iot-dm#OWLClass_f6444fa6_1240_4dfa_9bba_affd175076ca"/>
        <rdfs:label xml:lang="en">SingleObserveConditionForResource</rdfs:label>
    </owl:Class>
    


    <!-- http://purl.org/net/iot-dm#OWLClass_a6782e7b_231e_47f2_8e4e_14508f18888f -->

    <owl:Class rdf:about="http://purl.org/net/iot-dm#OWLClass_a6782e7b_231e_47f2_8e4e_14508f18888f">
        <rdfs:subClassOf rdf:resource="http://purl.org/net/iot-dm#OWLClass_13c796b1_46e2_4fc7_b2d1_299b6746d07f"/>
        <rdfs:comment>IoT home gateway for auto-conﬁguration and management of MQTT devices, section III.</rdfs:comment>
        <rdfs:label xml:lang="en">DeviceName</rdfs:label>
    </owl:Class>
    


    <!-- http://purl.org/net/iot-dm#OWLClass_a6cf31e3_5d7b_48b4_bce6_eada63815264 -->

    <owl:Class rdf:about="http://purl.org/net/iot-dm#OWLClass_a6cf31e3_5d7b_48b4_bce6_eada63815264">
        <rdfs:subClassOf rdf:resource="http://purl.org/net/iot-dm#OWLClass_9e3d4f19_96c7_4932_a007_26fa592f3423"/>
        <rdfs:label xml:lang="en">OperatingSystem</rdfs:label>
    </owl:Class>
    


    <!-- http://purl.org/net/iot-dm#OWLClass_a6f072f9_98b2_40d1_ba35_6dc98cfeeb54 -->

    <owl:Class rdf:about="http://purl.org/net/iot-dm#OWLClass_a6f072f9_98b2_40d1_ba35_6dc98cfeeb54">
        <rdfs:subClassOf rdf:resource="http://purl.org/net/iot-dm#OWLClass_1bd19af8_5e90_482f_b798_79ba7cc8d671"/>
        <rdfs:label xml:lang="en">ApplicationDevelopmentFeatures</rdfs:label>
    </owl:Class>
    


    <!-- http://purl.org/net/iot-dm#OWLClass_a9fa280a_8537_4626_a942_bab8a45552c7 -->

    <owl:Class rdf:about="http://purl.org/net/iot-dm#OWLClass_a9fa280a_8537_4626_a942_bab8a45552c7">
        <rdfs:subClassOf rdf:resource="http://purl.org/net/iot-dm#OWLClass_845f9a81_9845_4e96_b5cf_5d06ab798969"/>
        <rdfs:comment>Management of IoT Devices in a Physical Network, p. 487</rdfs:comment>
        <rdfs:label xml:lang="en">RealTimeEventDetection</rdfs:label>
    </owl:Class>
    


    <!-- http://purl.org/net/iot-dm#OWLClass_ab772eaa_6f3a_44f2_b270_a2e094d82405 -->

    <owl:Class rdf:about="http://purl.org/net/iot-dm#OWLClass_ab772eaa_6f3a_44f2_b270_a2e094d82405">
        <rdfs:subClassOf rdf:resource="http://purl.org/net/iot-dm#OWLClass_21fa4e78_3300_43d8_83c7_78d9ee314b79"/>
        <rdfs:comment>OMA-RD-LightweightM2M-V1_0-20170208-A, Label: LightweightM2M-HLF-031</rdfs:comment>
        <rdfs:label xml:lang="en">DeviceStateChanges</rdfs:label>
    </owl:Class>
    


    <!-- http://purl.org/net/iot-dm#OWLClass_ac4a21a3_3d0d_485c_89c4_330cf7a185c0 -->

    <owl:Class rdf:about="http://purl.org/net/iot-dm#OWLClass_ac4a21a3_3d0d_485c_89c4_330cf7a185c0">
        <rdfs:subClassOf rdf:resource="http://purl.org/net/iot-dm#OWLClass_3a67a3e7_f65a_4e72_870f_eadff0700201"/>
        <rdfs:comment>OMA-RD-LightweightM2M-V1_1-20180710-A, Label: LightweightM2M-ENC-5</rdfs:comment>
        <rdfs:label xml:lang="en">StandardizedBitmapDataTypes</rdfs:label>
    </owl:Class>
    


    <!-- http://purl.org/net/iot-dm#OWLClass_ac590a14_c363_4380_af94_cc6137c8707a -->

    <owl:Class rdf:about="http://purl.org/net/iot-dm#OWLClass_ac590a14_c363_4380_af94_cc6137c8707a">
        <rdfs:subClassOf rdf:resource="http://purl.org/net/iot-dm#OWLClass_213b255b_d2a6_41ac_9e58_75311a7288f3"/>
        <rdfs:comment>OMA-RD-LightweightM2M-V1_0-20170208-A, Label: LightweightM2M-HLF-033</rdfs:comment>
        <rdfs:label xml:lang="en">DeviceResourceGrouping</rdfs:label>
    </owl:Class>
    


    <!-- http://purl.org/net/iot-dm#OWLClass_adb0c29e_5b2c_4710_8d19_6c5640c1ba60 -->

    <owl:Class rdf:about="http://purl.org/net/iot-dm#OWLClass_adb0c29e_5b2c_4710_8d19_6c5640c1ba60">
        <rdfs:subClassOf rdf:resource="http://purl.org/net/iot-dm#OWLClass_defe9266_4e6d_4036_8134_4ad7f7a4797e"/>
        <rdfs:comment>OMA-RD-LightweightM2M-V1_1-20180710-A, Label: LightweightM2M-DSE-002</rdfs:comment>
        <rdfs:label xml:lang="en">RetrieveValueOfSingleInstanceOfMultiInstancesResource</rdfs:label>
    </owl:Class>
    


    <!-- http://purl.org/net/iot-dm#OWLClass_ae34f5cf_8888_4de3_9170_7e8f6eab5f86 -->

    <owl:Class rdf:about="http://purl.org/net/iot-dm#OWLClass_ae34f5cf_8888_4de3_9170_7e8f6eab5f86">
        <rdfs:subClassOf rdf:resource="http://purl.org/net/iot-dm#OWLClass_71dcf03b_6cc1_4da4_9574_874b4477d105"/>
        <rdfs:label xml:lang="en">ContainerLifecycleManagment</rdfs:label>
    </owl:Class>
    


    <!-- http://purl.org/net/iot-dm#OWLClass_aeedc945_dbf7_4c98_9625_addd661997c7 -->

    <owl:Class rdf:about="http://purl.org/net/iot-dm#OWLClass_aeedc945_dbf7_4c98_9625_addd661997c7">
        <rdfs:subClassOf rdf:resource="http://purl.org/net/iot-dm#OWLClass_a18f091d_134e_4059_ada6_9695459aa5f6"/>
        <rdfs:label xml:lang="en">ProtocolSupport</rdfs:label>
    </owl:Class>
    


    <!-- http://purl.org/net/iot-dm#OWLClass_afbcc94f_ef75_4d4e_8800_832362e18374 -->

    <owl:Class rdf:about="http://purl.org/net/iot-dm#OWLClass_afbcc94f_ef75_4d4e_8800_832362e18374">
        <rdfs:subClassOf rdf:resource="http://purl.org/net/iot-dm#OWLClass_6c28e358_b8d8_4bd2_81e9_21b2d308b2a8"/>
        <rdfs:comment>OMA-RD-LightweightM2M-V1_1-20180710-A, Label: LightweightM2M-LeG-004</rdfs:comment>
        <rdfs:label xml:lang="en">GroupConcept</rdfs:label>
    </owl:Class>
    


    <!-- http://purl.org/net/iot-dm#OWLClass_b1b5ed2a_164d_442c_b05a_f9d7c3177a43 -->

    <owl:Class rdf:about="http://purl.org/net/iot-dm#OWLClass_b1b5ed2a_164d_442c_b05a_f9d7c3177a43">
        <rdfs:subClassOf rdf:resource="http://purl.org/net/iot-dm#OWLClass_515bf129_124c_4413_9e49_8de009d76986"/>
        <rdfs:comment>&quot;The real world property measured
by the sensor (e.g., temperature, wind speed, etc.).&quot;</rdfs:comment>
        <rdfs:comment>Ontologies for the Internet of Things, 3.2</rdfs:comment>
        <rdfs:label xml:lang="en">PhysicalConcept</rdfs:label>
    </owl:Class>
    


    <!-- http://purl.org/net/iot-dm#OWLClass_b1f8545f_a25f_4736_a13d_3ca3506ab184 -->

    <owl:Class rdf:about="http://purl.org/net/iot-dm#OWLClass_b1f8545f_a25f_4736_a13d_3ca3506ab184">
        <rdfs:subClassOf rdf:resource="http://purl.org/net/iot-dm#OWLClass_68e5a285_5ba6_4cb1_85e7_ac792a46c65f"/>
        <rdfs:comment>Ontologies for the Internet of Things, 2.</rdfs:comment>
        <rdfs:label xml:lang="en">EstimationMethods</rdfs:label>
    </owl:Class>
    


    <!-- http://purl.org/net/iot-dm#OWLClass_b21422b7_b049_4b16_b3e0_53d1c9d53e85 -->

    <owl:Class rdf:about="http://purl.org/net/iot-dm#OWLClass_b21422b7_b049_4b16_b3e0_53d1c9d53e85">
        <rdfs:subClassOf rdf:resource="http://purl.org/net/iot-dm#OWLClass_ebbfff77_6bbb_477e_9f30_934e7239601e"/>
        <rdfs:label xml:lang="en">DeviceManagement</rdfs:label>
    </owl:Class>
    


    <!-- http://purl.org/net/iot-dm#OWLClass_b2c59191_ce07_4543_9371_aec4c083e4b8 -->

    <owl:Class rdf:about="http://purl.org/net/iot-dm#OWLClass_b2c59191_ce07_4543_9371_aec4c083e4b8">
        <rdfs:subClassOf rdf:resource="http://purl.org/net/iot-dm#OWLClass_f6444fa6_1240_4dfa_9bba_affd175076ca"/>
        <rdfs:comment>OMA-RD-LightweightM2M-V1_1-20180710-A, Label: LightweightM2M-DSE-005</rdfs:comment>
        <rdfs:label xml:lang="en">RespectStructureAndFormatWhenReportingUnsolicitedDataForDefinedObjects</rdfs:label>
    </owl:Class>
    


    <!-- http://purl.org/net/iot-dm#OWLClass_b36b9cf5_86ad_4f75_8368_c8d26856c4bf -->

    <owl:Class rdf:about="http://purl.org/net/iot-dm#OWLClass_b36b9cf5_86ad_4f75_8368_c8d26856c4bf">
        <rdfs:subClassOf rdf:resource="http://purl.org/net/iot-dm#OWLClass_9e1800f6_b3ba_41ee_b0ce_dac66a1a8680"/>
        <rdfs:label xml:lang="en">LinkLayerProtocol</rdfs:label>
    </owl:Class>
    


    <!-- http://purl.org/net/iot-dm#OWLClass_b39f059d_7905_49e8_ad5f_9c295491892b -->

    <owl:Class rdf:about="http://purl.org/net/iot-dm#OWLClass_b39f059d_7905_49e8_ad5f_9c295491892b">
        <rdfs:subClassOf rdf:resource="http://purl.org/net/iot-dm#OWLClass_574c5366_c20d_467b_8ad6_787581d5f349"/>
        <rdfs:comment>IoT home gateway for auto-conﬁguration and management of MQTT devices, section III.</rdfs:comment>
        <rdfs:label xml:lang="en">NonIpBased</rdfs:label>
    </owl:Class>
    


    <!-- http://purl.org/net/iot-dm#OWLClass_b46bcdaf_df8a_4518_bbde_2812fa79496b -->

    <owl:Class rdf:about="http://purl.org/net/iot-dm#OWLClass_b46bcdaf_df8a_4518_bbde_2812fa79496b">
        <rdfs:subClassOf rdf:resource="http://purl.org/net/iot-dm#OWLClass_21fa4e78_3300_43d8_83c7_78d9ee314b79"/>
        <rdfs:comment>OMA-RD-LightweightM2M-V1_0-20170208-A, Label: LightweightM2M-HLF-035</rdfs:comment>
        <rdfs:label xml:lang="en">MultipleResourcesPerRequest</rdfs:label>
    </owl:Class>
    


    <!-- http://purl.org/net/iot-dm#OWLClass_b5c0d821_b62f_4098_9a87_9ab068cebe46 -->

    <owl:Class rdf:about="http://purl.org/net/iot-dm#OWLClass_b5c0d821_b62f_4098_9a87_9ab068cebe46">
        <rdfs:subClassOf rdf:resource="http://purl.org/net/iot-dm#OWLClass_ba85de28_3f87_455f_9993_c51b31e1a44e"/>
        <rdfs:label xml:lang="en">DeviceIdentification</rdfs:label>
    </owl:Class>
    


    <!-- http://purl.org/net/iot-dm#OWLClass_b6149766_693b_4c9c_945b_1c93f4878cea -->

    <owl:Class rdf:about="http://purl.org/net/iot-dm#OWLClass_b6149766_693b_4c9c_945b_1c93f4878cea">
        <rdfs:subClassOf rdf:resource="http://purl.org/net/iot-dm#OWLClass_84497e4c_1cfe_4d3f_b1ba_e6304c70216c"/>
        <rdfs:comment>OMA-RD-LightweightM2M-V1_1-20180710-A, Label: LightweightM2M-LPW-10</rdfs:comment>
        <rdfs:label xml:lang="en">AppSKey</rdfs:label>
    </owl:Class>
    


    <!-- http://purl.org/net/iot-dm#OWLClass_b668637f_602c_449f_8033_693bcbee5b73 -->

    <owl:Class rdf:about="http://purl.org/net/iot-dm#OWLClass_b668637f_602c_449f_8033_693bcbee5b73">
        <rdfs:subClassOf rdf:resource="http://purl.org/net/iot-dm#OWLClass_2ee3c907_2ad6_45fc_999f_299667c29188"/>
        <rdfs:comment>Management of IoT Devices in a Physical Network, p. 488</rdfs:comment>
        <rdfs:label xml:lang="en">DeviceEvents</rdfs:label>
    </owl:Class>
    


    <!-- http://purl.org/net/iot-dm#OWLClass_b6721ba6_4ea5_4be0_b34f_ff739be47358 -->

    <owl:Class rdf:about="http://purl.org/net/iot-dm#OWLClass_b6721ba6_4ea5_4be0_b34f_ff739be47358">
        <rdfs:subClassOf rdf:resource="http://purl.org/net/iot-dm#OWLClass_9e3d4f19_96c7_4932_a007_26fa592f3423"/>
        <rdfs:label xml:lang="en">FirmwareUpdateMechanism</rdfs:label>
    </owl:Class>
    


    <!-- http://purl.org/net/iot-dm#OWLClass_b84fdf88_7527_465b_8c12_682dc6944aa5 -->

    <owl:Class rdf:about="http://purl.org/net/iot-dm#OWLClass_b84fdf88_7527_465b_8c12_682dc6944aa5">
        <rdfs:subClassOf rdf:resource="http://purl.org/net/iot-dm#OWLClass_9706d318_5cd1_4e58_8c3b_72eef36ee70a"/>
        <rdfs:comment>draft-moran-suit-architecture-03 (work in progress), p. 12</rdfs:comment>
        <rdfs:label xml:lang="en">FirmwareImageTargetStorage</rdfs:label>
    </owl:Class>
    


    <!-- http://purl.org/net/iot-dm#OWLClass_ba85de28_3f87_455f_9993_c51b31e1a44e -->

    <owl:Class rdf:about="http://purl.org/net/iot-dm#OWLClass_ba85de28_3f87_455f_9993_c51b31e1a44e">
        <rdfs:subClassOf rdf:resource="http://purl.org/net/iot-dm#OWLClass_59540155_cb79_4e35_8db8_7519fb3535d5"/>
        <rdfs:comment>Recent Advances in Industrial Wireless Sensor Networks Towards Efficient Management in IoT, p. 1</rdfs:comment>
        <rdfs:label xml:lang="en">DeviceProvisioning</rdfs:label>
        <rdfs:seeAlso>DeviceRegistration</rdfs:seeAlso>
    </owl:Class>
    


    <!-- http://purl.org/net/iot-dm#OWLClass_bc3a1c08_92da_4179_aa2b_861d9851f19e -->

    <owl:Class rdf:about="http://purl.org/net/iot-dm#OWLClass_bc3a1c08_92da_4179_aa2b_861d9851f19e">
        <rdfs:subClassOf rdf:resource="http://purl.org/net/iot-dm#OWLClass_8e4f6b4d_92dd_4de5_9e89_8d0f3d918c5e"/>
        <rdfs:comment>OMA-RD-LightweightM2M-V1_0-20170208-A, Label: LightweightM2M-HLF-019</rdfs:comment>
        <rdfs:label xml:lang="en">PeriodicResourceReportingMechanismConfiguration</rdfs:label>
    </owl:Class>
    


    <!-- http://purl.org/net/iot-dm#OWLClass_bd5e9555_04ef_464e_8fd9_87a74e6c2949 -->

    <owl:Class rdf:about="http://purl.org/net/iot-dm#OWLClass_bd5e9555_04ef_464e_8fd9_87a74e6c2949">
        <rdfs:subClassOf rdf:resource="http://purl.org/net/iot-dm#OWLClass_80cdf1ca_1960_443d_abdb_8842cae1f466"/>
        <rdfs:comment>OMA-RD-LightweightM2M-V1_1-20180710-A, Label: LightweightM2M-MaU-1</rdfs:comment>
        <rdfs:label xml:lang="en">SaveDeviceSettingsBeforeFirmwareUpgrade</rdfs:label>
    </owl:Class>
    


    <!-- http://purl.org/net/iot-dm#OWLClass_bd6c6ad8_c97e_4399_bfcc_6b77b7f5987f -->

    <owl:Class rdf:about="http://purl.org/net/iot-dm#OWLClass_bd6c6ad8_c97e_4399_bfcc_6b77b7f5987f">
        <rdfs:subClassOf rdf:resource="http://purl.org/net/iot-dm#OWLClass_e00944d4_c070_4cf7_91ed_7f4c58ff50c8"/>
        <rdfs:label xml:lang="en">NumberOfRetries</rdfs:label>
        <rdfs:seeAlso>OMA-RD-LightweightM2M-V1_1-20180710-A, Label: LightweightM2M-BsR-004</rdfs:seeAlso>
    </owl:Class>
    


    <!-- http://purl.org/net/iot-dm#OWLClass_be8c9911_33e0_4d3b_8684_14d7241af1a7 -->

    <owl:Class rdf:about="http://purl.org/net/iot-dm#OWLClass_be8c9911_33e0_4d3b_8684_14d7241af1a7">
        <rdfs:subClassOf rdf:resource="http://purl.org/net/iot-dm#OWLClass_99b11aed_52eb_4a10_bb75_199cc40de00f"/>
        <rdfs:comment>OMA-RD-LightweightM2M-V1_0-20170208-A, Label: LightweightM2M-AT-001</rdfs:comment>
        <rdfs:label xml:lang="en">MutualAuthenticationBetweenClientAndServer</rdfs:label>
    </owl:Class>
    


    <!-- http://purl.org/net/iot-dm#OWLClass_be9385a6_0ac3_41d7_8249_f6beae8acb64 -->

    <owl:Class rdf:about="http://purl.org/net/iot-dm#OWLClass_be9385a6_0ac3_41d7_8249_f6beae8acb64">
        <rdfs:subClassOf rdf:resource="http://purl.org/net/iot-dm#OWLClass_1d7dd666_95ba_4c41_9a91_d850e9c0f479"/>
        <rdfs:comment>Recent Advances in Industrial Wireless Sensor Networks Towards Efficient Management in IoT, p. 6</rdfs:comment>
        <rdfs:label xml:lang="en">DeviceEnergyEfficiency</rdfs:label>
    </owl:Class>
    


    <!-- http://purl.org/net/iot-dm#OWLClass_beae1841_eca4_4666_bf75_5e2665a737e8 -->

    <owl:Class rdf:about="http://purl.org/net/iot-dm#OWLClass_beae1841_eca4_4666_bf75_5e2665a737e8">
        <rdfs:subClassOf rdf:resource="http://purl.org/net/iot-dm#OWLClass_b6721ba6_4ea5_4be0_b34f_ff739be47358"/>
        <rdfs:comment xml:lang="en">draft-moran-suit-architecture-03 (work in progress), p. 4</rdfs:comment>
        <rdfs:label xml:lang="en">AuthenticityCheck</rdfs:label>
    </owl:Class>
    


    <!-- http://purl.org/net/iot-dm#OWLClass_bec04496_99a7_4304_ab0c_85592a8bdfca -->

    <owl:Class rdf:about="http://purl.org/net/iot-dm#OWLClass_bec04496_99a7_4304_ab0c_85592a8bdfca">
        <rdfs:subClassOf rdf:resource="http://purl.org/net/iot-dm#OWLClass_6783e7e3_bc50_49de_8d69_4e137eec977b"/>
        <rdfs:comment>https://resin.io/features/, 2018-09-15</rdfs:comment>
        <rdfs:label xml:lang="en">CommunicationEncryption</rdfs:label>
    </owl:Class>
    


    <!-- http://purl.org/net/iot-dm#OWLClass_bedfd126_558c_464e_a0de_9132ae55e7f4 -->

    <owl:Class rdf:about="http://purl.org/net/iot-dm#OWLClass_bedfd126_558c_464e_a0de_9132ae55e7f4">
        <rdfs:subClassOf rdf:resource="http://purl.org/net/iot-dm#OWLClass_4c69720e_8886_407a_b9ce_8fcb374ea363"/>
        <rdfs:comment>OMA-RD-LightweightM2M-V1_1-20180710-A, Label: LightweightM2M-LPW-11</rdfs:comment>
        <rdfs:label xml:lang="en">AppEui</rdfs:label>
    </owl:Class>
    


    <!-- http://purl.org/net/iot-dm#OWLClass_bf7efd4a_62aa_4826_9e57_bb136265d0e0 -->

    <owl:Class rdf:about="http://purl.org/net/iot-dm#OWLClass_bf7efd4a_62aa_4826_9e57_bb136265d0e0">
        <rdfs:subClassOf rdf:resource="http://purl.org/net/iot-dm#OWLClass_1bd19af8_5e90_482f_b798_79ba7cc8d671"/>
        <rdfs:comment>Recent Advances in Industrial Wireless Sensor Networks Towards Efficient Management in IoT, p. 13</rdfs:comment>
        <rdfs:label xml:lang="en">ApplicationRuntime</rdfs:label>
    </owl:Class>
    


    <!-- http://purl.org/net/iot-dm#OWLClass_c013fdbe_4c9d_4aff_835d_543df3b064d6 -->

    <owl:Class rdf:about="http://purl.org/net/iot-dm#OWLClass_c013fdbe_4c9d_4aff_835d_543df3b064d6">
        <rdfs:subClassOf rdf:resource="http://purl.org/net/iot-dm#OWLClass_ec9156ee_5023_4804_9c7c_19a9a4ad18b4"/>
        <rdfs:comment>Recent Advances in Industrial Wireless Sensor Networks Towards Efficient Management in IoT, p. 10</rdfs:comment>
        <rdfs:label xml:lang="en">EndToEndAcknowledgement</rdfs:label>
    </owl:Class>
    


    <!-- http://purl.org/net/iot-dm#OWLClass_c0146b07_0c7e_4207_a8df_d7e5f67bc654 -->

    <owl:Class rdf:about="http://purl.org/net/iot-dm#OWLClass_c0146b07_0c7e_4207_a8df_d7e5f67bc654">
        <rdfs:subClassOf rdf:resource="http://purl.org/net/iot-dm#OWLClass_7ed5a132_c15b_486f_91f4_ad5eb4433cef"/>
        <rdfs:comment>&quot;The services themselves can also make use of update locking to block updates from happening during critical times (e.g. a drone that is flying, or an industrial machine that is in the middle of an operation).&quot;, https://resin.io/how-it-works/, 2019-09-16</rdfs:comment>
        <rdfs:label xml:lang="en">UpdateLocking</rdfs:label>
    </owl:Class>
    


    <!-- http://purl.org/net/iot-dm#OWLClass_c35d26c2_65cc_49bd_9875_9932fb747dd5 -->

    <owl:Class rdf:about="http://purl.org/net/iot-dm#OWLClass_c35d26c2_65cc_49bd_9875_9932fb747dd5">
        <rdfs:subClassOf rdf:resource="http://purl.org/net/iot-dm#OWLClass_9e1800f6_b3ba_41ee_b0ce_dac66a1a8680"/>
        <rdfs:label xml:lang="en">ApplicationLayerProtocol</rdfs:label>
    </owl:Class>
    


    <!-- http://purl.org/net/iot-dm#OWLClass_c365d735_e954_4b1b_80cb_8e26f409d31e -->

    <owl:Class rdf:about="http://purl.org/net/iot-dm#OWLClass_c365d735_e954_4b1b_80cb_8e26f409d31e">
        <rdfs:subClassOf rdf:resource="http://purl.org/net/iot-dm#OWLClass_ffcb0dd3_5746_4e9b_9905_50bfb9faff34"/>
        <rdfs:comment>OMA-RD-LightweightM2M-V1_1-20180710-A, Label: LightweightM2M-MBT-002</rdfs:comment>
        <rdfs:label xml:lang="en">TransportBindingsSeparatedMassaging</rdfs:label>
    </owl:Class>
    


    <!-- http://purl.org/net/iot-dm#OWLClass_c3bb2fa2_0fdd_4f76_9a51_d8db80f60842 -->

    <owl:Class rdf:about="http://purl.org/net/iot-dm#OWLClass_c3bb2fa2_0fdd_4f76_9a51_d8db80f60842">
        <rdfs:subClassOf rdf:resource="http://purl.org/net/iot-dm#OWLClass_195de59b_34c2_45da_8aa8_591cd3847fc7"/>
        <rdfs:comment>OMA-RD-LightweightM2M-V1_1-20180710-A, Label: LightweightM2M-E2E-2</rdfs:comment>
        <rdfs:comment>OMA-RD-LightweightM2M-V1_1-20180710-A, Label: LightweightM2M-E2E-8</rdfs:comment>
        <rdfs:comment>OMA-RD-LightweightM2M-V1_1-20180710-A, Label: LightweightM2M-E2Eo-2</rdfs:comment>
        <rdfs:comment>OMA-RD-LightweightM2M-V1_1-20180710-A, Label: LightweightM2M-E2Eo-8</rdfs:comment>
        <rdfs:label xml:lang="en">Encryption</rdfs:label>
    </owl:Class>
    


    <!-- http://purl.org/net/iot-dm#OWLClass_c3ce4f0f_2c54_43f1_801e_ce9649e05082 -->

    <owl:Class rdf:about="http://purl.org/net/iot-dm#OWLClass_c3ce4f0f_2c54_43f1_801e_ce9649e05082">
        <rdfs:subClassOf rdf:resource="http://purl.org/net/iot-dm#OWLClass_f4c68c89_a4ee_4e3f_b527_9a88d50887fe"/>
        <rdfs:comment>OMA-RD-LightweightM2M-V1_0-20170208-A, Label: LightweightM2M-HLF-040</rdfs:comment>
        <rdfs:label xml:lang="en">NetworkConnectivityProhibitionRestoreMechanism</rdfs:label>
    </owl:Class>
    


    <!-- http://purl.org/net/iot-dm#OWLClass_c465ac2b_a0c1_4be6_bc30_442c9d95f8b4 -->

    <owl:Class rdf:about="http://purl.org/net/iot-dm#OWLClass_c465ac2b_a0c1_4be6_bc30_442c9d95f8b4">
        <rdfs:subClassOf rdf:resource="http://purl.org/net/iot-dm#OWLClass_2d9c2b5f_16f1_4947_b01d_6f7578a2c079"/>
        <rdfs:comment>https://resin.io/features/, 2018-09-15</rdfs:comment>
        <rdfs:label xml:lang="en">WebBasedAccess</rdfs:label>
    </owl:Class>
    


    <!-- http://purl.org/net/iot-dm#OWLClass_c50e4d77_da83_4a1c_b2af_de71fb6d913a -->

    <owl:Class rdf:about="http://purl.org/net/iot-dm#OWLClass_c50e4d77_da83_4a1c_b2af_de71fb6d913a">
        <rdfs:subClassOf rdf:resource="http://purl.org/net/iot-dm#OWLClass_38e18d87_aade_4d8b_ab6e_1da467276a13"/>
        <rdfs:comment>Ontologies for the Internet of Things, 3.2</rdfs:comment>
        <rdfs:label xml:lang="en">Manufacturer</rdfs:label>
    </owl:Class>
    


    <!-- http://purl.org/net/iot-dm#OWLClass_c5fe4857_655f_43bd_b2a7_05807c88528e -->

    <owl:Class rdf:about="http://purl.org/net/iot-dm#OWLClass_c5fe4857_655f_43bd_b2a7_05807c88528e">
        <rdfs:subClassOf rdf:resource="http://purl.org/net/iot-dm#OWLClass_843d87bc_a343_470f_bff0_872b15b14c16"/>
        <rdfs:comment>OMA-RD-LightweightM2M-V1_1-20180710-A, Label: LightweightM2M-MaU-2</rdfs:comment>
        <rdfs:label xml:lang="en">FirmwareUpgradeReversal</rdfs:label>
    </owl:Class>
    


    <!-- http://purl.org/net/iot-dm#OWLClass_c6361626_a366_4e0b_9bc1_d65ba49d8d7f -->

    <owl:Class rdf:about="http://purl.org/net/iot-dm#OWLClass_c6361626_a366_4e0b_9bc1_d65ba49d8d7f">
        <rdfs:subClassOf rdf:resource="http://purl.org/net/iot-dm#OWLClass_f6444fa6_1240_4dfa_9bba_affd175076ca"/>
        <rdfs:comment>OMA-RD-LightweightM2M-V1_1-20180710-A, Label: LightweightM2M-RMo-003</rdfs:comment>
        <rdfs:label xml:lang="en">MultipleObserveConditionsForSameResource</rdfs:label>
    </owl:Class>
    


    <!-- http://purl.org/net/iot-dm#OWLClass_c64ae4a2_8cfa_49cd_b99d_f4a326820c2f -->

    <owl:Class rdf:about="http://purl.org/net/iot-dm#OWLClass_c64ae4a2_8cfa_49cd_b99d_f4a326820c2f">
        <rdfs:subClassOf rdf:resource="http://purl.org/net/iot-dm#OWLClass_88bd0206_ec77_40fc_bde2_6c1e2637b12a"/>
        <rdfs:comment>https://resin.io/how-it-works/, 2019-09-16</rdfs:comment>
        <rdfs:label xml:lang="en">Stdout</rdfs:label>
    </owl:Class>
    


    <!-- http://purl.org/net/iot-dm#OWLClass_c74a5982_d5bc_40b3_9e18_c03e025b5949 -->

    <owl:Class rdf:about="http://purl.org/net/iot-dm#OWLClass_c74a5982_d5bc_40b3_9e18_c03e025b5949">
        <rdfs:subClassOf rdf:resource="http://purl.org/net/iot-dm#OWLClass_869abf01_eaf3_41bc_95ed_6a11d4959818"/>
        <rdfs:comment>draft-moran-suit-architecture-03 (work in progress), p. 7</rdfs:comment>
        <rdfs:label xml:lang="en">MinimalBootloader</rdfs:label>
    </owl:Class>
    


    <!-- http://purl.org/net/iot-dm#OWLClass_c8340585_9c41_4f98_8f90_b4e2436e8829 -->

    <owl:Class rdf:about="http://purl.org/net/iot-dm#OWLClass_c8340585_9c41_4f98_8f90_b4e2436e8829">
        <rdfs:subClassOf rdf:resource="http://purl.org/net/iot-dm#OWLClass_ffcb0dd3_5746_4e9b_9905_50bfb9faff34"/>
        <rdfs:label xml:lang="en">Lpwan</rdfs:label>
    </owl:Class>
    


    <!-- http://purl.org/net/iot-dm#OWLClass_c91df911_0a3c_41ea_b67e_82282b18d4fe -->

    <owl:Class rdf:about="http://purl.org/net/iot-dm#OWLClass_c91df911_0a3c_41ea_b67e_82282b18d4fe">
        <rdfs:subClassOf rdf:resource="http://purl.org/net/iot-dm#OWLClass_8a91ffb6_d1c9_4026_9031_fd318df66665"/>
        <rdfs:label xml:lang="en">MacAddress</rdfs:label>
    </owl:Class>
    


    <!-- http://purl.org/net/iot-dm#OWLClass_c9387f59_78a4_45ac_a4bc_157f6c976385 -->

    <owl:Class rdf:about="http://purl.org/net/iot-dm#OWLClass_c9387f59_78a4_45ac_a4bc_157f6c976385">
        <rdfs:subClassOf rdf:resource="http://purl.org/net/iot-dm#OWLClass_4aa258d4_0b15_42d1_b4ed_87a2494976e5"/>
        <rdfs:comment>Recent Advances in Industrial Wireless Sensor Networks Towards Efficient Management in IoT, p. 8</rdfs:comment>
        <rdfs:label xml:lang="en">Coap</rdfs:label>
    </owl:Class>
    


    <!-- http://purl.org/net/iot-dm#OWLClass_cbca8db6_d106_4651_a12c_b8fe629efbda -->

    <owl:Class rdf:about="http://purl.org/net/iot-dm#OWLClass_cbca8db6_d106_4651_a12c_b8fe629efbda">
        <rdfs:subClassOf rdf:resource="http://purl.org/net/iot-dm#OWLClass_b21422b7_b049_4b16_b3e0_53d1c9d53e85"/>
        <rdfs:comment>Recent Advances in Industrial Wireless Sensor Networks Towards Efficient Management in IoT, p. 1, 6</rdfs:comment>
        <rdfs:label xml:lang="en">DeviceMonitoring</rdfs:label>
    </owl:Class>
    


    <!-- http://purl.org/net/iot-dm#OWLClass_cdca4605_0981_47f3_be76_554636de1e00 -->

    <owl:Class rdf:about="http://purl.org/net/iot-dm#OWLClass_cdca4605_0981_47f3_be76_554636de1e00">
        <rdfs:subClassOf rdf:resource="http://purl.org/net/iot-dm#OWLClass_9848edfa_0cb1_4d11_96e3_a0d197164164"/>
        <rdfs:comment xml:lang="en">draft-moran-suit-architecture-03 (work in progress), p. 6</rdfs:comment>
        <rdfs:label xml:lang="en">BroadcastFirmwareDelivery</rdfs:label>
    </owl:Class>
    


    <!-- http://purl.org/net/iot-dm#OWLClass_ce0a0295_7d23_4e15_bede_e55ff6079039 -->

    <owl:Class rdf:about="http://purl.org/net/iot-dm#OWLClass_ce0a0295_7d23_4e15_bede_e55ff6079039">
        <rdfs:subClassOf rdf:resource="http://purl.org/net/iot-dm#OWLClass_8c2c705b_ddcf_4dc0_b9d5_6e507868806e"/>
        <rdfs:comment>OMA-RD-LightweightM2M-V1_0-20170208-A, Label: LightweightM2M-HLF-037</rdfs:comment>
        <rdfs:comment>https://resin.io/features/, 2018-09-15</rdfs:comment>
        <rdfs:label xml:lang="en">DeviceConnectionAddress</rdfs:label>
        <rdfs:seeAlso xml:lang="en">DeviceIPAddress</rdfs:seeAlso>
    </owl:Class>
    


    <!-- http://purl.org/net/iot-dm#OWLClass_cef6dc67_5fbe_4789_bcd6_d00d776c464e -->

    <owl:Class rdf:about="http://purl.org/net/iot-dm#OWLClass_cef6dc67_5fbe_4789_bcd6_d00d776c464e">
        <rdfs:subClassOf rdf:resource="http://purl.org/net/iot-dm#OWLClass_a9fa280a_8537_4626_a942_bab8a45552c7"/>
        <rdfs:comment>Management of IoT Devices in a Physical Network, p. 490</rdfs:comment>
        <rdfs:label xml:lang="en">ErrorEvent</rdfs:label>
    </owl:Class>
    


    <!-- http://purl.org/net/iot-dm#OWLClass_cf2144ec_9c35_4ed0_8634_362c5e24ad8a -->

    <owl:Class rdf:about="http://purl.org/net/iot-dm#OWLClass_cf2144ec_9c35_4ed0_8634_362c5e24ad8a">
        <rdfs:subClassOf rdf:resource="http://purl.org/net/iot-dm#OWLClass_ffcb0dd3_5746_4e9b_9905_50bfb9faff34"/>
        <rdfs:comment>OMA-RD-LightweightM2M-V1_1-20180710-A, Label: LightweightM2M-SCS-4</rdfs:comment>
        <rdfs:label xml:lang="en">IdenticalOperationsToAddressObjectInstancesInDifferentStorageLocations</rdfs:label>
    </owl:Class>
    


    <!-- http://purl.org/net/iot-dm#OWLClass_cf7d1708_1ca4_40a2_8852_72361ee2b730 -->

    <owl:Class rdf:about="http://purl.org/net/iot-dm#OWLClass_cf7d1708_1ca4_40a2_8852_72361ee2b730">
        <rdfs:subClassOf rdf:resource="http://purl.org/net/iot-dm#OWLClass_15514c90_84d5_4670_93a6_9566cb808feb"/>
        <rdfs:comment xml:lang="en">draft-moran-suit-architecture-03 (work in progress), p. 4</rdfs:comment>
        <rdfs:label xml:lang="en">FirmwareImageConfidentialityProtection</rdfs:label>
    </owl:Class>
    


    <!-- http://purl.org/net/iot-dm#OWLClass_cfbd03e3_461e_49ac_a682_824dcbfcacdd -->

    <owl:Class rdf:about="http://purl.org/net/iot-dm#OWLClass_cfbd03e3_461e_49ac_a682_824dcbfcacdd">
        <rdfs:subClassOf rdf:resource="http://purl.org/net/iot-dm#OWLClass_1bd19af8_5e90_482f_b798_79ba7cc8d671"/>
        <rdfs:comment>Recent Advances in Industrial Wireless Sensor Networks Towards Efficient Management in IoT, p. 13</rdfs:comment>
        <rdfs:label xml:lang="en">ApplicationServices</rdfs:label>
    </owl:Class>
    


    <!-- http://purl.org/net/iot-dm#OWLClass_cfc68839_b898_454c_9314_0822698917f2 -->

    <owl:Class rdf:about="http://purl.org/net/iot-dm#OWLClass_cfc68839_b898_454c_9314_0822698917f2">
        <rdfs:subClassOf rdf:resource="http://purl.org/net/iot-dm#OWLClass_2fb332cc_9b13_4fbc_af07_4ce1a662e062"/>
        <rdfs:label xml:lang="en">SoftwareVersions</rdfs:label>
    </owl:Class>
    


    <!-- http://purl.org/net/iot-dm#OWLClass_cfe637aa_ec08_45c2_88c1_6a6c989d5b1e -->

    <owl:Class rdf:about="http://purl.org/net/iot-dm#OWLClass_cfe637aa_ec08_45c2_88c1_6a6c989d5b1e">
        <rdfs:label xml:lang="en">Protocol</rdfs:label>
    </owl:Class>
    


    <!-- http://purl.org/net/iot-dm#OWLClass_d109a5cf_0531_435a_a664_088946e3bfb5 -->

    <owl:Class rdf:about="http://purl.org/net/iot-dm#OWLClass_d109a5cf_0531_435a_a664_088946e3bfb5">
        <rdfs:subClassOf rdf:resource="http://purl.org/net/iot-dm#OWLClass_c8340585_9c41_4f98_8f90_b4e2436e8829"/>
        <rdfs:comment>OMA-RD-LightweightM2M-V1_1-20180710-A, Label: LightweightM2M-LPW-3</rdfs:comment>
        <rdfs:label xml:lang="en">SmsUsingExternalIdentifier</rdfs:label>
    </owl:Class>
    


    <!-- http://purl.org/net/iot-dm#OWLClass_d1a0965b_1f40_47d7_a843_c95e73835de7 -->

    <owl:Class rdf:about="http://purl.org/net/iot-dm#OWLClass_d1a0965b_1f40_47d7_a843_c95e73835de7">
        <rdfs:subClassOf rdf:resource="http://purl.org/net/iot-dm#OWLClass_66c3fc69_337f_4795_a467_f0b64b90cb3b"/>
        <rdfs:comment>Recent Advances in Industrial Wireless Sensor Networks Towards Efficient Management in IoT, p. 13</rdfs:comment>
        <rdfs:label xml:lang="en">RealTimeDeviceManagement</rdfs:label>
    </owl:Class>
    


    <!-- http://purl.org/net/iot-dm#OWLClass_d1c35aff_78e2_440f_8842_f12fc0ad9a9f -->

    <owl:Class rdf:about="http://purl.org/net/iot-dm#OWLClass_d1c35aff_78e2_440f_8842_f12fc0ad9a9f">
        <rdfs:subClassOf rdf:resource="http://purl.org/net/iot-dm#OWLClass_ae34f5cf_8888_4de3_9170_7e8f6eab5f86"/>
        <rdfs:comment>https://resin.io/how-it-works/, 2019-09-16</rdfs:comment>
        <rdfs:label xml:lang="en">ContainerStartup</rdfs:label>
    </owl:Class>
    


    <!-- http://purl.org/net/iot-dm#OWLClass_d2af3e8e_4fff_4e3e_b8da_dab17ea1fe30 -->

    <owl:Class rdf:about="http://purl.org/net/iot-dm#OWLClass_d2af3e8e_4fff_4e3e_b8da_dab17ea1fe30">
        <rdfs:subClassOf rdf:resource="http://purl.org/net/iot-dm#OWLClass_195de59b_34c2_45da_8aa8_591cd3847fc7"/>
        <rdfs:comment>OMA-RD-LightweightM2M-V1_1-20180710-A, Label: LightweightM2M-E2E-12</rdfs:comment>
        <rdfs:comment>OMA-RD-LightweightM2M-V1_1-20180710-A, Label: LightweightM2M-E2E-6</rdfs:comment>
        <rdfs:comment>OMA-RD-LightweightM2M-V1_1-20180710-A, Label: LightweightM2M-E2Eo-12</rdfs:comment>
        <rdfs:comment>OMA-RD-LightweightM2M-V1_1-20180710-A, Label: LightweightM2M-E2Eo-6</rdfs:comment>
        <rdfs:label xml:lang="en">RequestFreshnessVerification</rdfs:label>
    </owl:Class>
    


    <!-- http://purl.org/net/iot-dm#OWLClass_d3e3783e_5cf5_4824_be85_cab239f5b321 -->

    <owl:Class rdf:about="http://purl.org/net/iot-dm#OWLClass_d3e3783e_5cf5_4824_be85_cab239f5b321">
        <rdfs:subClassOf rdf:resource="http://purl.org/net/iot-dm#OWLClass_4c69720e_8886_407a_b9ce_8fcb374ea363"/>
        <rdfs:comment>OMA-RD-LightweightM2M-V1_1-20180710-A, Label: LightweightM2M-LPW-11</rdfs:comment>
        <rdfs:label xml:lang="en">AppKey</rdfs:label>
    </owl:Class>
    


    <!-- http://purl.org/net/iot-dm#OWLClass_d4c400c3_4296_4e1f_8d68_3fc880b3eac4 -->

    <owl:Class rdf:about="http://purl.org/net/iot-dm#OWLClass_d4c400c3_4296_4e1f_8d68_3fc880b3eac4">
        <rdfs:subClassOf rdf:resource="http://purl.org/net/iot-dm#OWLClass_213b255b_d2a6_41ac_9e58_75311a7288f3"/>
        <rdfs:comment>Management of IoT Devices in a Physical Network, p. 486</rdfs:comment>
        <rdfs:label xml:lang="en">DeviceFunctionalities</rdfs:label>
    </owl:Class>
    


    <!-- http://purl.org/net/iot-dm#OWLClass_d4cad6cb_2254_4af2_9ece_5f8b6f2fd024 -->

    <owl:Class rdf:about="http://purl.org/net/iot-dm#OWLClass_d4cad6cb_2254_4af2_9ece_5f8b6f2fd024">
        <rdfs:subClassOf rdf:resource="http://purl.org/net/iot-dm#OWLClass_8e4f6b4d_92dd_4de5_9e89_8d0f3d918c5e"/>
        <rdfs:comment>OMA-RD-LightweightM2M-V1_0-20170208-A, Label: LightweightM2M-HLF-022</rdfs:comment>
        <rdfs:label xml:lang="en">ResourceReportingPeriodConfiguration</rdfs:label>
    </owl:Class>
    


    <!-- http://purl.org/net/iot-dm#OWLClass_d5baf8ff_3ca0_40a1_988a_a5e23a144824 -->

    <owl:Class rdf:about="http://purl.org/net/iot-dm#OWLClass_d5baf8ff_3ca0_40a1_988a_a5e23a144824">
        <rdfs:subClassOf rdf:resource="http://purl.org/net/iot-dm#OWLClass_ebbfff77_6bbb_477e_9f30_934e7239601e"/>
        <rdfs:label xml:lang="en">Connectivity</rdfs:label>
    </owl:Class>
    


    <!-- http://purl.org/net/iot-dm#OWLClass_d670f170_e604_4d1e_9d35_f8f9a6ef751e -->

    <owl:Class rdf:about="http://purl.org/net/iot-dm#OWLClass_d670f170_e604_4d1e_9d35_f8f9a6ef751e">
        <rdfs:subClassOf rdf:resource="http://purl.org/net/iot-dm#OWLClass_2c177064_e630_44da_bbb3_d692886a8e4a"/>
        <rdfs:comment>OMA-RD-LightweightM2M-V1_1-20180710-A, Label: LightweightM2M-BsR-005</rdfs:comment>
        <rdfs:label xml:lang="en">OrderOfRegistrationSequence</rdfs:label>
    </owl:Class>
    


    <!-- http://purl.org/net/iot-dm#OWLClass_d6c16025_fac0_46c8_8583_b885fc1b424b -->

    <owl:Class rdf:about="http://purl.org/net/iot-dm#OWLClass_d6c16025_fac0_46c8_8583_b885fc1b424b">
        <rdfs:subClassOf rdf:resource="http://purl.org/net/iot-dm#OWLClass_9706d318_5cd1_4e58_8c3b_72eef36ee70a"/>
        <rdfs:comment>draft-moran-suit-architecture-03 (work in progress), p. 12</rdfs:comment>
        <rdfs:label xml:lang="en">ManifestCreationDate</rdfs:label>
    </owl:Class>
    


    <!-- http://purl.org/net/iot-dm#OWLClass_d792353f_077e_4c3f_b673_89a89a54a4ee -->

    <owl:Class rdf:about="http://purl.org/net/iot-dm#OWLClass_d792353f_077e_4c3f_b673_89a89a54a4ee">
        <rdfs:subClassOf rdf:resource="http://purl.org/net/iot-dm#OWLClass_defe9266_4e6d_4036_8134_4ad7f7a4797e"/>
        <rdfs:comment>OMA-RD-LightweightM2M-V1_1-20180710-A, Label: LightweightM2M-DSE-002</rdfs:comment>
        <rdfs:label xml:lang="en">SetValueOfSingleInstanceOfMultiInstancesResource</rdfs:label>
    </owl:Class>
    


    <!-- http://purl.org/net/iot-dm#OWLClass_d7f22e0f_3381_4d55_9bbb_0cd4a1d919df -->

    <owl:Class rdf:about="http://purl.org/net/iot-dm#OWLClass_d7f22e0f_3381_4d55_9bbb_0cd4a1d919df">
        <rdfs:subClassOf rdf:resource="http://purl.org/net/iot-dm#OWLClass_4c69f2df_35c9_4bf1_8b7f_b0e8fcac7aca"/>
        <rdfs:comment>draft-moran-suit-architecture-03 (work in progress), p. 6</rdfs:comment>
        <rdfs:label xml:lang="en">FirmwareValidationFailure</rdfs:label>
    </owl:Class>
    


    <!-- http://purl.org/net/iot-dm#OWLClass_d82d3960_2a78_4353_815b_c8c9ad2b52c1 -->

    <owl:Class rdf:about="http://purl.org/net/iot-dm#OWLClass_d82d3960_2a78_4353_815b_c8c9ad2b52c1">
        <rdfs:subClassOf rdf:resource="http://purl.org/net/iot-dm#OWLClass_3a67a3e7_f65a_4e72_870f_eadff0700201"/>
        <rdfs:comment>OMA-RD-LightweightM2M-V1_1-20180710-A, Label: LightweightM2M-ENC-4</rdfs:comment>
        <rdfs:label xml:lang="en">StandardizedUriDataTypes</rdfs:label>
    </owl:Class>
    


    <!-- http://purl.org/net/iot-dm#OWLClass_d8e49365_06e1_40c2_99fc_891f2256aad1 -->

    <owl:Class rdf:about="http://purl.org/net/iot-dm#OWLClass_d8e49365_06e1_40c2_99fc_891f2256aad1">
        <rdfs:subClassOf rdf:resource="http://purl.org/net/iot-dm#OWLClass_aeedc945_dbf7_4c98_9625_addd661997c7"/>
        <rdfs:comment>IoT home gateway for auto-conﬁguration and management of MQTT devices, section I.</rdfs:comment>
        <rdfs:label xml:lang="en">DeviceManagementAndDiscoveryProtocol</rdfs:label>
    </owl:Class>
    


    <!-- http://purl.org/net/iot-dm#OWLClass_d95c726a_c63f_4e85_b9da_25bc5817b956 -->

    <owl:Class rdf:about="http://purl.org/net/iot-dm#OWLClass_d95c726a_c63f_4e85_b9da_25bc5817b956">
        <rdfs:subClassOf rdf:resource="http://purl.org/net/iot-dm#OWLClass_bec04496_99a7_4304_ab0c_85592a8bdfca"/>
        <rdfs:label xml:lang="en">Https</rdfs:label>
    </owl:Class>
    


    <!-- http://purl.org/net/iot-dm#OWLClass_da2307f8_c03c_43a0_b2d7_2a16bfb7bf1d -->

    <owl:Class rdf:about="http://purl.org/net/iot-dm#OWLClass_da2307f8_c03c_43a0_b2d7_2a16bfb7bf1d">
        <rdfs:subClassOf rdf:resource="http://purl.org/net/iot-dm#OWLClass_195de59b_34c2_45da_8aa8_591cd3847fc7"/>
        <rdfs:comment>OMA-RD-LightweightM2M-V1_1-20180710-A, Label: LightweightM2M-E2E-13</rdfs:comment>
        <rdfs:label xml:lang="en">SeparatelyVerifiableMessageFragments</rdfs:label>
    </owl:Class>
    


    <!-- http://purl.org/net/iot-dm#OWLClass_da249273_d7c6_4881_83fd_88aba0709718 -->

    <owl:Class rdf:about="http://purl.org/net/iot-dm#OWLClass_da249273_d7c6_4881_83fd_88aba0709718">
        <rdfs:subClassOf rdf:resource="http://purl.org/net/iot-dm#OWLClass_62fae845_5a8c_4d71_980f_2f8cea75de35"/>
        <rdfs:comment>IoT home gateway for auto-conﬁguration and management of MQTT devices, section III.</rdfs:comment>
        <rdfs:label xml:lang="en">DeviceControlMessagePushdown</rdfs:label>
    </owl:Class>
    


    <!-- http://purl.org/net/iot-dm#OWLClass_da50a2d9_4834_46a1_8732_acd2c232e6fe -->

    <owl:Class rdf:about="http://purl.org/net/iot-dm#OWLClass_da50a2d9_4834_46a1_8732_acd2c232e6fe">
        <rdfs:subClassOf rdf:resource="http://purl.org/net/iot-dm#OWLClass_6cb818a3_6278_4bad_8a6b_c01ee623c677"/>
        <rdfs:comment>OMA-RD-LightweightM2M-V1_0-20170208-A, Label: LightweightM2M-HLF-011</rdfs:comment>
        <rdfs:label xml:lang="en">PhysicalDeviceRessourcesEnablingAndDisabling</rdfs:label>
    </owl:Class>
    


    <!-- http://purl.org/net/iot-dm#OWLClass_dc03e030_6d6c_4437_b2df_51251234a10e -->

    <owl:Class rdf:about="http://purl.org/net/iot-dm#OWLClass_dc03e030_6d6c_4437_b2df_51251234a10e">
        <rdfs:subClassOf rdf:resource="http://purl.org/net/iot-dm#OWLClass_4daf23df_ce27_4a36_8ce8_efb91ef3cef6"/>
        <rdfs:comment>Management of IoT Devices in a Physical Network, p. 488, 490, 492</rdfs:comment>
        <rdfs:label xml:lang="en">ActionTriggers</rdfs:label>
    </owl:Class>
    


    <!-- http://purl.org/net/iot-dm#OWLClass_dd21fadb_8dfb_46e9_a311_b39ddefaad69 -->

    <owl:Class rdf:about="http://purl.org/net/iot-dm#OWLClass_dd21fadb_8dfb_46e9_a311_b39ddefaad69">
        <rdfs:subClassOf rdf:resource="http://purl.org/net/iot-dm#OWLClass_2fb332cc_9b13_4fbc_af07_4ce1a662e062"/>
        <rdfs:comment>Recent Advances in Industrial Wireless Sensor Networks Towards Efficient Management in IoT, p. 9</rdfs:comment>
        <rdfs:label xml:lang="en">DeviceStatus</rdfs:label>
    </owl:Class>
    


    <!-- http://purl.org/net/iot-dm#OWLClass_dd852ca2_21fe_412c_ba77_747bdc3e8cb0 -->

    <owl:Class rdf:about="http://purl.org/net/iot-dm#OWLClass_dd852ca2_21fe_412c_ba77_747bdc3e8cb0">
        <rdfs:subClassOf rdf:resource="http://purl.org/net/iot-dm#OWLClass_9e1800f6_b3ba_41ee_b0ce_dac66a1a8680"/>
        <rdfs:label xml:lang="en">InternetLayerProtocol</rdfs:label>
    </owl:Class>
    


    <!-- http://purl.org/net/iot-dm#OWLClass_defe9266_4e6d_4036_8134_4ad7f7a4797e -->

    <owl:Class rdf:about="http://purl.org/net/iot-dm#OWLClass_defe9266_4e6d_4036_8134_4ad7f7a4797e">
        <rdfs:subClassOf rdf:resource="http://purl.org/net/iot-dm#OWLClass_d5baf8ff_3ca0_40a1_988a_a5e23a144824"/>
        <rdfs:comment>Recent Advances in Industrial Wireless Sensor Networks Towards Efficient Management in IoT, p. 9</rdfs:comment>
        <rdfs:comment>ServiceEnablement</rdfs:comment>
        <rdfs:label xml:lang="en">ApplicationDataTransmission</rdfs:label>
    </owl:Class>
    


    <!-- http://purl.org/net/iot-dm#OWLClass_df3a8c65_3c73_47f9_9391_4f3082112ee4 -->

    <owl:Class rdf:about="http://purl.org/net/iot-dm#OWLClass_df3a8c65_3c73_47f9_9391_4f3082112ee4">
        <rdfs:subClassOf rdf:resource="http://purl.org/net/iot-dm#OWLClass_cbca8db6_d106_4651_a12c_b8fe629efbda"/>
        <rdfs:comment>Recent Advances in Industrial Wireless Sensor Networks Towards Efficient Management in IoT, p. 9</rdfs:comment>
        <rdfs:label xml:lang="en">ResourceObservation</rdfs:label>
    </owl:Class>
    


    <!-- http://purl.org/net/iot-dm#OWLClass_df537b47_a081_4de8_8904_3c63392ae836 -->

    <owl:Class rdf:about="http://purl.org/net/iot-dm#OWLClass_df537b47_a081_4de8_8904_3c63392ae836">
        <rdfs:subClassOf rdf:resource="http://purl.org/net/iot-dm#OWLClass_96668876_e17b_46e9_b086_5835d62ceaaa"/>
        <rdfs:comment>Management of IoT Devices in a Physical Network, p. 487</rdfs:comment>
        <rdfs:label xml:lang="en">DeviceKpis</rdfs:label>
    </owl:Class>
    


    <!-- http://purl.org/net/iot-dm#OWLClass_df6c8097_8c2d_4d16_9432_8735af0b6219 -->

    <owl:Class rdf:about="http://purl.org/net/iot-dm#OWLClass_df6c8097_8c2d_4d16_9432_8735af0b6219">
        <rdfs:subClassOf rdf:resource="http://purl.org/net/iot-dm#OWLClass_09ca2bb4_ca54_4693_816d_f45ba81e59fb"/>
        <rdfs:label xml:lang="en">DevicesWithoutGateway</rdfs:label>
    </owl:Class>
    


    <!-- http://purl.org/net/iot-dm#OWLClass_e00944d4_c070_4cf7_91ed_7f4c58ff50c8 -->

    <owl:Class rdf:about="http://purl.org/net/iot-dm#OWLClass_e00944d4_c070_4cf7_91ed_7f4c58ff50c8">
        <rdfs:subClassOf rdf:resource="http://purl.org/net/iot-dm#OWLClass_2c177064_e630_44da_bbb3_d692886a8e4a"/>
        <rdfs:label xml:lang="en">ConfigurableBootstrappingErrorFallbackMechanism</rdfs:label>
        <rdfs:seeAlso>OMA-RD-LightweightM2M-V1_1-20180710-A, Label: LightweightM2M-BsR-003</rdfs:seeAlso>
    </owl:Class>
    


    <!-- http://purl.org/net/iot-dm#OWLClass_e08e2786_4de4_4eb8_b28b_5d5fc6647ef1 -->

    <owl:Class rdf:about="http://purl.org/net/iot-dm#OWLClass_e08e2786_4de4_4eb8_b28b_5d5fc6647ef1">
        <rdfs:subClassOf rdf:resource="http://purl.org/net/iot-dm#OWLClass_6cb818a3_6278_4bad_8a6b_c01ee623c677"/>
        <rdfs:comment>OMA-RD-LightweightM2M-V1_0-20170208-A, Label: LightweightM2M-HLF-009</rdfs:comment>
        <rdfs:label xml:lang="en">DeviceFactoryReset</rdfs:label>
    </owl:Class>
    


    <!-- http://purl.org/net/iot-dm#OWLClass_e0a5dc16_da3c_4388_9b7e_ef806b814d12 -->

    <owl:Class rdf:about="http://purl.org/net/iot-dm#OWLClass_e0a5dc16_da3c_4388_9b7e_ef806b814d12">
        <rdfs:subClassOf rdf:resource="http://purl.org/net/iot-dm#OWLClass_b5c0d821_b62f_4098_9a87_9ab068cebe46"/>
        <rdfs:comment>Management of IoT Devices in a Physical Network, p. 488, 492</rdfs:comment>
        <rdfs:label xml:lang="en">Matching</rdfs:label>
    </owl:Class>
    


    <!-- http://purl.org/net/iot-dm#OWLClass_e3a74b22_351d_4806_be29_e5690e9c7b14 -->

    <owl:Class rdf:about="http://purl.org/net/iot-dm#OWLClass_e3a74b22_351d_4806_be29_e5690e9c7b14">
        <rdfs:subClassOf rdf:resource="http://purl.org/net/iot-dm#OWLClass_b5c0d821_b62f_4098_9a87_9ab068cebe46"/>
        <rdfs:comment>Management of IoT Devices in a Physical Network, p. 488</rdfs:comment>
        <rdfs:label xml:lang="en">Reasoning</rdfs:label>
    </owl:Class>
    


    <!-- http://purl.org/net/iot-dm#OWLClass_e468299f_e290_44f7_989c_7b1c80d2cf6b -->

    <owl:Class rdf:about="http://purl.org/net/iot-dm#OWLClass_e468299f_e290_44f7_989c_7b1c80d2cf6b">
        <rdfs:subClassOf rdf:resource="http://purl.org/net/iot-dm#OWLClass_201d2207_e63c_4bd0_ac8e_dac6fd8b7d61"/>
        <rdfs:comment>Recent Advances in Industrial Wireless Sensor Networks Towards Efficient Management in IoT, p. 13</rdfs:comment>
        <rdfs:label xml:lang="en">ProcessManagement</rdfs:label>
    </owl:Class>
    


    <!-- http://purl.org/net/iot-dm#OWLClass_e4fa8a9f_7683_40e0_bd25_190e3002f6c5 -->

    <owl:Class rdf:about="http://purl.org/net/iot-dm#OWLClass_e4fa8a9f_7683_40e0_bd25_190e3002f6c5">
        <rdfs:subClassOf rdf:resource="http://purl.org/net/iot-dm#OWLClass_defe9266_4e6d_4036_8134_4ad7f7a4797e"/>
        <rdfs:comment>OMA-RD-LightweightM2M-V1_1-20180710-A, Label: LightweightM2M-DSE-003</rdfs:comment>
        <rdfs:label xml:lang="en">AllowReportOfUnsolicitedDataByDevice</rdfs:label>
    </owl:Class>
    


    <!-- http://purl.org/net/iot-dm#OWLClass_e512b9bb_a591_4c14_9a22_c4819142eb18 -->

    <owl:Class rdf:about="http://purl.org/net/iot-dm#OWLClass_e512b9bb_a591_4c14_9a22_c4819142eb18">
        <rdfs:subClassOf rdf:resource="http://purl.org/net/iot-dm#OWLClass_3a4d744e_1ddc_4fc8_be82_966b2e491882"/>
        <rdfs:comment xml:lang="en">&quot;Firmware images and manifests are stored on untrusted fileservers or cloud storage infrastructure. Some deployments may require storage of the firmware images/manifests to be stored on various entities before they reach the device.&quot;, draft-moran-suit-architecture-03 (work in progress), p. 5</rdfs:comment>
        <rdfs:label xml:lang="en">UntrustedFirmwareStorage</rdfs:label>
    </owl:Class>
    


    <!-- http://purl.org/net/iot-dm#OWLClass_e5962d5f_21c4_44f3_9ffa_9d9ee33b4f99 -->

    <owl:Class rdf:about="http://purl.org/net/iot-dm#OWLClass_e5962d5f_21c4_44f3_9ffa_9d9ee33b4f99">
        <rdfs:subClassOf rdf:resource="http://purl.org/net/iot-dm#OWLClass_ae34f5cf_8888_4de3_9170_7e8f6eab5f86"/>
        <rdfs:comment>https://resin.io/how-it-works/, 2018-09-16</rdfs:comment>
        <rdfs:label xml:lang="en">ContainerAssembly</rdfs:label>
    </owl:Class>
    


    <!-- http://purl.org/net/iot-dm#OWLClass_e68b7577_38f1_497e_8b5c_229be057d711 -->

    <owl:Class rdf:about="http://purl.org/net/iot-dm#OWLClass_e68b7577_38f1_497e_8b5c_229be057d711">
        <rdfs:subClassOf rdf:resource="http://purl.org/net/iot-dm#OWLClass_36c8fbfb_7218_4373_a13b_f46a86f007be"/>
        <rdfs:label xml:lang="en">UserProvidedDeviceInfomation</rdfs:label>
    </owl:Class>
    


    <!-- http://purl.org/net/iot-dm#OWLClass_e68cce3c_c023_425e_bbcf_ab80711b21d3 -->

    <owl:Class rdf:about="http://purl.org/net/iot-dm#OWLClass_e68cce3c_c023_425e_bbcf_ab80711b21d3">
        <rdfs:subClassOf rdf:resource="http://purl.org/net/iot-dm#OWLClass_88bd0206_ec77_40fc_bde2_6c1e2637b12a"/>
        <rdfs:comment>https://resin.io/how-it-works/, 2019-09-16</rdfs:comment>
        <rdfs:label xml:lang="en">Stderr</rdfs:label>
    </owl:Class>
    


    <!-- http://purl.org/net/iot-dm#OWLClass_e73ce412_848f_4de5_aadb_256be525abe9 -->

    <owl:Class rdf:about="http://purl.org/net/iot-dm#OWLClass_e73ce412_848f_4de5_aadb_256be525abe9">
        <rdfs:subClassOf rdf:resource="http://purl.org/net/iot-dm#OWLClass_9706d318_5cd1_4e58_8c3b_72eef36ee70a"/>
        <rdfs:comment>draft-moran-suit-architecture-03 (work in progress), p. 12</rdfs:comment>
        <rdfs:label xml:lang="en">CryptographicInformation</rdfs:label>
    </owl:Class>
    


    <!-- http://purl.org/net/iot-dm#OWLClass_e7bf4653_bddc_4792_b111_b527b50ea755 -->

    <owl:Class rdf:about="http://purl.org/net/iot-dm#OWLClass_e7bf4653_bddc_4792_b111_b527b50ea755">
        <rdfs:subClassOf rdf:resource="http://purl.org/net/iot-dm#OWLClass_df537b47_a081_4de8_8904_3c63392ae836"/>
        <rdfs:comment>Management of IoT Devices in a Physical Network, p. 487</rdfs:comment>
        <rdfs:label xml:lang="en">KpiDefinition</rdfs:label>
    </owl:Class>
    


    <!-- http://purl.org/net/iot-dm#OWLClass_e7e81967_1b1b_4dfb_b9b6_c40e0ffab441 -->

    <owl:Class rdf:about="http://purl.org/net/iot-dm#OWLClass_e7e81967_1b1b_4dfb_b9b6_c40e0ffab441">
        <rdfs:subClassOf rdf:resource="http://purl.org/net/iot-dm#OWLClass_66c3fc69_337f_4795_a467_f0b64b90cb3b"/>
        <rdfs:comment>Recent Advances in Industrial Wireless Sensor Networks Towards Efficient Management in IoT, p. 13</rdfs:comment>
        <rdfs:label xml:lang="en">Security</rdfs:label>
    </owl:Class>
    


    <!-- http://purl.org/net/iot-dm#OWLClass_e7f24ae4_85a4_48f4_be0a_4110909373bb -->

    <owl:Class rdf:about="http://purl.org/net/iot-dm#OWLClass_e7f24ae4_85a4_48f4_be0a_4110909373bb">
        <rdfs:subClassOf rdf:resource="http://purl.org/net/iot-dm#OWLClass_a1b8792e_7d00_48b8_9efe_c6e47629e99c"/>
        <rdfs:comment>Recent Advances in Industrial Wireless Sensor Networks Towards Efficient Management in IoT, p. 13</rdfs:comment>
        <rdfs:label xml:lang="en">SensorDataAnalytics</rdfs:label>
    </owl:Class>
    


    <!-- http://purl.org/net/iot-dm#OWLClass_e88e14ac_6d0e_41b7_9a94_bcc9b084f763 -->

    <owl:Class rdf:about="http://purl.org/net/iot-dm#OWLClass_e88e14ac_6d0e_41b7_9a94_bcc9b084f763">
        <rdfs:subClassOf rdf:resource="http://purl.org/net/iot-dm#OWLClass_6cb818a3_6278_4bad_8a6b_c01ee623c677"/>
        <rdfs:comment>OMA-RD-LightweightM2M-V1_0-20170208-A, Label: LightweightM2M-HLF-029</rdfs:comment>
        <rdfs:label xml:lang="en">DataReportingBearerConfiguration</rdfs:label>
    </owl:Class>
    


    <!-- http://purl.org/net/iot-dm#OWLClass_e8bba4e0_1b39_45bf_b031_aaa20123bd06 -->

    <owl:Class rdf:about="http://purl.org/net/iot-dm#OWLClass_e8bba4e0_1b39_45bf_b031_aaa20123bd06">
        <rdfs:subClassOf rdf:resource="http://purl.org/net/iot-dm#OWLClass_66c3fc69_337f_4795_a467_f0b64b90cb3b"/>
        <rdfs:label xml:lang="en">DataIntegrity</rdfs:label>
    </owl:Class>
    


    <!-- http://purl.org/net/iot-dm#OWLClass_e9559715_ca44_42e4_ab33_3545bec40f7e -->

    <owl:Class rdf:about="http://purl.org/net/iot-dm#OWLClass_e9559715_ca44_42e4_ab33_3545bec40f7e">
        <rdfs:subClassOf rdf:resource="http://purl.org/net/iot-dm#OWLClass_a6f072f9_98b2_40d1_ba35_6dc98cfeeb54"/>
        <rdfs:comment>Recent Advances in Industrial Wireless Sensor Networks Towards Efficient Management in IoT, p. 12</rdfs:comment>
        <rdfs:label xml:lang="en">ApplicationDevelopmentEnvironment</rdfs:label>
    </owl:Class>
    


    <!-- http://purl.org/net/iot-dm#OWLClass_e96a1119_08e8_4614_80e8_2ecbeb431739 -->

    <owl:Class rdf:about="http://purl.org/net/iot-dm#OWLClass_e96a1119_08e8_4614_80e8_2ecbeb431739">
        <rdfs:subClassOf rdf:resource="http://purl.org/net/iot-dm#OWLClass_1d7dd666_95ba_4c41_9a91_d850e9c0f479"/>
        <rdfs:comment>OMA-RD-LightweightM2M-V1_1-20180710-A, Label: LightweightM2M-ENC-2</rdfs:comment>
        <rdfs:label xml:lang="en">EfficientEncodingAndDecoding</rdfs:label>
    </owl:Class>
    


    <!-- http://purl.org/net/iot-dm#OWLClass_e9d7d7c5_7e8c_4097_b246_1c97529acb5e -->

    <owl:Class rdf:about="http://purl.org/net/iot-dm#OWLClass_e9d7d7c5_7e8c_4097_b246_1c97529acb5e">
        <rdfs:subClassOf rdf:resource="http://purl.org/net/iot-dm#OWLClass_1bd19af8_5e90_482f_b798_79ba7cc8d671"/>
        <rdfs:comment>Ontologies for the Internet of Things, 1.</rdfs:comment>
        <rdfs:label xml:lang="en">ServiceAvailabilityLimitationHandling</rdfs:label>
    </owl:Class>
    


    <!-- http://purl.org/net/iot-dm#OWLClass_ea3d6bb7_6214_4f65_b908_d0465750090d -->

    <owl:Class rdf:about="http://purl.org/net/iot-dm#OWLClass_ea3d6bb7_6214_4f65_b908_d0465750090d">
        <rdfs:subClassOf rdf:resource="http://purl.org/net/iot-dm#OWLClass_14f6ac55_025a_4626_934b_e27de3af1145"/>
        <rdfs:comment>Recent Advances in Industrial Wireless Sensor Networks Towards Efficient Management in IoT, p. 12, 13</rdfs:comment>
        <rdfs:label xml:lang="en">FailureHandling</rdfs:label>
    </owl:Class>
    


    <!-- http://purl.org/net/iot-dm#OWLClass_ea675ce3_19d4_451f_948a_dfdbe92e4d75 -->

    <owl:Class rdf:about="http://purl.org/net/iot-dm#OWLClass_ea675ce3_19d4_451f_948a_dfdbe92e4d75">
        <rdfs:subClassOf rdf:resource="http://purl.org/net/iot-dm#OWLClass_9706d318_5cd1_4e58_8c3b_72eef36ee70a"/>
        <rdfs:comment>draft-moran-suit-architecture-03 (work in progress), p. 12</rdfs:comment>
        <rdfs:label xml:lang="en">DependenciesToOtherManifests</rdfs:label>
    </owl:Class>
    


    <!-- http://purl.org/net/iot-dm#OWLClass_eacb3011_0e6b_4345_927b_71cd05935ed8 -->

    <owl:Class rdf:about="http://purl.org/net/iot-dm#OWLClass_eacb3011_0e6b_4345_927b_71cd05935ed8">
        <rdfs:subClassOf rdf:resource="http://purl.org/net/iot-dm#OWLClass_3d63ac6a_4939_44eb_afc5_ebab6cf1cf53"/>
        <rdfs:comment>OMA-RD-LightweightM2M-V1_1-20180710-A, Label: LightweightM2M-SCS-5</rdfs:comment>
        <rdfs:label xml:lang="en">ObjectInstanceStorageLocationIndication</rdfs:label>
    </owl:Class>
    


    <!-- http://purl.org/net/iot-dm#OWLClass_eb55e31a_c8b3_4bd9_809d_197359daa7a4 -->

    <owl:Class rdf:about="http://purl.org/net/iot-dm#OWLClass_eb55e31a_c8b3_4bd9_809d_197359daa7a4">
        <rdfs:subClassOf rdf:resource="http://purl.org/net/iot-dm#OWLClass_88bd0206_ec77_40fc_bde2_6c1e2637b12a"/>
        <rdfs:comment>OMA-RD-LightweightM2M-V1_0-20170208-A, Label: LightweightM2M-HLF-038</rdfs:comment>
        <rdfs:label xml:lang="en">ConnectionLog</rdfs:label>
    </owl:Class>
    


    <!-- http://purl.org/net/iot-dm#OWLClass_eb872de9_1d72_443b_a517_5502e0766fe4 -->

    <owl:Class rdf:about="http://purl.org/net/iot-dm#OWLClass_eb872de9_1d72_443b_a517_5502e0766fe4">
        <rdfs:subClassOf rdf:resource="http://purl.org/net/iot-dm#OWLClass_8c2c705b_ddcf_4dc0_b9d5_6e507868806e"/>
        <rdfs:comment>OMA-RD-LightweightM2M-V1_0-20170208-A, Label: LightweightM2M-HLF-025</rdfs:comment>
        <rdfs:label xml:lang="en">DeviceRadioSignalStrength</rdfs:label>
    </owl:Class>
    


    <!-- http://purl.org/net/iot-dm#OWLClass_ebbfff77_6bbb_477e_9f30_934e7239601e -->

    <owl:Class rdf:about="http://purl.org/net/iot-dm#OWLClass_ebbfff77_6bbb_477e_9f30_934e7239601e">
        <rdfs:label xml:lang="en">InternetOfThingsPlatform</rdfs:label>
    </owl:Class>
    


    <!-- http://purl.org/net/iot-dm#OWLClass_ebf6283b_1c32_4dee_b1ba_5c32f88cd39c -->

    <owl:Class rdf:about="http://purl.org/net/iot-dm#OWLClass_ebf6283b_1c32_4dee_b1ba_5c32f88cd39c">
        <rdfs:subClassOf rdf:resource="http://purl.org/net/iot-dm#OWLClass_a6cf31e3_5d7b_48b4_bce6_eada63815264"/>
        <rdfs:label xml:lang="en">UnixLikeOperatingSystem</rdfs:label>
    </owl:Class>
    


    <!-- http://purl.org/net/iot-dm#OWLClass_ec9156ee_5023_4804_9c7c_19a9a4ad18b4 -->

    <owl:Class rdf:about="http://purl.org/net/iot-dm#OWLClass_ec9156ee_5023_4804_9c7c_19a9a4ad18b4">
        <rdfs:subClassOf rdf:resource="http://purl.org/net/iot-dm#OWLClass_ffcb0dd3_5746_4e9b_9905_50bfb9faff34"/>
        <rdfs:comment>Recent Advances in Industrial Wireless Sensor Networks Towards Efficient Management in IoT, p. 6</rdfs:comment>
        <rdfs:label xml:lang="en">ReliableCommunication</rdfs:label>
    </owl:Class>
    


    <!-- http://purl.org/net/iot-dm#OWLClass_ed6289ac_7d66_409b_825b_ecca07856dd0 -->

    <owl:Class rdf:about="http://purl.org/net/iot-dm#OWLClass_ed6289ac_7d66_409b_825b_ecca07856dd0">
        <rdfs:subClassOf rdf:resource="http://purl.org/net/iot-dm#OWLClass_42d9f56b_27ca_411a_8c4f_91ecb085e413"/>
        <rdfs:comment>OMA-RD-LightweightM2M-V1_1-20180710-A, Label: LightweightM2M-TLS-002</rdfs:comment>
        <rdfs:label xml:lang="en">TlsDtlsErrorHandlingProcedures</rdfs:label>
    </owl:Class>
    


    <!-- http://purl.org/net/iot-dm#OWLClass_edabf253_b496_407b_acae_0404f2e7d43b -->

    <owl:Class rdf:about="http://purl.org/net/iot-dm#OWLClass_edabf253_b496_407b_acae_0404f2e7d43b">
        <rdfs:subClassOf rdf:resource="http://purl.org/net/iot-dm#OWLClass_beae1841_eca4_4666_bf75_5e2665a737e8"/>
        <rdfs:comment xml:lang="en">draft-moran-suit-architecture-03 (work in progress), p. 4</rdfs:comment>
        <rdfs:label xml:lang="en">MaliciousFirmwareImageFlashingPrevention</rdfs:label>
    </owl:Class>
    


    <!-- http://purl.org/net/iot-dm#OWLClass_ef9faee2_1aea_4a46_b8a3_68bfe5a1e1be -->

    <owl:Class rdf:about="http://purl.org/net/iot-dm#OWLClass_ef9faee2_1aea_4a46_b8a3_68bfe5a1e1be">
        <rdfs:subClassOf rdf:resource="http://purl.org/net/iot-dm#OWLClass_88bd0206_ec77_40fc_bde2_6c1e2637b12a"/>
        <rdfs:comment>https://resin.io/how-it-works/, 2019-09-16</rdfs:comment>
        <rdfs:label xml:lang="en">ContainerSupervisorLogs</rdfs:label>
    </owl:Class>
    


    <!-- http://purl.org/net/iot-dm#OWLClass_efe7810e_2a97_4b8e_9967_d305e3277152 -->

    <owl:Class rdf:about="http://purl.org/net/iot-dm#OWLClass_efe7810e_2a97_4b8e_9967_d305e3277152">
        <rdfs:subClassOf rdf:resource="http://purl.org/net/iot-dm#OWLClass_f1b54d5c_4482_4645_a2f1_6efa8e12b8de"/>
        <rdfs:label xml:lang="en">Wireless</rdfs:label>
    </owl:Class>
    


    <!-- http://purl.org/net/iot-dm#OWLClass_f0ff9712_08e7_405e_ae96_7d6c3f319b37 -->

    <owl:Class rdf:about="http://purl.org/net/iot-dm#OWLClass_f0ff9712_08e7_405e_ae96_7d6c3f319b37">
        <rdfs:subClassOf rdf:resource="http://purl.org/net/iot-dm#OWLClass_38e18d87_aade_4d8b_ab6e_1da467276a13"/>
        <rdfs:comment>Recent Advances in Industrial Wireless Sensor Networks Towards Efficient Management in IoT, p. 13</rdfs:comment>
        <rdfs:label xml:lang="en">DeviceName</rdfs:label>
    </owl:Class>
    


    <!-- http://purl.org/net/iot-dm#OWLClass_f1b54d5c_4482_4645_a2f1_6efa8e12b8de -->

    <owl:Class rdf:about="http://purl.org/net/iot-dm#OWLClass_f1b54d5c_4482_4645_a2f1_6efa8e12b8de">
        <rdfs:subClassOf rdf:resource="http://purl.org/net/iot-dm#OWLClass_f9c2dcec_1d84_4a42_b0ba_c8c976636fd2"/>
        <rdfs:label xml:lang="en">DataTransferMechanism</rdfs:label>
    </owl:Class>
    


    <!-- http://purl.org/net/iot-dm#OWLClass_f1d1ac4d_e983_4876_ac01_41db93c58b88 -->

    <owl:Class rdf:about="http://purl.org/net/iot-dm#OWLClass_f1d1ac4d_e983_4876_ac01_41db93c58b88">
        <rdfs:subClassOf rdf:resource="http://purl.org/net/iot-dm#OWLClass_195de59b_34c2_45da_8aa8_591cd3847fc7"/>
        <rdfs:comment>OMA-RD-LightweightM2M-V1_1-20180710-A, Label: LightweightM2M-E2E-10</rdfs:comment>
        <rdfs:comment>OMA-RD-LightweightM2M-V1_1-20180710-A, Label: LightweightM2M-E2E-4</rdfs:comment>
        <rdfs:comment>OMA-RD-LightweightM2M-V1_1-20180710-A, Label: LightweightM2M-E2Eo-10</rdfs:comment>
        <rdfs:comment>OMA-RD-LightweightM2M-V1_1-20180710-A, Label: LightweightM2M-E2Eo-4</rdfs:comment>
        <rdfs:label xml:lang="en">Authentication</rdfs:label>
    </owl:Class>
    


    <!-- http://purl.org/net/iot-dm#OWLClass_f1d3bcad_a4a4_4c9b_9bc8_01fc7df976b4 -->

    <owl:Class rdf:about="http://purl.org/net/iot-dm#OWLClass_f1d3bcad_a4a4_4c9b_9bc8_01fc7df976b4">
        <rdfs:subClassOf rdf:resource="http://purl.org/net/iot-dm#OWLClass_30d8bc8b_4188_4a4f_be58_c4d70f00474e"/>
        <rdfs:comment>https://resin.io/how-it-works/, 2018-09-16</rdfs:comment>
        <rdfs:label xml:lang="en">ApplicationContainer</rdfs:label>
    </owl:Class>
    


    <!-- http://purl.org/net/iot-dm#OWLClass_f4a64f37_cafb_440d_8e03_c1895c63f6ea -->

    <owl:Class rdf:about="http://purl.org/net/iot-dm#OWLClass_f4a64f37_cafb_440d_8e03_c1895c63f6ea">
        <rdfs:subClassOf rdf:resource="http://purl.org/net/iot-dm#OWLClass_59540155_cb79_4e35_8db8_7519fb3535d5"/>
        <rdfs:label xml:lang="en">DeviceOverview</rdfs:label>
    </owl:Class>
    


    <!-- http://purl.org/net/iot-dm#OWLClass_f4c68c89_a4ee_4e3f_b527_9a88d50887fe -->

    <owl:Class rdf:about="http://purl.org/net/iot-dm#OWLClass_f4c68c89_a4ee_4e3f_b527_9a88d50887fe">
        <rdfs:subClassOf rdf:resource="http://purl.org/net/iot-dm#OWLClass_9e3d4f19_96c7_4932_a007_26fa592f3423"/>
        <rdfs:comment>The Internet of Things: An Overview, p. 25</rdfs:comment>
        <rdfs:label xml:lang="en">DeviceManagementAgent</rdfs:label>
    </owl:Class>
    


    <!-- http://purl.org/net/iot-dm#OWLClass_f519e17a_515d_402f_a5da_1cffe41727ea -->

    <owl:Class rdf:about="http://purl.org/net/iot-dm#OWLClass_f519e17a_515d_402f_a5da_1cffe41727ea">
        <rdfs:subClassOf rdf:resource="http://purl.org/net/iot-dm#OWLClass_f9db282e_22e2_48e5_a643_a42df05c880d"/>
        <rdfs:comment>&quot;translate the captured event from the sensor devices into a standard format and deliver it through broadband or wireless networks to the cloud platform&quot;, Recent Advances in Industrial Wireless Sensor Networks Towards Efficient Management in IoT, p. 6</rdfs:comment>
        <rdfs:label xml:lang="en">DeviceAdapter</rdfs:label>
    </owl:Class>
    


    <!-- http://purl.org/net/iot-dm#OWLClass_f54399c8_de31_4d25_a3e2_8bf624ed0afb -->

    <owl:Class rdf:about="http://purl.org/net/iot-dm#OWLClass_f54399c8_de31_4d25_a3e2_8bf624ed0afb">
        <rdfs:subClassOf rdf:resource="http://purl.org/net/iot-dm#OWLClass_ae34f5cf_8888_4de3_9170_7e8f6eab5f86"/>
        <rdfs:comment>https://resin.io/how-it-works/, 2019-09-16</rdfs:comment>
        <rdfs:label xml:lang="en">ContainerShutdown</rdfs:label>
    </owl:Class>
    


    <!-- http://purl.org/net/iot-dm#OWLClass_f5785649_0a85_47a8_a029_1d752a693e0a -->

    <owl:Class rdf:about="http://purl.org/net/iot-dm#OWLClass_f5785649_0a85_47a8_a029_1d752a693e0a">
        <rdfs:subClassOf rdf:resource="http://purl.org/net/iot-dm#OWLClass_cfc68839_b898_454c_9314_0822698917f2"/>
        <rdfs:comment>OMA-RD-LightweightM2M-V1_0-20170208-A, Label: LightweightM2M-HLF-003</rdfs:comment>
        <rdfs:label xml:lang="en">InstalledFirmwareVersion</rdfs:label>
    </owl:Class>
    


    <!-- http://purl.org/net/iot-dm#OWLClass_f58b9658_2ee9_4f41_83f0_3bbdce1de398 -->

    <owl:Class rdf:about="http://purl.org/net/iot-dm#OWLClass_f58b9658_2ee9_4f41_83f0_3bbdce1de398">
        <rdfs:subClassOf rdf:resource="http://purl.org/net/iot-dm#OWLClass_574c5366_c20d_467b_8ad6_787581d5f349"/>
        <rdfs:comment>Recent Advances in Industrial Wireless Sensor Networks Towards Efficient Management in IoT, p. 6</rdfs:comment>
        <rdfs:label xml:lang="en">ProtocolConversion</rdfs:label>
    </owl:Class>
    


    <!-- http://purl.org/net/iot-dm#OWLClass_f6444fa6_1240_4dfa_9bba_affd175076ca -->

    <owl:Class rdf:about="http://purl.org/net/iot-dm#OWLClass_f6444fa6_1240_4dfa_9bba_affd175076ca">
        <rdfs:subClassOf rdf:resource="http://purl.org/net/iot-dm#OWLClass_9e3d4f19_96c7_4932_a007_26fa592f3423"/>
        <rdfs:label xml:lang="en">DataReportingMechanisms</rdfs:label>
    </owl:Class>
    


    <!-- http://purl.org/net/iot-dm#OWLClass_f6834970_02d2_44b4_afa3_984bfb353727 -->

    <owl:Class rdf:about="http://purl.org/net/iot-dm#OWLClass_f6834970_02d2_44b4_afa3_984bfb353727">
        <rdfs:subClassOf rdf:resource="http://purl.org/net/iot-dm#OWLClass_169f3b27_aa22_4707_936a_088618ef2999"/>
        <rdfs:comment>draft-moran-suit-architecture-03 (work in progress), p. 7-8</rdfs:comment>
        <rdfs:label xml:lang="en">OperatorConfirmationBeforeUpdate</rdfs:label>
    </owl:Class>
    


    <!-- http://purl.org/net/iot-dm#OWLClass_f86901a5_61d3_4e5a_8ec6_984ffda5de83 -->

    <owl:Class rdf:about="http://purl.org/net/iot-dm#OWLClass_f86901a5_61d3_4e5a_8ec6_984ffda5de83">
        <rdfs:subClassOf rdf:resource="http://purl.org/net/iot-dm#OWLClass_0bbb7819_d9df_4553_8196_2a8ee5c4c6e6"/>
        <rdfs:comment>IoT home gateway for auto-conﬁguration and management of MQTT devices, section I.</rdfs:comment>
        <rdfs:comment>Recent Advances in Industrial Wireless Sensor Networks Towards Efficient Management in IoT, p. 12</rdfs:comment>
        <rdfs:label xml:lang="en">DeviceManagementBridge</rdfs:label>
    </owl:Class>
    


    <!-- http://purl.org/net/iot-dm#OWLClass_f8dc270e_05c8_4acc_8401_aa1e7c2d4cdf -->

    <owl:Class rdf:about="http://purl.org/net/iot-dm#OWLClass_f8dc270e_05c8_4acc_8401_aa1e7c2d4cdf">
        <rdfs:subClassOf rdf:resource="http://purl.org/net/iot-dm#OWLClass_1543e022_678c_4b10_9895_de120d944f03"/>
        <rdfs:comment>IoT home gateway for auto-conﬁguration and management of MQTT devices, section III.</rdfs:comment>
        <rdfs:label xml:lang="en">DeviceControlMessage</rdfs:label>
    </owl:Class>
    


    <!-- http://purl.org/net/iot-dm#OWLClass_f90a27f1_b907_4b25_8e8e_3614b29682e9 -->

    <owl:Class rdf:about="http://purl.org/net/iot-dm#OWLClass_f90a27f1_b907_4b25_8e8e_3614b29682e9">
        <rdfs:subClassOf rdf:resource="http://purl.org/net/iot-dm#OWLClass_e68b7577_38f1_497e_8b5c_229be057d711"/>
        <rdfs:comment>https://resin.io/features/, 2018-09-15</rdfs:comment>
        <rdfs:label xml:lang="en">Notes</rdfs:label>
    </owl:Class>
    


    <!-- http://purl.org/net/iot-dm#OWLClass_f9c2dcec_1d84_4a42_b0ba_c8c976636fd2 -->

    <owl:Class rdf:about="http://purl.org/net/iot-dm#OWLClass_f9c2dcec_1d84_4a42_b0ba_c8c976636fd2">
        <rdfs:label xml:lang="en">DataTransfer</rdfs:label>
    </owl:Class>
    


    <!-- http://purl.org/net/iot-dm#OWLClass_f9db282e_22e2_48e5_a643_a42df05c880d -->

    <owl:Class rdf:about="http://purl.org/net/iot-dm#OWLClass_f9db282e_22e2_48e5_a643_a42df05c880d">
        <rdfs:subClassOf rdf:resource="http://purl.org/net/iot-dm#OWLClass_0bbb7819_d9df_4553_8196_2a8ee5c4c6e6"/>
        <rdfs:label xml:lang="en">DeviceConnectivity</rdfs:label>
    </owl:Class>
    


    <!-- http://purl.org/net/iot-dm#OWLClass_fb0267bc_bf86_4446_ad0a_a300adb91c85 -->

    <owl:Class rdf:about="http://purl.org/net/iot-dm#OWLClass_fb0267bc_bf86_4446_ad0a_a300adb91c85">
        <rdfs:subClassOf rdf:resource="http://purl.org/net/iot-dm#OWLClass_13c796b1_46e2_4fc7_b2d1_299b6746d07f"/>
        <rdfs:comment>IoT home gateway for auto-conﬁguration and management of MQTT devices, section III.</rdfs:comment>
        <rdfs:label xml:lang="en">Uuid</rdfs:label>
    </owl:Class>
    


    <!-- http://purl.org/net/iot-dm#OWLClass_fcd9404e_bd15_4965_8208_dae7b7883655 -->

    <owl:Class rdf:about="http://purl.org/net/iot-dm#OWLClass_fcd9404e_bd15_4965_8208_dae7b7883655">
        <rdfs:subClassOf rdf:resource="http://purl.org/net/iot-dm#OWLClass_2ee3c907_2ad6_45fc_999f_299667c29188"/>
        <rdfs:label xml:lang="en">Mechanisms</rdfs:label>
    </owl:Class>
    


    <!-- http://purl.org/net/iot-dm#OWLClass_fd01a49f_3b5f_46f9_abfb_6c4a21997ea2 -->

    <owl:Class rdf:about="http://purl.org/net/iot-dm#OWLClass_fd01a49f_3b5f_46f9_abfb_6c4a21997ea2">
        <rdfs:subClassOf rdf:resource="http://purl.org/net/iot-dm#OWLClass_66c3fc69_337f_4795_a467_f0b64b90cb3b"/>
        <rdfs:comment>OMA-RD-LightweightM2M-V1_1-20180710-A, Label: LightweightM2M-LeG-002</rdfs:comment>
        <rdfs:label xml:lang="en">LegacyGatewayConfigurationSupport</rdfs:label>
    </owl:Class>
    


    <!-- http://purl.org/net/iot-dm#OWLClass_fd5e408d_9ebf_433d_b9cc_9ff5fb8945ec -->

    <owl:Class rdf:about="http://purl.org/net/iot-dm#OWLClass_fd5e408d_9ebf_433d_b9cc_9ff5fb8945ec">
        <rdfs:subClassOf rdf:resource="http://purl.org/net/iot-dm#OWLClass_6cb818a3_6278_4bad_8a6b_c01ee623c677"/>
        <rdfs:comment>OMA-RD-LightweightM2M-V1_0-20170208-A, Label: LightweightM2M-HLF-034</rdfs:comment>
        <rdfs:label xml:lang="en">DeviceResourceManagement</rdfs:label>
    </owl:Class>
    


    <!-- http://purl.org/net/iot-dm#OWLClass_fd976a8f_5722_4bc3_82e7_06a832fd9581 -->

    <owl:Class rdf:about="http://purl.org/net/iot-dm#OWLClass_fd976a8f_5722_4bc3_82e7_06a832fd9581">
        <rdfs:subClassOf rdf:resource="http://purl.org/net/iot-dm#OWLClass_1bd19af8_5e90_482f_b798_79ba7cc8d671"/>
        <rdfs:comment>Recent Advances in Industrial Wireless Sensor Networks Towards Efficient Management in IoT, p. 6</rdfs:comment>
        <rdfs:label xml:lang="en">IotComponentAbstraction</rdfs:label>
    </owl:Class>
    


    <!-- http://purl.org/net/iot-dm#OWLClass_fdbd52a2_d5aa_49e4_87de_ac4d1a1db37e -->

    <owl:Class rdf:about="http://purl.org/net/iot-dm#OWLClass_fdbd52a2_d5aa_49e4_87de_ac4d1a1db37e">
        <rdfs:subClassOf rdf:resource="http://purl.org/net/iot-dm#OWLClass_5c08eefa_8244_4272_b68c_6f24666eb49d"/>
        <rdfs:comment>OMA-RD-LightweightM2M-V1_1-20180710-A, Label: LightweightM2M-SCS-3</rdfs:comment>
        <rdfs:label xml:lang="en">SecureComponentManagement</rdfs:label>
    </owl:Class>
    


    <!-- http://purl.org/net/iot-dm#OWLClass_fe29038f_fa6a_4e4a_bd8d_193a2ba9554e -->

    <owl:Class rdf:about="http://purl.org/net/iot-dm#OWLClass_fe29038f_fa6a_4e4a_bd8d_193a2ba9554e">
        <rdfs:subClassOf rdf:resource="http://purl.org/net/iot-dm#OWLClass_829a4147_2a1d_44ea_a9ef_0efaae5eaa5b"/>
        <rdfs:comment>https://resin.io/features/, 2018-09-15</rdfs:comment>
        <rdfs:label xml:lang="en">JsonApi</rdfs:label>
    </owl:Class>
    


    <!-- http://purl.org/net/iot-dm#OWLClass_fe76d8fa_9eac_4291_88ca_ce15ffe1ac80 -->

    <owl:Class rdf:about="http://purl.org/net/iot-dm#OWLClass_fe76d8fa_9eac_4291_88ca_ce15ffe1ac80">
        <rdfs:subClassOf rdf:resource="http://purl.org/net/iot-dm#OWLClass_beae1841_eca4_4666_bf75_5e2665a737e8"/>
        <rdfs:comment>draft-moran-suit-architecture-03 (work in progress), p. 6</rdfs:comment>
        <rdfs:label xml:lang="en">FirmwareAuthorVerification</rdfs:label>
    </owl:Class>
    


    <!-- http://purl.org/net/iot-dm#OWLClass_ffcb0dd3_5746_4e9b_9905_50bfb9faff34 -->

    <owl:Class rdf:about="http://purl.org/net/iot-dm#OWLClass_ffcb0dd3_5746_4e9b_9905_50bfb9faff34">
        <rdfs:subClassOf rdf:resource="http://purl.org/net/iot-dm#OWLClass_66c3fc69_337f_4795_a467_f0b64b90cb3b"/>
        <rdfs:label xml:lang="en">CommunicationProtocol</rdfs:label>
    </owl:Class>
    


    <!-- 
    ///////////////////////////////////////////////////////////////////////////////////////
    //
    // General axioms
    //
    ///////////////////////////////////////////////////////////////////////////////////////
     -->

    <rdf:Description>
        <rdf:type rdf:resource="http://www.w3.org/2002/07/owl#AllDisjointClasses"/>
        <owl:members rdf:parseType="Collection">
            <rdf:Description rdf:about="http://purl.org/net/iot-dm#OWLClass_15514c90_84d5_4670_93a6_9566cb808feb"/>
            <rdf:Description rdf:about="http://purl.org/net/iot-dm#OWLClass_49ac79d7_c437_4c71_8da3_ae6ad1e83073"/>
            <rdf:Description rdf:about="http://purl.org/net/iot-dm#OWLClass_9706d318_5cd1_4e58_8c3b_72eef36ee70a"/>
        </owl:members>
    </rdf:Description>
    <rdf:Description>
        <rdf:type rdf:resource="http://www.w3.org/2002/07/owl#AllDisjointClasses"/>
        <owl:members rdf:parseType="Collection">
            <rdf:Description rdf:about="http://purl.org/net/iot-dm#OWLClass_5445a1b7_eb6b_4343_bd06_a0427b710d6d"/>
            <rdf:Description rdf:about="http://purl.org/net/iot-dm#OWLClass_b36b9cf5_86ad_4f75_8368_c8d26856c4bf"/>
            <rdf:Description rdf:about="http://purl.org/net/iot-dm#OWLClass_c35d26c2_65cc_49bd_9875_9932fb747dd5"/>
            <rdf:Description rdf:about="http://purl.org/net/iot-dm#OWLClass_dd852ca2_21fe_412c_ba77_747bdc3e8cb0"/>
        </owl:members>
    </rdf:Description>
</rdf:RDF>



<!-- Generated by the OWL API (version 4.2.8.20170104-2310) https://github.com/owlcs/owlapi -->

